# baseURI: http://qudt.org/2.0/vocab/scale/astrophysics
# imports: http://qudt.org/2.0/schema/qudt
# imports: http://www.linkedmodel.org/schema/vaem
# imports: http://www.linkedmodel.org/schema/vaem-xics
# imports: http://www.w3.org/2004/02/skos/core

# c14n-version: 3
@prefix dc: <http://purl.org/dc/elements/1.1/> .
@prefix dcterms: <http://purl.org/dc/terms/> .
@prefix dimension: <http://qudt.org/vocab/dimensionvector/> .
@prefix dtype: <http://www.linkedmodel.org/schema/dtype#> .
@prefix owl: <http://www.w3.org/2002/07/owl#> .
@prefix quantitykind: <http://qudt.org/vocab/quantitykind/> .
@prefix qudt: <http://qudt.org/schema/qudt/> .
@prefix rdf: <http://www.w3.org/1999/02/22-rdf-syntax-ns#> .
@prefix rdfs: <http://www.w3.org/2000/01/rdf-schema#> .
@prefix skos: <http://www.w3.org/2004/02/skos/core#> .
@prefix unit: <http://qudt.org/vocab/unit/> .
@prefix vaem: <http://www.linkedmodel.org/schema/vaem#> .
@prefix voag: <http://voag.linkedmodel.org/schema/voag#> .
@prefix xsd: <http://www.w3.org/2001/XMLSchema#> .
<http://qudt.org/2.0/vocab/scale/astrophysics>
  rdf:type owl:Ontology ;
  dc:author "Ralph Hodgson"^^xsd:string ;
  dc:contributor "Irene Polikoff"^^xsd:string ;
  dc:creator "Ralph Hodgson"^^xsd:string ;
  dc:rights "The QUDT Scale Vocabularies are issued under a Creative Commons Attribution Share Alike 3.0 United States License. Attribution should be made to NASA Ames Research Center and TopQuadrant, Inc."^^xsd:string ;
  dc:subject "Scales"^^xsd:string ;
  dc:title "Astrophysics Scales"^^xsd:string ;
  vaem:dateCreated "2010-12-30T21:26:38"^^xsd:dateTime ;
  vaem:description "The QUDT Astrophysics Scales Vocabulary is an RDF/OWL specifications of scales relating to cosmology and solar system phenomena."^^xsd:string ;
  vaem:hasDisciplineScope "All Disciplines"^^xsd:string ;
  vaem:hasDomainScope "Science and Engineering Units"^^xsd:string ;
  vaem:hasGraphRole vaem:VocabularyGraph ;
  vaem:hasLicenseType voag:CC-SHAREALIKE_3PT0-US ;
  vaem:intent "To provide a vocabulary of commonly used units. This comprises the SI and many non-SI Units."^^xsd:string ;
  vaem:lastUpdated "$LastChangedDate: 2011-06-01 15:18:25 -0700 (Wed, 01 Jun 2011) $"^^xsd:string ;
  vaem:namespace "http://qudt.org/vocab/unit"^^xsd:string ;
  vaem:namespacePrefix "unit"^^xsd:string ;
  vaem:ownedBy "qudt.org"^^xsd:string ;
  vaem:revision "1.1"^^xsd:string ;
  vaem:usesNonImportedResource dc:author ;
  vaem:usesNonImportedResource dc:contributor ;
  vaem:usesNonImportedResource dc:creator ;
  vaem:usesNonImportedResource dc:description ;
  vaem:usesNonImportedResource dc:rights ;
  vaem:usesNonImportedResource dc:subject ;
  vaem:usesNonImportedResource dc:title ;
  vaem:usesNonImportedResource voag:CC-SHAREALIKE_3PT0-US ;
  vaem:usesNonImportedResource voag:QUDT-Attribution ;
  vaem:usesNonImportedResource voag:hasCatalogEntry ;
  vaem:usesNonImportedResource voag:hasLicenseType ;
  vaem:usesNonImportedResource voag:withAttributionTo ;
  vaem:withAttributionTo voag:QUDT-Attribution ;
  rdfs:label "QUDT Scales: Astrophysics"^^xsd:string ;
  owl:imports <http://qudt.org/2.1/schema/facade/qudt> ;
  owl:imports <http://www.linkedmodel.org/schema/vaem> ;
  owl:imports <http://www.w3.org/2004/02/skos/core> ;
  owl:versionIRI <http://qudt.org/2.0/vocab/unit/base> ;
.
qudt:TorinoScale
  rdf:type qudt:EnumerationScale ;
  dc:description """The Torino Scale is for assessing asteroid and comet impact hazard predictions in the 21st Century.



Reference: Morrison, D., Chapman, C. R., Steel, D., and Binzel R. P. \"Impacts and the Public: Communicating the Nature of the Impact Hazard\" In Mitigation of Hazardous Comets and Asteroids,(M.J.S. Belton, T.H. Morgan, N.H. Samarasinha and D.K. Yeomans, Eds), Cambridge University Press, 2004."""^^xsd:string ;
  dtype:value qudt:TorinoScaleValue_00 ;
  dtype:value qudt:TorinoScaleValue_01 ;
  dtype:value qudt:TorinoScaleValue_02 ;
  dtype:value qudt:TorinoScaleValue_03 ;
  dtype:value qudt:TorinoScaleValue_04 ;
  dtype:value qudt:TorinoScaleValue_05 ;
  dtype:value qudt:TorinoScaleValue_06 ;
  dtype:value qudt:TorinoScaleValue_07 ;
  dtype:value qudt:TorinoScaleValue_08 ;
  dtype:value qudt:TorinoScaleValue_09 ;
  dtype:value qudt:TorinoScaleValue_10 ;
  vaem:url "http://neo.jpl.nasa.gov/torino_scale.html"^^xsd:anyURI ;
.
qudt:TorinoScaleValue
  rdf:type owl:Class ;
  dc:description "The Torino Scale is a \"Richter Scale\" for categorizing the Earth impact hazard associated with newly discovered asteroids and comets. It is intended to serve as a communication tool for astronomers and the public to assess the seriousness of predictions of close encounters by asteroids and comets during the 21st century.  See \\href{http://www.google.com/url?q=http://impact.arc.nasa.gov/torino.cfm&sa=U&ei=SdYqUMOGI8_2iQLUzoGwCQ&ved=0CBUQFjAA&usg=AFQjCNHp6InNWMzdZnRgToMBqdWos84lnQ}{NASA ARC Impact Website} for more information."^^xsd:string ;
  rdfs:label "Torino scale value"^^xsd:string ;
  rdfs:subClassOf qudt:EnumeratedValue ;
  rdfs:subClassOf qudt:OrdinalScale ;
  rdfs:subClassOf [
      rdf:type owl:Restriction ;
      owl:allValuesFrom qudt:TorinoScaleZone ;
      owl:onProperty qudt:categorizedAs ;
    ] ;
  rdfs:subClassOf [
      rdf:type owl:Restriction ;
      owl:cardinality "1"^^xsd:nonNegativeInteger ;
      owl:onProperty qudt:categorizedAs ;
    ] ;
.
qudt:TorinoScaleValue_00
  rdf:type qudt:TorinoScaleValue ;
  qudt:categorizedAs qudt:TorinoScaleZone_White ;
  qudt:code "0"^^xsd:string ;
  dcterms:description "The likelihood of a collision is zero, or is so low as to be effectively zero. Also applies to small objects such as meteors and bodies that burn up in the atmosphere as well as infrequent meteorite falls that rarely cause damage."^^xsd:string ;
  qudt:literal "no-hazard-white-zone"^^xsd:string ;
  qudt:order "1"^^xsd:nonNegativeInteger ;
  rdfs:label "No Hazard (White Zone)"^^xsd:string ;
.
qudt:TorinoScaleValue_01
  rdf:type qudt:TorinoScaleValue ;
  qudt:categorizedAs qudt:TorinoScaleZone_Green ;
  qudt:code "1"^^xsd:string ;
  dcterms:description "A routine discovery in which a pass near the Earth is predicted that poses no unusual level of danger. Current calculations show the chance of collision is extremely unlikely with no cause for public attention or public concern. New telescopic observations very likely will lead to re-assignment to Level 0."^^xsd:string ;
  qudt:literal "normal-green-zone"^^xsd:string ;
  qudt:order "2"^^xsd:nonNegativeInteger ;
  rdfs:label "Normal (Green Zone)"^^xsd:string ;
.
qudt:TorinoScaleValue_02
  rdf:type qudt:TorinoScaleValue ;
  qudt:categorizedAs qudt:TorinoScaleZone_Yellow ;
  qudt:code "2"^^xsd:string ;
  dcterms:description "A discovery, which may become routine with expanded searches, of an object making a somewhat close but not highly unusual pass near the Earth. While meriting attention by astronomers, there is no cause for public attention or public concern as an actual collision is very unlikely. New telescopic observations very likely will lead to re-assignment to Level 0."^^xsd:string ;
  qudt:literal "merits-attention-yellow-zone-2"^^xsd:string ;
  qudt:order "3"^^xsd:nonNegativeInteger ;
  rdfs:label "Meriting Attention by Astronomers (Yellow Zone 2)"^^xsd:string ;
.
qudt:TorinoScaleValue_03
  rdf:type qudt:TorinoScaleValue ;
  qudt:categorizedAs qudt:TorinoScaleZone_Yellow ;
  qudt:code "3"^^xsd:string ;
  dcterms:description "A close encounter, meriting attention by astronomers. Current calculations give a 1% or greater chance of collision capable of localized destruction. Most likely, new telescopic observations will lead to re-assignment to Level 0. Attention by public and by public officials is merited if the encounter is less than a decade away."^^xsd:string ;
  qudt:literal "merits-attention-yellow-zone-3"^^xsd:string ;
  qudt:order "4"^^xsd:nonNegativeInteger ;
  rdfs:label "Meriting Attention by Astronomers (Yellow Zone 3)"^^xsd:string ;
.
qudt:TorinoScaleValue_04
  rdf:type qudt:TorinoScaleValue ;
  qudt:categorizedAs qudt:TorinoScaleZone_Yellow ;
  qudt:code "4"^^xsd:string ;
  dcterms:description "A close encounter, meriting attention by astronomers. Current calculations give a 1% or greater chance of collision capable of regional devastation. Most likely, new telescopic observations will lead to re-assignment to Level 0. Attention by public and by public officials is merited if the encounter is less than a decade away."^^xsd:string ;
  qudt:literal "merits-attention-yellow-zone-4"^^xsd:string ;
  dtype:order "5"^^xsd:nonNegativeInteger ;
  rdfs:label "Meriting Attention by Astronomers (Yellow Zone 4)"^^xsd:string ;
.
qudt:TorinoScaleValue_05
  rdf:type qudt:TorinoScaleValue ;
  qudt:categorizedAs qudt:TorinoScaleZone_Orange ;
  qudt:code "5"^^xsd:string ;
  dcterms:description "A close encounter posing a serious, but still uncertain threat of regional devastation. Critical attention by astronomers is needed to determine conclusively whether or not a collision will occur. If the encounter is less than a decade away, governmental contingency planning may be warranted."^^xsd:string ;
  qudt:literal "threatening-orange-zone-5"^^xsd:string ;
  qudt:order "6"^^xsd:nonNegativeInteger ;
  rdfs:label "Threatening (Orange Zone 5)"^^xsd:string ;
.
qudt:TorinoScaleValue_06
  rdf:type qudt:TorinoScaleValue ;
  qudt:categorizedAs qudt:TorinoScaleZone_Orange ;
  qudt:code "7"^^xsd:string ;
  dcterms:description "A close encounter by a large object posing a serious but still uncertain threat of a global catastrophe. Critical attention by astronomers is needed to determine conclusively whether or not a collision will occur. If the encounter is less than three decades away, governmental contingency planning may be warranted."^^xsd:string ;
  qudt:literal "threatening-orange-zone-6"^^xsd:string ;
  qudt:order "8"^^xsd:nonNegativeInteger ;
  rdfs:label "Threatening (Orange Zone 6)"^^xsd:string ;
.
qudt:TorinoScaleValue_07
  rdf:type qudt:TorinoScaleValue ;
  qudt:categorizedAs qudt:TorinoScaleZone_Orange ;
  qudt:code "7"^^xsd:string ;
  dcterms:description "A very close encounter by a large object, which if occurring this century, poses an unprecedented but still uncertain threat of a global catastrophe. For such a threat in this century, international contingency planning is warranted, especially to determine urgently and conclusively whether or not a collision will occur."^^xsd:string ;
  qudt:literal "threatening-orange-zone-7"^^xsd:string ;
  qudt:order "8"^^xsd:nonNegativeInteger ;
  rdfs:label "Threatening (Orange Zone 7)"^^xsd:string ;
.
qudt:TorinoScaleValue_08
  rdf:type qudt:TorinoScaleValue ;
  qudt:categorizedAs qudt:TorinoScaleZone_Red ;
  qudt:code "8"^^xsd:string ;
  dcterms:description "A collision is certain, capable of causing localized destruction for an impact over land or possibly a tsunami if close offshore. Such events occur on average between once per 50 years and once per several 1000 years."^^xsd:string ;
  qudt:literal "threatening-orange-zone-8"^^xsd:string ;
  dtype:order "9"^^xsd:nonNegativeInteger ;
  rdfs:label "Certain Collisions (Red Zone 8)"^^xsd:string ;
.
qudt:TorinoScaleValue_09
  rdf:type qudt:TorinoScaleValue ;
  qudt:categorizedAs qudt:TorinoScaleZone_Red ;
  qudt:code "9"^^xsd:string ;
  dcterms:description "A collision is certain, capable of causing unprecedented regional devastation for a land impact or the threat of a major tsunami for an ocean impact. Such events occur on average between once per 10,000 years and once per 100,000 years."^^xsd:string ;
  qudt:literal "threatening-orange-zone-9"^^xsd:string ;
  qudt:order "10"^^xsd:nonNegativeInteger ;
  rdfs:label "Certain Collisions (Red Zone 9)"^^xsd:string ;
.
qudt:TorinoScaleValue_10
  rdf:type qudt:TorinoScaleValue ;
  qudt:categorizedAs qudt:TorinoScaleZone_Red ;
  qudt:code "10"^^xsd:string ;
  dcterms:description "A collision is certain, capable of causing global climatic catastrophe that may threaten the future of civilization as we know it, whether impacting land or ocean. Such events occur on average once per 100,000 years, or less often."^^xsd:string ;
  qudt:literal "certain-collisions-red-zone"^^xsd:string ;
  qudt:order "11"^^xsd:nonNegativeInteger ;
  rdfs:label "Certain Collisions (Red Zone 10)"^^xsd:string ;
.
qudt:TorinoScaleZone
  rdf:type owl:Class ;
  dc:description "A color-code for severity in the Torino Scale."^^xsd:string ;
  rdfs:label "Torino scale zone"^^xsd:string ;
  rdfs:subClassOf qudt:EnumeratedValue ;
  owl:oneOf (
      qudt:TorinoScaleZone_White
      qudt:TorinoScaleZone_Green
      qudt:TorinoScaleZone_Yellow
      qudt:TorinoScaleZone_Orange
      qudt:TorinoScaleZone_Red
    ) ;
.
qudt:TorinoScaleZone_Green
  rdf:type qudt:TorinoScaleZone ;
  qudt:literal "green"^^xsd:string ;
  rdfs:label "Torino scale zone Green"^^xsd:string ;
.
qudt:TorinoScaleZone_Orange
  rdf:type qudt:TorinoScaleZone ;
  qudt:literal "orange"^^xsd:string ;
  rdfs:label "Torino scale zone Orange"^^xsd:string ;
.
qudt:TorinoScaleZone_Red
  rdf:type qudt:TorinoScaleZone ;
  qudt:literal "red"^^xsd:string ;
  rdfs:label "Torino scale zone Red"^^xsd:string ;
.
qudt:TorinoScaleZone_White
  rdf:type qudt:TorinoScaleZone ;
  qudt:literal "white"^^xsd:string ;
  rdfs:label "No Hazard (White Zone)"^^xsd:string ;
.
qudt:TorinoScaleZone_Yellow
  rdf:type qudt:TorinoScaleZone ;
  qudt:literal "yellow"^^xsd:string ;
  rdfs:label "Torino scale zone Yellow"^^xsd:string ;
.
voag:hasCatalogEntry
  rdf:type owl:ObjectProperty ;
  rdfs:label "has catalog entry"^^xsd:string ;
.
voag:hasLicenseType
  rdf:type owl:ObjectProperty ;
  rdfs:label "has license type"@en-US ;
.
voag:withAttributionTo
  rdf:type owl:ObjectProperty ;
  rdfs:label "with attribution to"^^xsd:string ;
.
skos:closeMatch
  rdf:type rdf:Property ;
.
skos:exactMatch
  rdf:type rdf:Property ;
.
