# baseURI: http://qudt.org/2.0/schema/qudt/science
# imports: http://qudt.org/2.1/schema/qudt
# imports: http://www.linkedmodel.org/schema/dtype
# imports: http://www.linkedmodel.org/schema/vaem
# imports: http://www.w3.org/2004/02/skos/core

@prefix dc: <http://purl.org/dc/elements/1.1/> .
@prefix dct: <http://purl.org/dc/terms/> .
@prefix dtype: <http://www.linkedmodel.org/schema/dtype#> .
@prefix owl: <http://www.w3.org/2002/07/owl#> .
@prefix prov: <http://www.w3.org/ns/prov#> .
@prefix quantitykind: <http://qudt.org/vocab/quantitykind/> .
@prefix qudt: <http://qudt.org/schema/qudt/> .
@prefix rdf: <http://www.w3.org/1999/02/22-rdf-syntax-ns#> .
@prefix rdfs: <http://www.w3.org/2000/01/rdf-schema#> .
@prefix skos: <http://www.w3.org/2004/02/skos/core#> .
@prefix unit: <http://qudt.org/vocab/unit/> .
@prefix vaem: <http://www.linkedmodel.org/schema/vaem#> .
@prefix voag: <http://voag.linkedmodel.org/schema/voag#> .
@prefix xsd: <http://www.w3.org/2001/XMLSchema#> .

dct:author
  a rdf:Property ;
  rdfs:range xsd:string ;
.
dct:contributor
  a rdf:Property ;
  rdfs:range xsd:string ;
.
dct:created
  a rdf:Property ;
  rdfs:label "created" ;
  rdfs:range xsd:date ;
.
dct:creator
  a owl:AnnotationProperty ;
  rdfs:isDefinedBy <http://qudt.org/schema/qudt> ;
  rdfs:label "creator" ;
  rdfs:range xsd:string ;
.
dct:description
  a rdf:Property ;
  a owl:AnnotationProperty ;
  rdfs:label "description" ;
  rdfs:range xsd:string ;
.
dct:modified
  a rdf:Property ;
  rdfs:label "modified" ;
  rdfs:range xsd:date ;
.
dct:rights
  a owl:AnnotationProperty ;
  rdfs:label "rights" ;
  rdfs:range xsd:string ;
.
dct:source
  a owl:AnnotationProperty ;
  rdfs:isDefinedBy dct: ;
  rdfs:label "source" ;
  rdfs:range xsd:string ;
.
dct:subject
  a owl:AnnotationProperty ;
  rdfs:label "subject" ;
  rdfs:range xsd:string ;
.
dct:title
  a owl:AnnotationProperty ;
  rdfs:label "title" ;
  rdfs:range xsd:string ;
.
<http://qudt.org/2.0/schema/qudt/science>
  a owl:Ontology ;
  vaem:hasGraphMetadata vaem:GMD_QUDT-SCHEMA-SCIENCE ;
  rdfs:label "QUDT Schema - Science - version 2.0" ;
  owl:imports <http://qudt.org/2.1/schema/qudt> ;
  owl:imports <http://www.linkedmodel.org/schema/dtype> ;
  owl:imports <http://www.linkedmodel.org/schema/vaem> ;
  owl:imports <http://www.w3.org/2004/02/skos/core> ;
  owl:versionIRI <http://qudt.org/2.1/schema/qudt> ;
.
qudt:AbsorbedDoseRateUnit
  a owl:Class ;
  dct:description "A sub-type of 'Radiology Unit'. Detailed desciption to be provided in a future version." ;
  rdfs:isDefinedBy <http://qudt.org/2.0/schema/qudt/science> ;
  rdfs:isDefinedBy qudt:science ;
  rdfs:label "Absorbed dose rate unit" ;
  rdfs:subClassOf qudt:RadiologyUnit ;
  rdfs:subClassOf [
      a owl:Restriction ;
      owl:hasValue quantitykind:AbsorbedDoseRate ;
      owl:onProperty qudt:hasQuantityKind ;
    ] ;
  owl:equivalentClass qudt:AbsorbedDoseUnit ;
.
qudt:AbsorbedDoseUnit
  a owl:Class ;
  dct:description "A sub-type of 'Radiology Unit'. Detailed desciption to be provided in a future version." ;
  rdfs:isDefinedBy <http://qudt.org/2.0/schema/qudt/science> ;
  rdfs:isDefinedBy qudt:science ;
  rdfs:label "Absorbed Dose Unit" ;
  rdfs:subClassOf qudt:RadiologyUnit ;
  rdfs:subClassOf [
      a owl:Restriction ;
      owl:hasValue quantitykind:AbsorbedDose ;
      owl:onProperty qudt:hasQuantityKind ;
    ] ;
.
qudt:AccelerationUnit
  a owl:Class ;
  dct:description "A sub-type of 'Space And Time Unit'. Detailed desciption to be provided in a future version." ;
  rdfs:isDefinedBy <http://qudt.org/2.0/schema/qudt/science> ;
  rdfs:isDefinedBy qudt:science ;
  rdfs:label "Acceleration Unit" ;
  rdfs:subClassOf qudt:SpaceAndTimeUnit ;
.
qudt:AcousticsQuantityKind
  a owl:Class ;
  dct:description "A sub-type of 'Classical Mechanics Quantity Kind'. Detailed desciption to be provided in a future version." ;
  rdfs:isDefinedBy <http://qudt.org/2.0/schema/qudt/science> ;
  rdfs:isDefinedBy qudt:science ;
  rdfs:label "Acoustics Quantity Kind" ;
  rdfs:subClassOf qudt:ClassicalMechanicsQuantityKind ;
.
qudt:AcousticsUnit
  a owl:Class ;
  qudt:description "Acoustics is the interdisciplinary science that deals with the study of all mechanical waves in gases, liquids, and solids including vibration, sound, ultrasound and infrasound."^^rdf:HTML ;
  rdfs:isDefinedBy <http://qudt.org/2.0/schema/qudt/science> ;
  rdfs:isDefinedBy qudt:science ;
  rdfs:label "Acoustics unit" ;
  rdfs:subClassOf qudt:ClassicalMechanicsUnit ;
.
qudt:ActivityUnit
  a owl:Class ;
  dct:description "A sub-type of 'Radiology Unit'. Detailed desciption to be provided in a future version." ;
  rdfs:isDefinedBy <http://qudt.org/2.0/schema/qudt/science> ;
  rdfs:isDefinedBy qudt:science ;
  rdfs:label "Activity Unit" ;
  rdfs:subClassOf qudt:RadiologyUnit ;
  rdfs:subClassOf [
      a owl:Restriction ;
      owl:hasValue quantitykind:Activity ;
      owl:onProperty qudt:hasQuantityKind ;
    ] ;
  skos:exactMatch <http://dbpedia.org/resource/Category:Units_of_radioactivity> ;
.
qudt:AeroThermalDynamicsQuantityKind
  a owl:Class ;
  dct:description "A sub-type of 'Aerodynamics Quantity Kind'. Detailed desciption to be provided in a future version." ;
  rdfs:isDefinedBy <http://qudt.org/2.0/schema/qudt/science> ;
  rdfs:isDefinedBy qudt:science ;
  rdfs:label "Aerothermal Dynamics Quantity Kind" ;
  rdfs:subClassOf qudt:AerodynamicsQuantityKind ;
.
qudt:AerodynamicsQuantityKind
  a owl:Class ;
  dct:description "Aerodynamics is a branch of dynamics concerned with the study of forces and the resulting motion of objects through the air, particularly when it interacts with a solid object. Aerodynamics is a subfield of fluid dynamics and gas dynamics, with much theory shared between them. Aerodynamics is often used synonymously with gas dynamics, with the difference being that gas dynamics applies to all gases." ;
  rdfs:isDefinedBy <http://qudt.org/2.0/schema/qudt/science> ;
  rdfs:isDefinedBy qudt:science ;
  rdfs:label "Aerodynamics Quantity Kind" ;
  rdfs:subClassOf qudt:FluidDynamicsQuantityKind ;
  prov:wasInfluencedBy <http://en.wikipedia.org/wiki/Aerodynamics> ;
  prov:wasInfluencedBy <http://www.grc.nasa.gov/WWW/K-12/airplane/short.html> ;
.
qudt:AmountOfSubstanceTemperatureUnit
  a owl:Class ;
  dct:description "A sub-type of 'Chemistry Unit'. Detailed desciption to be provided in a future version." ;
  rdfs:isDefinedBy <http://qudt.org/2.0/schema/qudt/science> ;
  rdfs:isDefinedBy qudt:science ;
  rdfs:label "Amount of substance temperature unit" ;
  rdfs:subClassOf qudt:ChemistryUnit ;
  rdfs:subClassOf [
      a owl:Restriction ;
      owl:hasValue quantitykind:TemperatureAmountOfSubstance ;
      owl:onProperty qudt:hasQuantityKind ;
    ] ;
.
qudt:AmountOfSubstanceUnit
  a owl:Class ;
  dct:description "A sub-type of 'Chemistry Unit'. Detailed desciption to be provided in a future version." ;
  rdfs:isDefinedBy <http://qudt.org/2.0/schema/qudt/science> ;
  rdfs:isDefinedBy qudt:science ;
  rdfs:label "Amount Of Substance Unit" ;
  rdfs:subClassOf qudt:ChemistryUnit ;
  rdfs:subClassOf [
      a owl:Restriction ;
      owl:hasValue quantitykind:AmountOfSubstance ;
      owl:onProperty qudt:hasQuantityKind ;
    ] ;
  skos:exactMatch <http://dbpedia.org/resource/Category:Units_of_amount_of_substance> ;
.
qudt:AngleUnit
  a owl:Class ;
  qudt:description "All units relating to specificaiton of angles. "^^rdf:HTML ;
  rdfs:isDefinedBy <http://qudt.org/2.0/schema/qudt/science> ;
  rdfs:isDefinedBy qudt:science ;
  rdfs:label "Angle unit" ;
  rdfs:subClassOf qudt:DimensionlessUnit ;
  rdfs:subClassOf qudt:SpaceAndTimeUnit ;
  rdfs:subClassOf [
      a owl:Restriction ;
      owl:hasValue quantitykind:Angle ;
      owl:onProperty qudt:hasQuantityKind ;
    ] ;
  skos:exactMatch <http://dbpedia.org/resource/Category:Units_of_angle> ;
.
qudt:AngularAccelerationUnit
  a owl:Class ;
  dct:description "A sub-type of 'Acceleration Unit'. Detailed desciption to be provided in a future version." ;
  rdfs:isDefinedBy <http://qudt.org/2.0/schema/qudt/science> ;
  rdfs:isDefinedBy qudt:science ;
  rdfs:label "Angular Acceleration Unit" ;
  rdfs:subClassOf qudt:AccelerationUnit ;
  rdfs:subClassOf [
      a owl:Restriction ;
      owl:hasValue quantitykind:AngularAcceleration ;
      owl:onProperty qudt:hasQuantityKind ;
    ] ;
.
qudt:AngularMassUnit
  a owl:Class ;
  qudt:description "The units of angular mass have dimensions of mass * area. They are used to measure the moment of inertia."^^rdf:HTML ;
  rdfs:isDefinedBy <http://qudt.org/2.0/schema/qudt/science> ;
  rdfs:isDefinedBy qudt:science ;
  rdfs:label "Angular mass unit" ;
  rdfs:subClassOf qudt:MassUnit ;
  rdfs:subClassOf [
      a owl:Restriction ;
      owl:hasValue quantitykind:MomentOfInertia ;
      owl:onProperty qudt:hasQuantityKind ;
    ] ;
.
qudt:AngularMomentumUnit
  a owl:Class ;
  dct:description "A sub-type of 'Momentum Unit'. Detailed desciption to be provided in a future version." ;
  rdfs:isDefinedBy <http://qudt.org/2.0/schema/qudt/science> ;
  rdfs:isDefinedBy qudt:science ;
  rdfs:label "Angular Momentum Unit" ;
  rdfs:subClassOf qudt:MomentumUnit ;
  rdfs:subClassOf [
      a owl:Restriction ;
      owl:hasValue quantitykind:AngularMomentum ;
      owl:onProperty qudt:hasQuantityKind ;
    ] ;
.
qudt:AngularVelocityUnit
  a owl:Class ;
  dct:description "A sub-type of 'Velocity Unit'. Detailed desciption to be provided in a future version." ;
  rdfs:isDefinedBy <http://qudt.org/2.0/schema/qudt/science> ;
  rdfs:isDefinedBy qudt:science ;
  rdfs:label "Angular Velocity Unit" ;
  rdfs:subClassOf qudt:VelocityUnit ;
  rdfs:subClassOf [
      a owl:Restriction ;
      owl:hasValue quantitykind:AngularVelocity ;
      owl:onProperty qudt:hasQuantityKind ;
    ] ;
.
qudt:AreaAngleUnit
  a owl:Class ;
  dct:description "A sub-type of 'Space And Time Unit'. Detailed desciption to be provided in a future version." ;
  rdfs:isDefinedBy <http://qudt.org/2.0/schema/qudt/science> ;
  rdfs:isDefinedBy qudt:science ;
  rdfs:label "Area Angle Unit" ;
  rdfs:subClassOf qudt:SpaceAndTimeUnit ;
  rdfs:subClassOf [
      a owl:Restriction ;
      owl:hasValue quantitykind:AreaAngle ;
      owl:onProperty qudt:hasQuantityKind ;
    ] ;
.
qudt:AreaTemperatureUnit
  a owl:Class ;
  dct:description "A sub-type of 'Thermodynamics Unit'. Detailed desciption to be provided in a future version." ;
  rdfs:isDefinedBy <http://qudt.org/2.0/schema/qudt/science> ;
  rdfs:isDefinedBy qudt:science ;
  rdfs:label "Area Temperature Unit" ;
  rdfs:subClassOf qudt:ThermodynamicsUnit ;
  rdfs:subClassOf [
      a owl:Restriction ;
      owl:hasValue quantitykind:AreaTemperature ;
      owl:onProperty qudt:hasQuantityKind ;
    ] ;
.
qudt:AreaThermalExpansionUnit
  a owl:Class ;
  qudt:description """When the temperature of a substance changes, the energy that is stored in the intermolecular bonds between atoms changes. When the stored energy increases, so does the length of the molecular bonds. As a result, solids typically expand in response to heating and contract on cooling; this dimensional response to temperature change is expressed by its coefficient of thermal expansion.



Different coefficients of thermal expansion can be defined for a substance depending on whether the expansion is measured by:



    * linear thermal expansion

    * area thermal expansion

    * volumetric thermal expansion



These characteristics are closely related. The volumetric thermal expansion coefficient can be defined for both liquids and solids. The linear thermal expansion can only be defined for solids, and is common in engineering applications.



Some substances expand when cooled, such as freezing water, so they have negative thermal expansion coefficients.



For exactly isotropic materials, the area thermal expansion coefficient is very closely approximated as twice the linear coefficient."""^^rdf:HTML ;
  rdfs:isDefinedBy <http://qudt.org/2.0/schema/qudt/science> ;
  rdfs:isDefinedBy qudt:science ;
  rdfs:label "Area Thermal Expansion Unit" ;
  rdfs:subClassOf qudt:ThermalExpansionUnit ;
  rdfs:subClassOf [
      a owl:Restriction ;
      owl:hasValue quantitykind:AreaThermalExpansion ;
      owl:onProperty qudt:hasQuantityKind ;
    ] ;
.
qudt:AreaTimeTemperatureUnit
  a owl:Class ;
  dct:description "A sub-type of 'Thermodynamics Unit'. Detailed desciption to be provided in a future version." ;
  rdfs:isDefinedBy <http://qudt.org/2.0/schema/qudt/science> ;
  rdfs:isDefinedBy qudt:science ;
  rdfs:label "Area Time Temperature Unit" ;
  rdfs:subClassOf qudt:ThermodynamicsUnit ;
  rdfs:subClassOf [
      a owl:Restriction ;
      owl:hasValue quantitykind:AreaTimeTemperature ;
      owl:onProperty qudt:hasQuantityKind ;
    ] ;
.
qudt:AreaUnit
  a owl:Class ;
  dct:description "A sub-type of 'Space And Time Unit'. Detailed desciption to be provided in a future version." ;
  rdfs:isDefinedBy <http://qudt.org/2.0/schema/qudt/science> ;
  rdfs:isDefinedBy qudt:science ;
  rdfs:label "Area Unit" ;
  rdfs:subClassOf qudt:SpaceAndTimeUnit ;
  rdfs:subClassOf [
      a owl:Restriction ;
      owl:hasValue quantitykind:Area ;
      owl:onProperty qudt:hasQuantityKind ;
    ] ;
  skos:exactMatch <http://dbpedia.org/resource/Category:Units_of_area> ;
.
qudt:ArtificalGravityQuantityKind
  a owl:Class ;
  dct:description "A sub-type of 'Structures And Mechanics Quantity Kind'. Detailed desciption to be provided in a future version." ;
  rdfs:isDefinedBy <http://qudt.org/2.0/schema/qudt/science> ;
  rdfs:isDefinedBy qudt:science ;
  rdfs:label "Artifical Gravity Quantity Kind" ;
  rdfs:subClassOf qudt:StructuresAndMechanicsQuantityKind ;
.
qudt:AstrionicsQuantityKind
  a owl:Class ;
  dct:description "A sub-type of 'Space System Engineering Quantity Kind'. Detailed desciption to be provided in a future version." ;
  rdfs:isDefinedBy <http://qudt.org/2.0/schema/qudt/science> ;
  rdfs:isDefinedBy qudt:science ;
  rdfs:label "Astrionics Quantity Kind" ;
  rdfs:subClassOf qudt:SpaceSystemEngineeringQuantityKind ;
  skos:definition "Astrionics is the science and technology of the development and application of electronic systems, sub-systems, and components used in spacecraft. The electronic systems on board a spacecraft include attitude determination and control, communications, command and telemetry, and computer systems. Sensors refers to the electronic components on board a spacecraft. For engineers one of the most important considerations that must be made in the design process is the environment in which the spacecraft systems and components must operate and endure. The challenges of designing systems and components for the space environment include more than the fact that space is a vacuum." ;
.
qudt:AstrobiologyQuantityKind
  a owl:Class ;
  dct:description "A sub-type of 'Biology'. Detailed desciption to be provided in a future version." ;
  rdfs:isDefinedBy <http://qudt.org/2.0/schema/qudt/science> ;
  rdfs:isDefinedBy qudt:science ;
  rdfs:label "Astrobiology Quantity Kind" ;
  rdfs:subClassOf qudt:BiologyQuantityKind ;
.
qudt:AstrodynamicsQuantityKind
  a owl:Class ;
  dct:description "A sub-type of 'Classical Mechanics Quantity Kind'. Detailed desciption to be provided in a future version." ;
  rdfs:isDefinedBy <http://qudt.org/2.0/schema/qudt/science> ;
  rdfs:isDefinedBy qudt:science ;
  rdfs:label "Astrodynamics Quantity Kind" ;
  rdfs:subClassOf qudt:ClassicalMechanicsQuantityKind ;
.
qudt:AstrodynamicsUnit
  a owl:Class ;
  dct:description "A sub-type of 'Classical Mechanics Unit'. Detailed desciption to be provided in a future version." ;
  rdfs:isDefinedBy <http://qudt.org/2.0/schema/qudt/science> ;
  rdfs:isDefinedBy qudt:science ;
  rdfs:label "Astrodynamics unit" ;
  rdfs:subClassOf qudt:ClassicalMechanicsUnit ;
.
qudt:AtmosphericChemistryQuantityKind
  a owl:Class ;
  dct:description "Atmospheric chemistry is a branch of atmospheric science in which the chemistry of the Earth's atmosphere and that of other planets is studied. It is a multidisciplinary field of research and draws on environmental chemistry, physics, meteorology, computer modeling, oceanography, geology and volcanology and other disciplines. Research is increasingly connected with other areas of study such as climatology." ;
  rdfs:isDefinedBy <http://qudt.org/2.0/schema/qudt/science> ;
  rdfs:isDefinedBy qudt:science ;
  rdfs:label "Atmospheric chemistry quantity kind" ;
  rdfs:subClassOf qudt:AtmosphericScienceQuantityKind ;
  prov:wasInfluencedBy <http://en.wikipedia.org/wiki/Atmospheric_chemistry> ;
.
qudt:AtmosphericPhysicsQuantityKind
  a owl:Class ;
  dct:description "Atmospheric physics is the application of physics to the study of the atmosphere. Atmospheric physicists attempt to model Earth's atmosphere and the atmospheres of the other planets using fluid flow equations, chemical models, radiation balancing, and energy transfer processes in the atmosphere (as well as how these tie in to other systems such as the oceans). In order to model weather systems, atmospheric physicists employ elements of scattering theory, wave propagation models, cloud physics, statistical mechanics and spatial statistics which are highly mathematical and related to physics. It has close links to meteorology and climatology and also covers the design and construction of instruments for studying the atmosphere and the interpretation of the data they provide, including remote sensing instruments. At the dawn of the space age and the introduction of sounding rockets, aeronomy became a subdiscipline concerning the upper layers of the atmosphere, where dissociation and ionization are important." ;
  rdfs:isDefinedBy <http://qudt.org/2.0/schema/qudt/science> ;
  rdfs:isDefinedBy qudt:science ;
  rdfs:label "Atmospheric Physics Quantity Kind" ;
  rdfs:subClassOf qudt:AtmosphericScienceQuantityKind ;
  prov:wasInfluencedBy <http://en.wikipedia.org/wiki/Atmospheric_physics> ;
.
qudt:AtmosphericScienceQuantityKind
  a owl:Class ;
  dct:description "A sub-type of 'Science quantity kind'. Detailed desciption to be provided in a future version." ;
  rdfs:isDefinedBy <http://qudt.org/2.0/schema/qudt/science> ;
  rdfs:isDefinedBy qudt:science ;
  rdfs:label "Atmospheric Science Quantity Kind" ;
  rdfs:subClassOf qudt:ScienceQuantityKind ;
.
qudt:AtomicChargeUnit
  a owl:Class ;
  dct:description "A sub-type of 'Atomic unit'. Detailed desciption to be provided in a future version." ;
  rdfs:isDefinedBy <http://qudt.org/2.0/schema/qudt/science> ;
  rdfs:isDefinedBy qudt:science ;
  rdfs:label "Atomic charge unit" ;
  rdfs:subClassOf qudt:AtomicUnit ;
  rdfs:subClassOf [
      a owl:Restriction ;
      owl:hasValue quantitykind:AtomicCharge ;
      owl:onProperty qudt:hasQuantityKind ;
    ] ;
.
qudt:AtomicMassUnit
  a owl:Class ;
  dct:description "A sub-type of 'Atomic unit'. Detailed desciption to be provided in a future version." ;
  rdfs:isDefinedBy <http://qudt.org/2.0/schema/qudt/science> ;
  rdfs:isDefinedBy qudt:science ;
  rdfs:label "Atomic mass unit" ;
  rdfs:subClassOf qudt:AtomicUnit ;
.
qudt:AtomicPhysicsQuantityKind
  a owl:Class ;
  dct:description "A sub-type of 'Physics Quantity Kind'. Detailed desciption to be provided in a future version." ;
  rdfs:isDefinedBy <http://qudt.org/2.0/schema/qudt/science> ;
  rdfs:isDefinedBy qudt:science ;
  rdfs:label "Atomic Physics" ;
  rdfs:subClassOf qudt:PhysicsQuantityKind ;
.
qudt:AtomicUnit
  a owl:Class ;
  dct:description "A sub-type of 'Physics Unit'. Detailed desciption to be provided in a future version." ;
  qudt:fieldCode "710" ;
  rdfs:isDefinedBy <http://qudt.org/2.0/schema/qudt/science> ;
  rdfs:isDefinedBy qudt:science ;
  rdfs:label "Atomic unit" ;
  rdfs:subClassOf qudt:PhysicsUnit ;
  rdfs:subClassOf [
      a owl:Restriction ;
      owl:allValuesFrom qudt:AtomicPhysicsQuantityKind ;
      owl:onProperty qudt:hasQuantityKind ;
    ] ;
  owl:equivalentClass [
      a owl:Restriction ;
      owl:allValuesFrom qudt:AtomicPhysicsQuantityKind ;
      owl:onProperty qudt:hasQuantityKind ;
    ] ;
.
qudt:AttitudeControlQuantityKind
  a owl:Class ;
  dct:description "A sub-type of 'Astrionics Quantity Kind'. Detailed desciption to be provided in a future version." ;
  rdfs:isDefinedBy <http://qudt.org/2.0/schema/qudt/science> ;
  rdfs:isDefinedBy qudt:science ;
  rdfs:label "Attitude Control Quantity Kind" ;
  rdfs:subClassOf qudt:AstrionicsQuantityKind ;
.
qudt:AvionicsQuantityKind
  a owl:Class ;
  dct:description "A sub-type of 'Space System Engineering Quantity Kind'. Detailed desciption to be provided in a future version." ;
  rdfs:isDefinedBy <http://qudt.org/2.0/schema/qudt/science> ;
  rdfs:isDefinedBy qudt:science ;
  rdfs:label "Avionics Quantity Kind" ;
  rdfs:subClassOf qudt:SpaceSystemEngineeringQuantityKind ;
.
qudt:BaseUnit
  rdfs:isDefinedBy <http://qudt.org/schema/qudt> ;
.
qudt:BendingMomentOrTorqueUnit
  a owl:Class ;
  dct:description "A sub-type of 'Force Unit'. Detailed desciption to be provided in a future version." ;
  rdfs:isDefinedBy <http://qudt.org/2.0/schema/qudt/science> ;
  rdfs:isDefinedBy qudt:science ;
  rdfs:label "Bending Moment Or Torque Unit" ;
  rdfs:subClassOf qudt:ForceUnit ;
  rdfs:subClassOf [
      a owl:Restriction ;
      owl:hasValue quantitykind:LengthByForce ;
      owl:onProperty qudt:hasQuantityKind ;
    ] ;
  skos:exactMatch <http://dbpedia.org/resource/Category:Units_of_torque> ;
.
qudt:BinaryPrefixUnit
  rdfs:isDefinedBy <http://qudt.org/schema/qudt> ;
.
qudt:BioChemistryQuantityKind
  a owl:Class ;
  dct:description "A sub-type of 'Life Sciences Quantity Kind'. Detailed desciption to be provided in a future version." ;
  rdfs:isDefinedBy <http://qudt.org/2.0/schema/qudt/science> ;
  rdfs:isDefinedBy qudt:science ;
  rdfs:label "Bio chemistry quantity kind" ;
  rdfs:subClassOf qudt:LifeSciencesQuantityKind ;
.
qudt:BioInformaticsQuantityKind
  a owl:Class ;
  dct:description "A sub-type of 'Infomatics quantity kind'. Detailed desciption to be provided in a future version." ;
  rdfs:isDefinedBy <http://qudt.org/2.0/schema/qudt/science> ;
  rdfs:isDefinedBy qudt:science ;
  rdfs:label "Bio informatics Quantity Kind" ;
  rdfs:subClassOf qudt:InformaticsQuantityKind ;
.
qudt:BiologyQuantityKind
  a owl:Class ;
  dct:description "A sub-type of 'Science quantity kind'. Detailed desciption to be provided in a future version." ;
  rdfs:isDefinedBy <http://qudt.org/2.0/schema/qudt/science> ;
  rdfs:isDefinedBy qudt:science ;
  rdfs:label "Biology" ;
  rdfs:subClassOf qudt:ScienceQuantityKind ;
.
qudt:BiologyUnit
  a owl:Class ;
  dct:description "A sub-type of 'Science unit'. Detailed desciption to be provided in a future version." ;
  qudt:fieldCode "300" ;
  rdfs:isDefinedBy <http://qudt.org/2.0/schema/qudt/science> ;
  rdfs:isDefinedBy qudt:science ;
  rdfs:label "Biology unit" ;
  rdfs:subClassOf qudt:ScienceUnit ;
  skos:prefLabel "Biology unit" ;
.
qudt:BiomechanicsQuantityKind
  a owl:Class ;
  dct:description "A sub-type of 'Classical Mechanics Quantity Kind'. Detailed desciption to be provided in a future version." ;
  rdfs:isDefinedBy <http://qudt.org/2.0/schema/qudt/science> ;
  rdfs:isDefinedBy qudt:science ;
  rdfs:label "Biomechanics Quantity Kind" ;
  rdfs:subClassOf qudt:ClassicalMechanicsQuantityKind ;
.
qudt:BiomechanicsUnit
  a owl:Class ;
  dct:description "A sub-type of 'Classical Mechanics Unit'. Detailed desciption to be provided in a future version." ;
  rdfs:isDefinedBy <http://qudt.org/2.0/schema/qudt/science> ;
  rdfs:isDefinedBy qudt:science ;
  rdfs:label "Biomechanics unit" ;
  rdfs:subClassOf qudt:ClassicalMechanicsUnit ;
.
qudt:BiomedicalUnit
  a owl:Class ;
  dct:description "A sub-type of 'Science unit'. Detailed desciption to be provided in a future version." ;
  qudt:fieldCode "360" ;
  rdfs:isDefinedBy <http://qudt.org/2.0/schema/qudt/science> ;
  rdfs:isDefinedBy qudt:science ;
  rdfs:label "Biomedical Unit" ;
  rdfs:subClassOf qudt:ScienceUnit ;
.
qudt:CapacitanceUnit
  a owl:Class ;
  qudt:description "Capacitance is a measure of the amount of electric charge stored (or separated) for a given electric potential."^^rdf:HTML ;
  rdfs:isDefinedBy <http://qudt.org/2.0/schema/qudt/science> ;
  rdfs:isDefinedBy qudt:science ;
  rdfs:label "Capacitance Unit" ;
  rdfs:subClassOf qudt:ElectricityAndMagnetismUnit ;
  rdfs:subClassOf [
      a owl:Restriction ;
      owl:hasValue quantitykind:Capacitance ;
      owl:onProperty qudt:hasQuantityKind ;
    ] ;
  skos:exactMatch <http://dbpedia.org/resource/Category:Units_of_electrical_capacitance> ;
.
qudt:CatalyticActivityUnit
  a owl:Class ;
  dct:description "A sub-type of 'Chemistry Unit'. Detailed desciption to be provided in a future version." ;
  rdfs:isDefinedBy <http://qudt.org/2.0/schema/qudt/science> ;
  rdfs:isDefinedBy qudt:science ;
  rdfs:label "Catalytic Activity Unit" ;
  rdfs:subClassOf qudt:ChemistryUnit ;
  rdfs:subClassOf [
      a owl:Restriction ;
      owl:hasValue quantitykind:CatalyticActivity ;
      owl:onProperty qudt:hasQuantityKind ;
    ] ;
  skos:exactMatch <http://dbpedia.org/resource/Category:Units_of_catalytic_activity> ;
.
qudt:CelestialMechanicsQuantityKind
  a owl:Class ;
  dct:description "A sub-type of 'Classical Mechanics Quantity Kind'. Detailed desciption to be provided in a future version." ;
  dct:description "The branch of astronomy that calculates the orbits of celestial bodies and their gravitational attractions, and the orbits of artificial satellites and space probes. A spacecraft approaching a planet can use radio science to measure its own acceleration caused by the planet's gravity. This can be translated into a measurement of the planet's mass and, if images are available, its density." ;
  rdfs:isDefinedBy <http://qudt.org/2.0/schema/qudt/science> ;
  rdfs:isDefinedBy qudt:science ;
  rdfs:label "Celestial Mechanics Quantity Kind" ;
  rdfs:subClassOf qudt:ClassicalMechanicsQuantityKind ;
  prov:wasInfluencedBy <http://www.oxfordreference.com/view/10.1093/acref/9780192806314.001.0001/acref-9780192806314-e-298> ;
  prov:wasInfluencedBy <http://www.oxfordreference.com/view/10.1093/acref/9780199765324.001.0001/acref-9780199765324-e-0341> ;
.
qudt:CelestialMechanicsUnit
  a owl:Class ;
  dct:description "A sub-type of 'Classical Mechanics Unit'. Detailed desciption to be provided in a future version." ;
  rdfs:isDefinedBy <http://qudt.org/2.0/schema/qudt/science> ;
  rdfs:isDefinedBy qudt:science ;
  rdfs:label "Celestial mechanics unit" ;
  rdfs:subClassOf qudt:ClassicalMechanicsUnit ;
.
qudt:CharacteristicNumber
  a owl:Class ;
  qudt:description """<p class=\"lm-para\"><b>Characteristic Numbers</b> are quantities of dimension one. Hence the coherent unit of all characteristic numbers is the number one, symbol \\(1\\). For example, characteristic numbers are used in fluid dynamics to describe an aspect of the flow. Other examples are:</p>
<ul>
<li>\\(\\textit{Biot Number}\\),</li>
<li>\\(\\textit{Damköhler number}\\),</li>
<li>\\(\\textit{Euler Number}\\),</li>
<li>\\(\\textit{Froude Number}\\),</li>
<li>\\(\\textit{Grashof Number}\\),</li>
<li>\\(\\textit{Knudsen Number}\\),</li>
<li>\\(\\textit{Mach Number}\\),</li>
<li>\\(\\textit{Nusselt Number}\\),</li>
<li>\\(\\textit{Péclet Number}\\),</li>
<li>\\(\\textit{Prandtl Number}\\),</li>
<li>\\(\\textit{Rayleigh Number}\\),</li>
<li>\\(\\textit{Reynolds Number}\\),</li>
<li>\\(\\textit{Schmidt Number}\\),</li>
<li>\\(\\textit{Sherwood Number}\\),</li>
<li>\\(\\textit{Stanton Number}\\),</li>
<li>\\(\\textit{Strouhal Number}\\), and </li>
<li>\\(\\textit{Weber}\\).</li>
</ul>"""^^rdf:HTML ;
  rdfs:isDefinedBy <http://qudt.org/2.0/schema/qudt/science> ;
  rdfs:isDefinedBy qudt:science ;
  rdfs:label "Characteristic Number" ;
  rdfs:subClassOf qudt:Quantity ;
  skos:prefLabel "Characteristic Number" ;
  prov:wasInfluencedBy <http://en.wikipedia.org/wiki/Characteristic_number_(fluid_dynamics)> ;
  prov:wasInfluencedBy <https://en.wikipedia.org/wiki/Damköhler_numbers> ;
  prov:wasInfluencedBy <https://en.wikipedia.org/wiki/Nusselt_number> ;
  prov:wasInfluencedBy <https://en.wikipedia.org/wiki/P%C3%A9clet_number> ;
.
qudt:ChemicalEngineeringQuantityKind
  a owl:Class ;
  dct:description "A sub-type of 'Engineering quantity kind'. Detailed desciption to be provided in a future version." ;
  rdfs:isDefinedBy <http://qudt.org/2.0/schema/qudt/science> ;
  rdfs:isDefinedBy qudt:science ;
  rdfs:label "Chemical Engineering Quantity Kind" ;
  rdfs:subClassOf qudt:EngineeringQuantityKind ;
.
qudt:ChemistryQuantityKind
  a owl:Class ;
  dct:description "A sub-type of 'Science quantity kind'. Detailed desciption to be provided in a future version." ;
  rdfs:isDefinedBy <http://qudt.org/2.0/schema/qudt/science> ;
  rdfs:isDefinedBy qudt:science ;
  rdfs:label "Chemistry Quantity Kind" ;
  rdfs:subClassOf qudt:ScienceQuantityKind ;
  skos:exactMatch <http://dbpedia.org/resource/Chemistry> ;
.
qudt:ChemistryUnit
  a owl:Class ;
  dct:description "A sub-type of 'Science unit'. Detailed desciption to be provided in a future version." ;
  qudt:fieldCode "400" ;
  rdfs:isDefinedBy <http://qudt.org/2.0/schema/qudt/science> ;
  rdfs:isDefinedBy qudt:science ;
  rdfs:label "Chemistry Unit"@us ;
  rdfs:subClassOf qudt:ScienceUnit ;
  rdfs:subClassOf [
      a owl:Restriction ;
      owl:allValuesFrom qudt:ChemistryQuantityKind ;
      owl:onProperty qudt:hasQuantityKind ;
    ] ;
  owl:equivalentClass [
      a owl:Restriction ;
      owl:allValuesFrom qudt:ChemistryQuantityKind ;
      owl:onProperty qudt:hasQuantityKind ;
    ] ;
  skos:prefLabel "Chemistry Unit" ;
.
qudt:ClassicalMechanicsQuantityKind
  a owl:Class ;
  dct:description "A sub-type of 'Mechanics Quantity Kind'. Detailed desciption to be provided in a future version." ;
  rdfs:isDefinedBy <http://qudt.org/2.0/schema/qudt/science> ;
  rdfs:isDefinedBy qudt:science ;
  rdfs:label "Classical Mechanics Quantity Kind" ;
  rdfs:subClassOf qudt:MechanicsQuantityKind ;
.
qudt:ClassicalMechanicsUnit
  a owl:Class ;
  dct:description "A sub-type of 'Mechanics Unit'. Detailed desciption to be provided in a future version." ;
  rdfs:isDefinedBy <http://qudt.org/2.0/schema/qudt/science> ;
  rdfs:isDefinedBy qudt:science ;
  rdfs:label "Classical Mechanics Unit" ;
  rdfs:subClassOf qudt:MechanicsUnit ;
.
qudt:ClimatologyQuantityKind
  a owl:Class ;
  dct:description "A sub-type of 'Atmospheric Science Quantity Kind'. Detailed desciption to be provided in a future version." ;
  dct:description "Climatology is the study of climate, scientifically defined as weather conditions averaged over a period of time.Traditionally it is regarded as a branch of the atmospheric sciences." ;
  rdfs:isDefinedBy <http://qudt.org/2.0/schema/qudt/science> ;
  rdfs:isDefinedBy qudt:science ;
  rdfs:label "Climatology Quantity Kind" ;
  rdfs:subClassOf qudt:AtmosphericScienceQuantityKind ;
  prov:wasInfluencedBy <http://en.wikipedia.org/wiki/Climatology> ;
.
qudt:CoefficientOfHeatTransferUnit
  a owl:Class ;
  dct:description "A sub-type of 'Thermodynamics Unit'. Detailed desciption to be provided in a future version." ;
  rdfs:isDefinedBy <http://qudt.org/2.0/schema/qudt/science> ;
  rdfs:isDefinedBy qudt:science ;
  rdfs:label "Coefficient Of Heat Transfer Unit" ;
  rdfs:subClassOf qudt:ThermodynamicsUnit ;
  rdfs:subClassOf [
      a owl:Restriction ;
      owl:hasValue quantitykind:CoefficientOfHeatTransfer ;
      owl:onProperty qudt:hasQuantityKind ;
    ] ;
.
qudt:CommunicationsQuantityKind
  a owl:Class ;
  dct:description "A sub-type of 'Engineering quantity kind'. Detailed desciption to be provided in a future version." ;
  rdfs:isDefinedBy <http://qudt.org/2.0/schema/qudt/science> ;
  rdfs:isDefinedBy qudt:science ;
  rdfs:label "Communications Quantity Kind" ;
  rdfs:subClassOf qudt:EngineeringQuantityKind ;
  skos:exactMatch <http://dbpedia.org/resource/Communication> ;
.
qudt:CommunicationsUnit
  rdfs:isDefinedBy <http://qudt.org/schema/qudt> ;
.
qudt:ComputerScienceQuantityKind
  a owl:Class ;
  dct:description "A sub-type of 'Science quantity kind'. Detailed desciption to be provided in a future version." ;
  rdfs:isDefinedBy <http://qudt.org/2.0/schema/qudt/science> ;
  rdfs:isDefinedBy qudt:science ;
  rdfs:label "Computer Science Quantity Kind" ;
  rdfs:subClassOf qudt:ScienceQuantityKind ;
.
qudt:ComputingUnit
  rdfs:isDefinedBy <http://qudt.org/schema/qudt> ;
.
qudt:ConcentrationUnit
  a owl:Class ;
  dct:description "A sub-type of 'Chemistry Unit'. Detailed desciption to be provided in a future version." ;
  rdfs:isDefinedBy <http://qudt.org/2.0/schema/qudt/science> ;
  rdfs:isDefinedBy qudt:science ;
  rdfs:label "Concentration Unit" ;
  rdfs:subClassOf qudt:ChemistryUnit ;
  rdfs:subClassOf [
      a owl:Restriction ;
      owl:hasValue quantitykind:AmountOfSubstancePerUnitVolume ;
      owl:onProperty qudt:hasQuantityKind ;
    ] ;
.
qudt:Concept
  dct:description "A sub-type of 'Thing'. Detailed desciption to be provided in a future version." ;
.
qudt:ConductanceUnit
  a owl:Class ;
  qudt:description "Electrical conductance is the inverse of electrical resistance. It measures the ease with which electricity flows along a path through an electrical element."^^rdf:HTML ;
  rdfs:isDefinedBy <http://qudt.org/2.0/schema/qudt/science> ;
  rdfs:isDefinedBy qudt:science ;
  rdfs:label "Conductance Unit" ;
  rdfs:subClassOf qudt:ElectricityAndMagnetismUnit ;
  rdfs:subClassOf [
      a owl:Restriction ;
      owl:hasValue quantitykind:ElectricConductivity ;
      owl:onProperty qudt:hasQuantityKind ;
    ] ;
  skos:exactMatch <http://dbpedia.org/resource/Category:Units_of_electrical_conductance> ;
.
qudt:ConfigurationManagementQuantityKind
  a owl:Class ;
  dct:description "A sub-type of 'System Engineering Quantity Kind'. Detailed desciption to be provided in a future version." ;
  rdfs:isDefinedBy <http://qudt.org/2.0/schema/qudt/science> ;
  rdfs:isDefinedBy qudt:science ;
  rdfs:label "Configuration Management Quantity Kind" ;
  rdfs:subClassOf qudt:SystemEngineeringQuantityKind ;
.
qudt:ConstantValue
  a owl:Class ;
  rdfs:label "Constant value" ;
.
qudt:ContinuumMechanicsQuantityKind
  a owl:Class ;
  dct:description "A sub-type of 'Mechanics Quantity Kind'. Detailed desciption to be provided in a future version." ;
  rdfs:isDefinedBy <http://qudt.org/2.0/schema/qudt/science> ;
  rdfs:isDefinedBy qudt:science ;
  rdfs:label "Continuum Mechanics Quantity Kind" ;
  rdfs:subClassOf qudt:MechanicsQuantityKind ;
.
qudt:ControlEngineeringQuantityKind
  a owl:Class ;
  dct:description "A sub-type of 'Engineering quantity kind'. Detailed desciption to be provided in a future version." ;
  rdfs:isDefinedBy <http://qudt.org/2.0/schema/qudt/science> ;
  rdfs:isDefinedBy qudt:science ;
  rdfs:label "Control Engineering Quantity Kind" ;
  rdfs:subClassOf qudt:EngineeringQuantityKind ;
.
qudt:CostEstimationQuantityKind
  a owl:Class ;
  dct:description "A sub-type of 'Finance Quantity Kind'. Detailed desciption to be provided in a future version." ;
  rdfs:isDefinedBy <http://qudt.org/2.0/schema/qudt/science> ;
  rdfs:isDefinedBy qudt:science ;
  rdfs:label "Cost estimation" ;
  rdfs:subClassOf qudt:FinanceQuantityKind ;
.
qudt:CountingUnit
  a owl:Class ;
  qudt:description "All units about counts. Examples are Atomic Number, Number, Number per Year, Percent and Sample per Second."^^rdf:HTML ;
  rdfs:isDefinedBy <http://qudt.org/2.0/schema/qudt/science> ;
  rdfs:isDefinedBy qudt:science ;
  rdfs:label "Counting Unit" ;
  rdfs:subClassOf qudt:DimensionlessUnit ;
  rdfs:subClassOf qudt:ResourceUnit ;
  skos:closeMatch <http://dbpedia.org/resource/Category:Units_of_amount> ;
.
qudt:CryogenicsQuantityKind
  a owl:Class ;
  dct:description "A sub-type of 'Physics Quantity Kind'. Detailed desciption to be provided in a future version." ;
  rdfs:isDefinedBy <http://qudt.org/2.0/schema/qudt/science> ;
  rdfs:isDefinedBy qudt:science ;
  rdfs:label "Cryogenics Quantity Kind" ;
  rdfs:subClassOf qudt:PhysicsQuantityKind ;
.
qudt:CurrencyQuantityKind
  a owl:Class ;
  dct:description "A sub-type of 'Finance Quantity Kind'. Detailed desciption to be provided in a future version." ;
  rdfs:isDefinedBy <http://qudt.org/2.0/schema/qudt/science> ;
  rdfs:isDefinedBy qudt:science ;
  rdfs:label "Currency Quantity Kind" ;
  rdfs:subClassOf qudt:FinanceQuantityKind ;
.
qudt:CurrencyUnit
  rdfs:isDefinedBy <http://qudt.org/schema/qudt> ;
  rdfs:subClassOf [
      a owl:Restriction ;
      owl:hasValue quantitykind:Currency ;
      owl:onProperty qudt:hasQuantityKind ;
    ] ;
.
qudt:CurrentPerAngleUnit
  a owl:Class ;
  dct:description "A sub-type of 'Electricity And Magnetism Unit'. Detailed desciption to be provided in a future version." ;
  rdfs:isDefinedBy <http://qudt.org/2.0/schema/qudt/science> ;
  rdfs:isDefinedBy qudt:science ;
  rdfs:label "Current Per Angle Unit" ;
  rdfs:subClassOf qudt:ElectricityAndMagnetismUnit ;
  rdfs:subClassOf [
      a owl:Restriction ;
      owl:hasValue quantitykind:ElectricCurrentPerAngle ;
      owl:onProperty qudt:hasQuantityKind ;
    ] ;
.
qudt:CurvatureUnit
  a owl:Class ;
  qudt:description """<p class=\"lm-para\">The canonical example of extrinsic curvature is that of a circle, which has curvature equal to the inverse of its radius everywhere. Smaller circles bend more sharply, and hence have higher curvature. The curvature of a smooth curve is defined as the curvature of its osculating circle at each point.</p>
<p class=\"lm-para\">The osculating circle of a sufficiently smooth plane curve at a given point on the curve is the circle whose center lies on the inner normal line and whose curvature is the same as that of the given curve at that point. This circle is tangent to the curve at the given point.  That is, given a point P on a smooth curve C, the curvature of C at P is defined to be \\(1/R\\) where \\(R\\) is the radius of the osculating circle of \\(C\\) at \\(P\\). The magnitude of curvature at points on physical curves can be measured in diopters (also spelled \"dioptre\"), a convention in optics.</p>"""^^rdf:HTML ;
  rdfs:isDefinedBy <http://qudt.org/2.0/schema/qudt/science> ;
  rdfs:isDefinedBy qudt:science ;
  rdfs:label "Curvature Unit" ;
  rdfs:subClassOf qudt:SpaceAndTimeUnit ;
.
qudt:DataRateUnit
  a owl:Class ;
  dct:description "A sub-type of 'Informatics Unit' and 'Resource Unit'. Detailed desciption to be provided in a future version." ;
  rdfs:isDefinedBy <http://qudt.org/2.0/schema/qudt/science> ;
  rdfs:isDefinedBy qudt:science ;
  rdfs:label "Data Rate Unit" ;
  rdfs:subClassOf qudt:InformaticsUnit ;
  rdfs:subClassOf qudt:ResourceUnit ;
  rdfs:subClassOf [
      a owl:Restriction ;
      owl:hasValue quantitykind:DataRate ;
      owl:onProperty qudt:hasQuantityKind ;
    ] ;
.
qudt:DecimalPrefixUnit
  rdfs:isDefinedBy <http://qudt.org/schema/qudt> ;
.
qudt:DecimalScaledUnit
  dct:description "A sub-type of 'Scaled unit'. Detailed desciption to be provided in a future version." ;
.
qudt:DerivedCoherentUnit
  dct:description "A sub-type of 'Derived Unit'. Detailed desciption to be provided in a future version." ;
.
qudt:DerivedNonCoherentUnit
  dct:description "A sub-type of 'Derived Unit'. Detailed desciption to be provided in a future version." ;
.
qudt:DerivedUnit
  rdfs:isDefinedBy <http://qudt.org/schema/qudt> ;
.
qudt:DimensionlessConcentrationUnit
  a owl:Class ;
  dct:description "A sub-type of 'Dimensionless Unit'. Detailed desciption to be provided in a future version." ;
  rdfs:isDefinedBy <http://qudt.org/2.0/schema/qudt/science> ;
  rdfs:isDefinedBy qudt:science ;
  rdfs:label "Dimensionless concentration unit" ;
  rdfs:subClassOf qudt:DimensionlessUnit ;
.
qudt:DimensionlessQuantityKind
  a owl:Class ;
  dct:description "A \"Dimensionless\" Quantity is simply a numeric value that  is typically a count or a ratio. Dimensionless quantities are often defined as products or ratios of quantities that are not dimensionless, but whose dimensions cancel out when their powers are multiplied." ;
  dct:description "A sub-type of 'Quantity Kind'. Detailed desciption to be provided in a future version." ;
  rdfs:isDefinedBy <http://qudt.org/2.0/schema/qudt/science> ;
  rdfs:isDefinedBy qudt:science ;
  rdfs:label "Dimensionless Quantity Kind" ;
  rdfs:subClassOf qudt:QuantityKind ;
.
qudt:DimensionlessUnit
  rdfs:isDefinedBy <http://qudt.org/schema/qudt> ;
  rdfs:subClassOf [
      a owl:Restriction ;
      owl:hasValue quantitykind:Dimensionless ;
      owl:onProperty qudt:hasQuantityKind ;
    ] ;
  rdfs:subClassOf [
      a owl:Restriction ;
      owl:hasValue quantitykind:Dimensionless ;
      owl:onProperty qudt:hasQuantityKind ;
    ] ;
.
qudt:DoseEquivalentUnit
  a owl:Class ;
  dct:description "A sub-type of 'Radiology Unit'. Detailed desciption to be provided in a future version." ;
  rdfs:isDefinedBy <http://qudt.org/2.0/schema/qudt/science> ;
  rdfs:isDefinedBy qudt:science ;
  rdfs:label "Dose Equivalent Unit" ;
  rdfs:subClassOf qudt:RadiologyUnit ;
  rdfs:subClassOf [
      a owl:Restriction ;
      owl:hasValue quantitykind:DoseEquivalent ;
      owl:onProperty qudt:hasQuantityKind ;
    ] ;
.
qudt:DynamicViscosityUnit
  a owl:Class ;
  dct:description "A sub-type of 'Viscosity Units'. Detailed desciption to be provided in a future version." ;
  rdfs:isDefinedBy <http://qudt.org/2.0/schema/qudt/science> ;
  rdfs:isDefinedBy qudt:science ;
  rdfs:label "Dynamic Viscosity Units" ;
  rdfs:subClassOf qudt:ViscosityUnit ;
  rdfs:subClassOf [
      a owl:Restriction ;
      owl:hasValue quantitykind:DynamicViscosity ;
      owl:onProperty qudt:hasQuantityKind ;
    ] ;
  skos:exactMatch <http://dbpedia.org/resource/Category:Units_of_dynamic_viscosity> ;
  prov:wasInfluencedBy <http://no-valid-base-found.com/> ;
.
qudt:ElectricChargeAreaDensityUnit
  a owl:Class ;
  dct:description "A sub-type of 'Electric Charge Density Unit'. Detailed desciption to be provided in a future version." ;
  rdfs:isDefinedBy <http://qudt.org/2.0/schema/qudt/science> ;
  rdfs:isDefinedBy qudt:science ;
  rdfs:label "Electric Charge Area Density Unit" ;
  rdfs:subClassOf qudt:ElectricChargeDensityUnit ;
  rdfs:subClassOf [
      a owl:Restriction ;
      owl:hasValue quantitykind:PolarizationField ;
      owl:onProperty qudt:hasQuantityKind ;
    ] ;
.
qudt:ElectricChargeDensityUnit
  a owl:Class ;
  qudt:description "The linear, surface, or volume charge density is the amount of electric charge in a line, surface, or volume. It is measured in coulombs per metre (C/m), square metre (C/m^2), or cubic metre (C/m^3), respectively. Since there are positive as well as negative charges, the charge density can take on negative values."^^rdf:HTML ;
  rdfs:isDefinedBy <http://qudt.org/2.0/schema/qudt/science> ;
  rdfs:isDefinedBy qudt:science ;
  rdfs:label "Electric Charge Density Unit" ;
  rdfs:subClassOf qudt:ElectricChargeUnit ;
.
qudt:ElectricChargeLineDensityUnit
  a owl:Class ;
  qudt:description "The linear charge density is the amount of electric charge in a line. It is measured in coulombs per metre (C/m). Since there are positive as well as negative charges, the charge density can take on negative values. [Wikipedia]"^^rdf:HTML ;
  rdfs:isDefinedBy <http://qudt.org/2.0/schema/qudt/science> ;
  rdfs:isDefinedBy qudt:science ;
  rdfs:label "Electric Charge Line Density Unit" ;
  rdfs:subClassOf qudt:ElectricChargeDensityUnit ;
  rdfs:subClassOf [
      a owl:Restriction ;
      owl:hasValue quantitykind:ElectricChargeLineDensity ;
      owl:onProperty qudt:hasQuantityKind ;
    ] ;
.
qudt:ElectricChargePerAmountOfSubstanceUnit
  a owl:Class ;
  dct:description "A sub-type of 'Electric Charge Density Unit'. Detailed desciption to be provided in a future version." ;
  rdfs:isDefinedBy <http://qudt.org/2.0/schema/qudt/science> ;
  rdfs:isDefinedBy qudt:science ;
  rdfs:label "Electric charge per amount of substance unit" ;
  rdfs:subClassOf qudt:ElectricChargeDensityUnit ;
.
qudt:ElectricChargeUnit
  a owl:Class ;
  qudt:description "\"Electric Charge\" is a fundamental conserved property of some subatomic particles, which determines their electromagnetic interaction. Electrically charged matter is influenced by, and produces, electromagnetic fields. The interaction between a moving charge and an electromagnetic field is the source of the electromagnetic force, which is one of the four fundamental forces."^^rdf:HTML ;
  rdfs:isDefinedBy <http://qudt.org/2.0/schema/qudt/science> ;
  rdfs:isDefinedBy qudt:science ;
  rdfs:label "Electric Charge Unit" ;
  rdfs:subClassOf qudt:ElectricityAndMagnetismUnit ;
  rdfs:subClassOf [
      a owl:Restriction ;
      owl:hasValue quantitykind:ElectricCharge ;
      owl:onProperty qudt:hasQuantityKind ;
    ] ;
  skos:exactMatch <http://dbpedia.org/resource/Category:Units_of_electrical_charge> ;
.
qudt:ElectricChargeVolumeDensityUnit
  a owl:Class ;
  qudt:description "The volume charge density is the amount of electric charge in a volume. It is measured in coulombs per cubic metre (C/m^3).  Since there are positive as well as negative charges, the charge density can take on negative values. [Wikipedia]"^^rdf:HTML ;
  rdfs:isDefinedBy <http://qudt.org/2.0/schema/qudt/science> ;
  rdfs:isDefinedBy qudt:science ;
  rdfs:label "Electric Charge Volume Density Unit" ;
  rdfs:subClassOf qudt:ElectricChargeDensityUnit ;
  rdfs:subClassOf [
      a owl:Restriction ;
      owl:hasValue quantitykind:ElectricChargeVolumeDensity ;
      owl:onProperty qudt:hasQuantityKind ;
    ] ;
.
qudt:ElectricCurrentDensityUnit
  a owl:Class ;
  qudt:description "<p class=\"lm-para\"><b>Electric Current Density</b> is a measure of the density of flow of a conserved charge. Usually the charge is the electric charge, in which case the associated current density is the electric current per unit area of cross section, but the term current density can also be applied to other conserved quantities. It is defined as a vector whose magnitude is the current per cross-sectional area.  In SI units, the electric current density is measured in \\(ampere\\,per\\,metre\\,squared\\).</p>"^^rdf:HTML ;
  rdfs:isDefinedBy <http://qudt.org/2.0/schema/qudt/science> ;
  rdfs:isDefinedBy qudt:science ;
  rdfs:label "Electric Current Density Unit" ;
  rdfs:subClassOf qudt:ElectricCurrentUnit ;
  rdfs:subClassOf [
      a owl:Restriction ;
      owl:hasValue quantitykind:ElectricCurrentDensity ;
      owl:onProperty qudt:hasQuantityKind ;
    ] ;
.
qudt:ElectricCurrentUnit
  a owl:Class ;
  qudt:description "\"Electric Current\" is the flow (movement) of electric charge. The SI unit of electric current is the ampere."^^rdf:HTML ;
  rdfs:isDefinedBy <http://qudt.org/2.0/schema/qudt/science> ;
  rdfs:isDefinedBy qudt:science ;
  rdfs:label "Electric Current Unit" ;
  rdfs:subClassOf qudt:ElectricityAndMagnetismUnit ;
  rdfs:subClassOf [
      a owl:Restriction ;
      owl:hasValue quantitykind:ElectricCurrent ;
      owl:onProperty qudt:hasQuantityKind ;
    ] ;
  skos:exactMatch <http://dbpedia.org/resource/Category:Units_of_electrical_current> ;
.
qudt:ElectricDipoleMomentUnit
  a owl:Class ;
  qudt:description "The electric dipole moment (or electric dipole for short) is a measure of the polarity of a system of electric charges. "^^rdf:HTML ;
  rdfs:isDefinedBy <http://qudt.org/2.0/schema/qudt/science> ;
  rdfs:isDefinedBy qudt:science ;
  rdfs:label "Electric Dipole Moment Unit" ;
  rdfs:subClassOf qudt:ElectricityAndMagnetismUnit ;
  rdfs:subClassOf [
      a owl:Restriction ;
      owl:hasValue quantitykind:ElectricDipoleMoment ;
      owl:onProperty qudt:hasQuantityKind ;
    ] ;
.
qudt:ElectricFieldStrengthUnit
  a owl:Class ;
  qudt:description "<p class=\"lm-para\">The strength of the electric field at a given point is defined as the force that would be exerted on a positive test charge of +1 coulomb placed at that point; the direction of the field is given by the direction of that force. Electric fields contain electrical energy with energy density proportional to the square of the field intensity. The electric field is to charge as gravitational acceleration is to mass and force density is to volume.</p>"^^rdf:HTML ;
  rdfs:isDefinedBy <http://qudt.org/2.0/schema/qudt/science> ;
  rdfs:isDefinedBy qudt:science ;
  rdfs:label "Electric Field Strength Unit" ;
  rdfs:subClassOf qudt:ElectricityAndMagnetismUnit ;
  rdfs:subClassOf [
      a owl:Restriction ;
      owl:hasValue quantitykind:ElectricFieldStrength ;
      owl:onProperty qudt:hasQuantityKind ;
    ] ;
.
qudt:ElectricFluxDensityUnit
  a owl:Class ;
  dct:description "A sub-type of 'Electric Charge Density Unit'. Detailed desciption to be provided in a future version." ;
  rdfs:isDefinedBy <http://qudt.org/2.0/schema/qudt/science> ;
  rdfs:isDefinedBy qudt:science ;
  rdfs:label "Electric Flux Density Unit" ;
  rdfs:subClassOf qudt:ElectricChargeDensityUnit ;
  rdfs:subClassOf [
      a owl:Restriction ;
      owl:hasValue quantitykind:ElectricDisplacement ;
      owl:onProperty qudt:hasQuantityKind ;
    ] ;
.
qudt:ElectricFluxUnit
  a owl:Class ;
  dct:description "A sub-type of 'Electricity And Magnetism Unit'. Detailed desciption to be provided in a future version." ;
  rdfs:isDefinedBy <http://qudt.org/2.0/schema/qudt/science> ;
  rdfs:isDefinedBy qudt:science ;
  rdfs:label "Electric Flux Unit" ;
  rdfs:subClassOf qudt:ElectricityAndMagnetismUnit ;
.
qudt:ElectricPowerUnit
  a owl:Class ;
  dct:description "A sub-type of 'Electricity And Magnetism Unit'. Detailed desciption to be provided in a future version." ;
  rdfs:isDefinedBy <http://qudt.org/2.0/schema/qudt/science> ;
  rdfs:isDefinedBy qudt:science ;
  rdfs:label "Electric power unit" ;
  rdfs:subClassOf qudt:ElectricityAndMagnetismUnit ;
.
qudt:ElectricalEngineeringQuantityKind
  a owl:Class ;
  dct:description "A sub-type of 'Engineering quantity kind'. Detailed desciption to be provided in a future version." ;
  rdfs:isDefinedBy <http://qudt.org/2.0/schema/qudt/science> ;
  rdfs:isDefinedBy qudt:science ;
  rdfs:label "Electrical Engineering Quantity Kind" ;
  rdfs:subClassOf qudt:EngineeringQuantityKind ;
  skos:prefLabel "Electrical engineering quantity kind" ;
.
qudt:ElectricityAndMagnetismQuantityKind
  a owl:Class ;
  dct:description "A sub-type of 'Physics Quantity Kind'. Detailed desciption to be provided in a future version." ;
  rdfs:isDefinedBy <http://qudt.org/2.0/schema/qudt/science> ;
  rdfs:isDefinedBy qudt:science ;
  rdfs:label "Electricity and Magnetism" ;
  rdfs:subClassOf qudt:PhysicsQuantityKind ;
.
qudt:ElectricityAndMagnetismUnit
  a owl:Class ;
  qudt:description "The class of units used to measure the properties of electricity and magnetism."^^rdf:HTML ;
  qudt:fieldCode "720" ;
  rdfs:isDefinedBy <http://qudt.org/2.0/schema/qudt/science> ;
  rdfs:isDefinedBy qudt:science ;
  rdfs:label "Electricity And Magnetism Unit" ;
  rdfs:subClassOf qudt:PhysicsUnit ;
  rdfs:subClassOf [
      a owl:Restriction ;
      owl:allValuesFrom qudt:ElectricityAndMagnetismQuantityKind ;
      owl:onProperty qudt:hasQuantityKind ;
    ] ;
  owl:equivalentClass [
      a owl:Restriction ;
      owl:allValuesFrom qudt:ElectricityAndMagnetismQuantityKind ;
      owl:onProperty qudt:hasQuantityKind ;
    ] ;
.
qudt:ElectrochemistryUnit
  a owl:Class ;
  dct:description "A sub-type of 'Chemistry Unit' and 'Electricity And Magnetism Unit'. Detailed desciption to be provided in a future version." ;
  rdfs:isDefinedBy <http://qudt.org/2.0/schema/qudt/science> ;
  rdfs:isDefinedBy qudt:science ;
  rdfs:label "Electrochemistry Unit" ;
  rdfs:subClassOf qudt:ChemistryUnit ;
  rdfs:subClassOf qudt:ElectricityAndMagnetismUnit ;
.
qudt:ElectronicEngineeringQuantityKind
  a owl:Class ;
  dct:description "A sub-type of 'Engineering quantity kind'. Detailed desciption to be provided in a future version." ;
  rdfs:isDefinedBy <http://qudt.org/2.0/schema/qudt/science> ;
  rdfs:isDefinedBy qudt:science ;
  rdfs:label "Electronic Engineering Quantity Kind" ;
  rdfs:subClassOf qudt:EngineeringQuantityKind ;
.
qudt:EnergyAndWorkPerMassAmountOfSubstance
  a owl:Class ;
  dct:description "A sub-type of 'Chemistry Unit'. Detailed desciption to be provided in a future version." ;
  rdfs:isDefinedBy <http://qudt.org/2.0/schema/qudt/science> ;
  rdfs:isDefinedBy qudt:science ;
  rdfs:label "Energy and work per mass amount of substance" ;
  rdfs:subClassOf qudt:ChemistryUnit ;
  rdfs:subClassOf [
      a owl:Restriction ;
      owl:hasValue quantitykind:EnergyAndWorkPerMassAmountOfSubstance ;
      owl:onProperty qudt:hasQuantityKind ;
    ] ;
.
qudt:EnergyAndWorkUnit
  a owl:Class ;
  dct:description "A sub-type of 'Energy unit'. Detailed desciption to be provided in a future version." ;
  rdfs:isDefinedBy <http://qudt.org/2.0/schema/qudt/science> ;
  rdfs:isDefinedBy qudt:science ;
  rdfs:label "Energy And Work Unit" ;
  rdfs:subClassOf qudt:EnergyUnit ;
  rdfs:subClassOf [
      a owl:Restriction ;
      owl:hasValue quantitykind:EnergyAndWork ;
      owl:onProperty qudt:hasQuantityKind ;
    ] ;
  skos:exactMatch <http://dbpedia.org/resource/Category:Units_of_energy> ;
.
qudt:EnergyDensityUnit
  a owl:Class ;
  qudt:description "Units that measure energy density, i.e. energy per unit volume."^^rdf:HTML ;
  rdfs:isDefinedBy <http://qudt.org/2.0/schema/qudt/science> ;
  rdfs:isDefinedBy qudt:science ;
  rdfs:label "Energy Density Unit" ;
  rdfs:subClassOf qudt:EnergyUnit ;
  rdfs:subClassOf [
      a owl:Restriction ;
      owl:hasValue quantitykind:EnergyDensity ;
      owl:onProperty qudt:hasQuantityKind ;
    ] ;
.
qudt:EnergyPerAreaUnit
  a owl:Class ;
  qudt:description "Units that quantify energy per unit area."^^rdf:HTML ;
  rdfs:isDefinedBy <http://qudt.org/2.0/schema/qudt/science> ;
  rdfs:isDefinedBy qudt:science ;
  rdfs:label "Energy Per Area Unit" ;
  rdfs:subClassOf qudt:EnergyUnit ;
  rdfs:subClassOf [
      a owl:Restriction ;
      owl:hasValue quantitykind:EnergyPerArea ;
      owl:onProperty qudt:hasQuantityKind ;
    ] ;
.
qudt:EnergyPerElectricChargeUnit
  a owl:Class ;
  qudt:description "The ratio of energy to electric charge arises repeatedly in electrodynamics. It is the dimensional equivalent to the electrostatic potential and electromotive force. In both cases, the SI unit is the volt, or newton meters per coulomb."^^rdf:HTML ;
  rdfs:isDefinedBy <http://qudt.org/2.0/schema/qudt/science> ;
  rdfs:isDefinedBy qudt:science ;
  rdfs:label "Energy per Electric Charge Unit" ;
  rdfs:subClassOf qudt:ElectricityAndMagnetismUnit ;
  rdfs:subClassOf [
      a owl:Restriction ;
      owl:hasValue quantitykind:ElectromotiveForce ;
      owl:onProperty qudt:hasQuantityKind ;
    ] ;
.
qudt:EnergyQuantityKind
  a owl:Class ;
  dct:description "A sub-type of 'Physics Quantity Kind'. Detailed desciption to be provided in a future version." ;
  rdfs:isDefinedBy <http://qudt.org/2.0/schema/qudt/science> ;
  rdfs:isDefinedBy qudt:science ;
  rdfs:label "Energy quantity kind" ;
  rdfs:subClassOf qudt:PhysicsQuantityKind ;
.
qudt:EnergyUnit
  a owl:Class ;
  dct:description "A sub-type of 'Physics Unit'. Detailed desciption to be provided in a future version." ;
  qudt:fieldCode "730" ;
  rdfs:isDefinedBy <http://qudt.org/2.0/schema/qudt/science> ;
  rdfs:isDefinedBy qudt:science ;
  rdfs:label "Energy unit" ;
  rdfs:subClassOf qudt:PhysicsUnit ;
.
qudt:EngineeringQuantityKind
  a owl:Class ;
  dct:description "A sub-type of 'Quantity Kind'. Detailed desciption to be provided in a future version." ;
  dct:description """Engineering is the science, skill, and profession of acquiring and applying scientific, economic, social, and practical knowledge, in order to design and also build structures, machines, devices, systems, materials and processes.

\"Quantity Kinds} are organzied primarily by domain (subject area of knowledge), however, some \\textit{Quantity Kinds} are specific to the application of a domain of knowledge.  These \\textit{Quantity Kinds\" are organized according to  well-known fields of engineering.""" ;
  rdfs:isDefinedBy <http://qudt.org/2.0/schema/qudt/science> ;
  rdfs:isDefinedBy qudt:science ;
  rdfs:label "Engineering Quantity Kind" ;
  rdfs:subClassOf qudt:QuantityKind ;
  skos:prefLabel "Engineering quantity kind" ;
  prov:wasInfluencedBy <http://en.wikipedia.org/wiki/Engineering> ;
.
qudt:EnumeratedValue
  rdfs:isDefinedBy <http://qudt.org/schema/qudt> ;
.
qudt:Enumeration
  rdfs:isDefinedBy <http://qudt.org/schema/qudt> ;
.
qudt:EnumerationScale
  dct:description "A sub-type of 'DTYPE Enumeration' and 'Scale'. Detailed desciption to be provided in a future version." ;
.
qudt:EnvironmentControlQuantityKind
  a owl:Class ;
  dct:description "A sub-type of 'Space System Engineering Quantity Kind'. Detailed desciption to be provided in a future version." ;
  rdfs:isDefinedBy <http://qudt.org/2.0/schema/qudt/science> ;
  rdfs:isDefinedBy qudt:science ;
  rdfs:label "Environment Control Quantity Kind" ;
  rdfs:subClassOf qudt:SpaceSystemEngineeringQuantityKind ;
.
qudt:EventUnit
  a owl:Class ;
  dct:description "A sub-type of 'Resource Unit'. Detailed desciption to be provided in a future version." ;
  rdfs:isDefinedBy <http://qudt.org/2.0/schema/qudt/science> ;
  rdfs:isDefinedBy qudt:science ;
  rdfs:label "Event Unit" ;
  rdfs:subClassOf qudt:ResourceUnit ;
.
qudt:ExposureUnit
  a owl:Class ;
  dct:description "A sub-type of 'Radiology Unit'. Detailed desciption to be provided in a future version." ;
  rdfs:isDefinedBy <http://qudt.org/2.0/schema/qudt/science> ;
  rdfs:isDefinedBy qudt:science ;
  rdfs:label "Exposure Unit" ;
  rdfs:subClassOf qudt:RadiologyUnit ;
  rdfs:subClassOf [
      a owl:Restriction ;
      owl:hasValue quantitykind:Exposure ;
      owl:onProperty qudt:hasQuantityKind ;
    ] ;
.
qudt:Figure
  dct:description "A sub-type of 'QUDT Concept'. Detailed desciption to be provided in a future version." ;
.
qudt:FinanceQuantityKind
  a owl:Class ;
  dct:description "A sub-type of 'Quantity Kind'. Detailed desciption to be provided in a future version." ;
  rdfs:isDefinedBy <http://qudt.org/2.0/schema/qudt/science> ;
  rdfs:isDefinedBy qudt:science ;
  rdfs:label "Finance Quantity Kind" ;
  rdfs:subClassOf qudt:QuantityKind ;
  skos:exactMatch <http://dbpedia.org/resource/Finance> ;
.
qudt:FinancialUnit
  rdfs:isDefinedBy <http://qudt.org/schema/qudt> ;
  rdfs:subClassOf [
      a owl:Restriction ;
      owl:allValuesFrom qudt:FinanceQuantityKind ;
      owl:onProperty qudt:hasQuantityKind ;
    ] ;
  owl:equivalentClass [
      a owl:Restriction ;
      owl:allValuesFrom qudt:FinanceQuantityKind ;
      owl:onProperty qudt:hasQuantityKind ;
    ] ;
.
qudt:FluidDynamicsQuantityKind
  a owl:Class ;
  dct:description "A sub-type of 'Fluid Mechanics Quantity Kind'. Detailed desciption to be provided in a future version." ;
  dct:description """Fluid dynamics is the sub-discipline of fluid mechanics dealing with fluids (liquids and gases) in motion. It has several subdisciplines itself, including aerodynamics (the study of gases in motion) and hydrodynamics (the study of liquids in motion). Fluid dynamics has a wide range of applications, including calculating forces and moments on aircraft, determining the mass flow rate of petroleum through pipelines, predicting weather patterns, understanding nebulae in interstellar space and reportedly modelling fission weapon detonation. Some of its principles are even used in traffic engineering, where traffic is treated as a continuous fluid.

Fluid dynamics offers a systematic structure that underlies these practical disciplines and that embraces empirical and semi-empirical laws, derived from flow measurement, used to solve practical problems. The solution of a fluid dynamics problem typically involves calculation of various properties of the fluid, such as velocity, pressure, density, and temperature, as functions of space and time.""" ;
  rdfs:isDefinedBy <http://qudt.org/2.0/schema/qudt/science> ;
  rdfs:isDefinedBy qudt:science ;
  rdfs:label "Fluid Dynamics Quantity Kind" ;
  rdfs:subClassOf qudt:FluidMechanicsQuantityKind ;
  prov:wasInfluencedBy <http://en.wikipedia.org/wiki/Fluid_dynamics> ;
.
qudt:FluidDynamicsUnit
  a owl:Class ;
  dct:description "A sub-type of 'Fluid Mechanics Unit'. Detailed desciption to be provided in a future version." ;
  rdfs:isDefinedBy <http://qudt.org/2.0/schema/qudt/science> ;
  rdfs:isDefinedBy qudt:science ;
  rdfs:label "Fluid dynamics unit" ;
  rdfs:subClassOf qudt:FluidMechanicsUnit ;
.
qudt:FluidMechanicsQuantityKind
  a owl:Class ;
  dct:description "A sub-type of 'Classical Mechanics Quantity Kind'. Detailed desciption to be provided in a future version." ;
  rdfs:isDefinedBy <http://qudt.org/2.0/schema/qudt/science> ;
  rdfs:isDefinedBy qudt:science ;
  rdfs:label "Fluid Mechanics Quantity Kind" ;
  rdfs:subClassOf qudt:ClassicalMechanicsQuantityKind ;
.
qudt:FluidMechanicsUnit
  a owl:Class ;
  dct:description "A sub-type of 'Classical Mechanics Unit'. Detailed desciption to be provided in a future version." ;
  rdfs:isDefinedBy <http://qudt.org/2.0/schema/qudt/science> ;
  rdfs:isDefinedBy qudt:science ;
  rdfs:label "Fluid Mechanics Unit" ;
  rdfs:subClassOf qudt:ClassicalMechanicsUnit ;
.
qudt:ForcePerElectricChargeUnit
  a owl:Class ;
  dct:description "A sub-type of 'Electricity And Magnetism Unit'. Detailed desciption to be provided in a future version." ;
  rdfs:isDefinedBy <http://qudt.org/2.0/schema/qudt/science> ;
  rdfs:isDefinedBy qudt:science ;
  rdfs:label "Force Per Electric Charge Unit" ;
  rdfs:subClassOf qudt:ElectricityAndMagnetismUnit ;
  rdfs:subClassOf [
      a owl:Restriction ;
      owl:hasValue quantitykind:ForcePerElectricCharge ;
      owl:onProperty qudt:hasQuantityKind ;
    ] ;
.
qudt:ForcePerLengthUnit
  a owl:Class ;
  dct:description "A sub-type of 'Force Unit'. Detailed desciption to be provided in a future version." ;
  rdfs:isDefinedBy <http://qudt.org/2.0/schema/qudt/science> ;
  rdfs:isDefinedBy qudt:science ;
  rdfs:label "Force Per Length Unit" ;
  rdfs:subClassOf qudt:ForceUnit ;
  rdfs:subClassOf [
      a owl:Restriction ;
      owl:hasValue quantitykind:ForcePerLength ;
      owl:onProperty qudt:hasQuantityKind ;
    ] ;
.
qudt:ForceUnit
  a owl:Class ;
  dct:description "A sub-type of 'Classical Mechanics Unit'. Detailed desciption to be provided in a future version." ;
  rdfs:isDefinedBy <http://qudt.org/2.0/schema/qudt/science> ;
  rdfs:isDefinedBy qudt:science ;
  rdfs:label "Force Unit" ;
  rdfs:subClassOf qudt:ClassicalMechanicsUnit ;
  rdfs:subClassOf [
      a owl:Restriction ;
      owl:hasValue quantitykind:Force ;
      owl:onProperty qudt:hasQuantityKind ;
    ] ;
  skos:exactMatch <http://dbpedia.org/resource/Category:Units_of_force> ;
.
qudt:FrequencyUnit
  a owl:Class ;
  dct:description "A sub-type of 'Space And Time Unit'. Detailed desciption to be provided in a future version." ;
  rdfs:isDefinedBy <http://qudt.org/2.0/schema/qudt/science> ;
  rdfs:isDefinedBy qudt:science ;
  rdfs:label "Frequency Unit" ;
  rdfs:subClassOf qudt:SpaceAndTimeUnit ;
  skos:exactMatch <http://dbpedia.org/resource/Category:Units_of_frequency> ;
.
qudt:GravitationalAttractionUnit
  a owl:Class ;
  dct:description "A sub-type of 'Mechanics Unit'. Detailed desciption to be provided in a future version." ;
  rdfs:isDefinedBy <http://qudt.org/2.0/schema/qudt/science> ;
  rdfs:isDefinedBy qudt:science ;
  rdfs:label "Gravitational Attraction Unit" ;
  rdfs:subClassOf qudt:MechanicsUnit ;
  rdfs:subClassOf [
      a owl:Restriction ;
      owl:hasValue quantitykind:GravitationalAttraction ;
      owl:onProperty qudt:hasQuantityKind ;
    ] ;
.
qudt:GreekCharacter
  a owl:Class ;
  dc:source "http://www.charbase.com/block/greek-and-coptic" ;
  dct:description "A sub-type of 'Symbol'. Detailed desciption to be provided in a future version." ;
  rdfs:isDefinedBy <http://qudt.org/2.0/schema/qudt/science> ;
  rdfs:isDefinedBy qudt:science ;
  rdfs:label "Greek character" ;
  rdfs:subClassOf qudt:Symbol ;
  skos:prefLabel "Greek character" ;
.
qudt:GuidanceAndNavigationQuantityKind
  a owl:Class ;
  dct:description "A sub-type of 'Astrionics Quantity Kind' and 'Avionics Quantity Kind'. Detailed desciption to be provided in a future version." ;
  rdfs:isDefinedBy <http://qudt.org/2.0/schema/qudt/science> ;
  rdfs:isDefinedBy qudt:science ;
  rdfs:label "Guidance And Navigation Quantity Kind" ;
  rdfs:subClassOf qudt:AstrionicsQuantityKind ;
  rdfs:subClassOf qudt:AvionicsQuantityKind ;
.
qudt:HeartRateUnit
  a owl:Class ;
  dct:description "A sub-type of 'Biomedical Unit'. Detailed desciption to be provided in a future version." ;
  rdfs:isDefinedBy <http://qudt.org/2.0/schema/qudt/science> ;
  rdfs:isDefinedBy qudt:science ;
  rdfs:label "Heart Rate Unit" ;
  rdfs:subClassOf qudt:BiomedicalUnit ;
  rdfs:subClassOf [
      a owl:Restriction ;
      owl:hasValue quantitykind:HeartRate ;
      owl:onProperty qudt:hasQuantityKind ;
    ] ;
.
qudt:HeatCapacityAndEntropyUnit
  a owl:Class ;
  dct:description "A sub-type of 'Thermodynamics Unit'. Detailed desciption to be provided in a future version." ;
  rdfs:isDefinedBy <http://qudt.org/2.0/schema/qudt/science> ;
  rdfs:isDefinedBy qudt:science ;
  rdfs:label "Heat Capacity And Entropy Unit" ;
  rdfs:subClassOf qudt:ThermodynamicsUnit ;
  rdfs:subClassOf [
      a owl:Restriction ;
      owl:hasValue quantitykind:HeatCapacity ;
      owl:onProperty qudt:hasQuantityKind ;
    ] ;
.
qudt:HeatFlowRateUnit
  a owl:Class ;
  dct:description "A sub-type of 'Thermodynamics Unit'. Detailed desciption to be provided in a future version." ;
  rdfs:isDefinedBy <http://qudt.org/2.0/schema/qudt/science> ;
  rdfs:isDefinedBy qudt:science ;
  rdfs:label "Heat Flow Rate Unit" ;
  rdfs:subClassOf qudt:ThermodynamicsUnit ;
  rdfs:subClassOf [
      a owl:Restriction ;
      owl:hasValue quantitykind:ElectricPower ;
      owl:onProperty qudt:hasQuantityKind ;
    ] ;
  rdfs:subClassOf [
      a owl:Restriction ;
      owl:hasValue quantitykind:HeatFlowRate ;
      owl:onProperty qudt:hasQuantityKind ;
    ] ;
.
qudt:HumanFactorsQuantityKind
  a owl:Class ;
  dct:description "A sub-type of 'Social Science Quantity Kind'. Detailed desciption to be provided in a future version." ;
  rdfs:isDefinedBy <http://qudt.org/2.0/schema/qudt/science> ;
  rdfs:isDefinedBy qudt:science ;
  rdfs:label "Human Factors Quantity Kind" ;
  rdfs:subClassOf qudt:SocialScienceQuantityKind ;
.
qudt:HumanUnit
  a owl:Class ;
  qudt:description "units for measuring human resources"^^rdf:HTML ;
  rdfs:isDefinedBy <http://qudt.org/2.0/schema/qudt/science> ;
  rdfs:isDefinedBy qudt:science ;
  rdfs:label "Human Unit" ;
  rdfs:subClassOf qudt:ResourceUnit ;
.
qudt:HydraulicsQuantityKind
  a owl:Class ;
  dct:description "A sub-type of 'Classical Mechanics Quantity Kind'. Detailed desciption to be provided in a future version." ;
  rdfs:isDefinedBy <http://qudt.org/2.0/schema/qudt/science> ;
  rdfs:isDefinedBy qudt:science ;
  rdfs:label "Hydraulics Quantity Kind" ;
  rdfs:subClassOf qudt:ClassicalMechanicsQuantityKind ;
.
qudt:HydraulicsUnit
  a owl:Class ;
  dct:description "A sub-type of 'Classical Mechanics Unit'. Detailed desciption to be provided in a future version." ;
  rdfs:isDefinedBy <http://qudt.org/2.0/schema/qudt/science> ;
  rdfs:isDefinedBy qudt:science ;
  rdfs:label "Hydraulics unit" ;
  rdfs:subClassOf qudt:ClassicalMechanicsUnit ;
.
qudt:HydrodynamicsQuantityKind
  a owl:Class ;
  dct:description "A sub-type of 'Fluid Dynamics Quantity Kind'. Detailed desciption to be provided in a future version." ;
  rdfs:isDefinedBy <http://qudt.org/2.0/schema/qudt/science> ;
  rdfs:isDefinedBy qudt:science ;
  rdfs:label "Hydrodynamics Quantity Kind" ;
  rdfs:subClassOf qudt:FluidDynamicsQuantityKind ;
.
qudt:HypersonicAerodynamicsQuantityKind
  a owl:Class ;
  dct:description "A sub-type of 'Aerodynamics Quantity Kind'. Detailed desciption to be provided in a future version." ;
  rdfs:isDefinedBy <http://qudt.org/2.0/schema/qudt/science> ;
  rdfs:isDefinedBy qudt:science ;
  rdfs:label "Hypersonic Aerodynamics Quantity Kind" ;
  rdfs:subClassOf qudt:AerodynamicsQuantityKind ;
  skos:definition "Hypersonic aerodynamics is a special branch of the study of aeronautics. The chief characteristic of hypersonic aerodynamics is that the temperature of the flow around the aircraft is so great that the chemistry of the gas must be considered. At low hypersonic speeds, the molecular bonds vibrate, which changes the magnitude of the forces generated by the air on the aircraft. At higher hypersonic speeds, the molecules break apart producing an electrically charged plasma around the aircraft. Large variations in air density and pressure occur because of shock waves, and expansions. Hypersonic aircraft typically have very thick boundary layers along the surface and high heat transfer to the surface. All of these high speed flow phenomena lead to a vehicle design unlike the typical airliner or fighter aircraft." ;
  prov:wasInfluencedBy <http://www.grc.nasa.gov/WWW/BGH/bgh.html> ;
.
qudt:IMPERIAL-DimensionVector
  dct:description "A sub-type of 'Quantity Dimension Vector'. Detailed desciption to be provided in a future version." ;
.
qudt:ISO-DimensionVector
  dct:description "A sub-type of 'Quantity Dimension Vector'. Detailed desciption to be provided in a future version." ;
.
qudt:IlluminanceUnit
  rdfs:isDefinedBy <http://qudt.org/schema/qudt> ;
  rdfs:subClassOf [
      a owl:Restriction ;
      owl:hasValue quantitykind:Illuminance ;
      owl:onProperty qudt:hasQuantityKind ;
    ] ;
.
qudt:ImperialUnit
  dct:description "A sub-type of 'Standards unit'. Detailed desciption to be provided in a future version." ;
.
qudt:InductanceUnit
  a owl:Class ;
  qudt:description """An electric current flowing around a circuit produces a magnetic field and hence a magnetic flux through the circuit. The ratio of the magnetic flux to the current is called the inductance, or more accurately self-inductance of the circuit. [Wikipedia]



This class contains the following instance(s): \"Abhenry\", \"Henry\", \"Micro Henry\", \"Milli Henry\", \"Stathenry\"."""^^rdf:HTML ;
  rdfs:isDefinedBy <http://qudt.org/2.0/schema/qudt/science> ;
  rdfs:isDefinedBy qudt:science ;
  rdfs:label "Inductance Unit" ;
  rdfs:subClassOf qudt:ElectricityAndMagnetismUnit ;
  rdfs:subClassOf [
      a owl:Restriction ;
      owl:hasValue quantitykind:Inductance ;
      owl:onProperty qudt:hasQuantityKind ;
    ] ;
  skos:exactMatch <http://dbpedia.org/resource/Category:Units_of_electrical_inductance> ;
.
qudt:InformaticsQuantityKind
  a owl:Class ;
  dct:description "A sub-type of 'Computer Science Quantity Kind'. Detailed desciption to be provided in a future version." ;
  rdfs:isDefinedBy <http://qudt.org/2.0/schema/qudt/science> ;
  rdfs:isDefinedBy qudt:science ;
  rdfs:label "Infomatics Quantity Kind" ;
  rdfs:subClassOf qudt:ComputerScienceQuantityKind ;
  skos:prefLabel "Infomatics quantity kind" ;
.
qudt:InformaticsUnit
  a owl:Class ;
  dct:description "A sub-type of 'Science unit'. Detailed desciption to be provided in a future version." ;
  qudt:fieldCode "110" ;
  rdfs:isDefinedBy <http://qudt.org/2.0/schema/qudt/science> ;
  rdfs:isDefinedBy qudt:science ;
  rdfs:label "Informatics Unit" ;
  rdfs:subClassOf qudt:ScienceUnit ;
  skos:closeMatch <http://dbpedia.org/resource/Category:Units_of_information> ;
.
qudt:InformationEntropyUnit
  a owl:Class ;
  dct:description "A sub-type of 'Informatics Unit' and 'Logarithmic Unit'. Detailed desciption to be provided in a future version." ;
  rdfs:isDefinedBy <http://qudt.org/2.0/schema/qudt/science> ;
  rdfs:isDefinedBy qudt:science ;
  rdfs:label "Information Entropy Unit" ;
  rdfs:subClassOf qudt:InformaticsUnit ;
  rdfs:subClassOf qudt:LogarithmicUnit ;
  rdfs:subClassOf qudt:ResourceUnit ;
  rdfs:subClassOf [
      a owl:Restriction ;
      owl:hasValue quantitykind:InformationEntropy ;
      owl:onProperty qudt:hasQuantityKind ;
    ] ;
.
qudt:InformationTheoryQuantityKind
  a owl:Class ;
  dct:description "A sub-type of 'Infomatics quantity kind'. Detailed desciption to be provided in a future version." ;
  rdfs:isDefinedBy <http://qudt.org/2.0/schema/qudt/science> ;
  rdfs:isDefinedBy qudt:science ;
  rdfs:label "Information Theory Quantity Kind" ;
  rdfs:subClassOf qudt:InformaticsQuantityKind ;
  skos:exactMatch <http://dbpedia.org/resource/Information> ;
.
qudt:IntegratedSystemHealthMonitoringQuantityKind
  a owl:Class ;
  dct:description "A sub-type of 'System Engineering Quantity Kind'. Detailed desciption to be provided in a future version." ;
  dct:description "Integrated System Health Management (ISHM) is the unified capability of systems to assess the current or future state of the member system health and integrate that picture of system health within a framework of available resources and operational demand." ;
  rdfs:isDefinedBy <http://qudt.org/2.0/schema/qudt/science> ;
  rdfs:isDefinedBy qudt:science ;
  rdfs:label "Integrated System Health Monitoring (ISHM) Quantity Kind" ;
  rdfs:subClassOf qudt:SystemEngineeringQuantityKind ;
  skos:prefLabel "Integrated system health monitoring" ;
  prov:wasInfluencedBy <http://en.wikipedia.org/wiki/Integrated_Vehicle_Health_Management> ;
.
qudt:IntegratedVehicleHealthManagementQuantityKind
  a owl:Class ;
  dct:description "A sub-type of 'System Engineering Quantity Kind'. Detailed desciption to be provided in a future version." ;
  dct:description "Integrated Vehicle Health Management (IVHM) is the unified capability of systems to assess the current or future state of the member system health and integrate that picture of system health within a framework of available resources and operational demand." ;
  rdfs:isDefinedBy <http://qudt.org/2.0/schema/qudt/science> ;
  rdfs:isDefinedBy qudt:science ;
  rdfs:label "Integrated Vehicle Health Management (IVHM) Quantity Kind" ;
  rdfs:subClassOf qudt:SystemEngineeringQuantityKind ;
  prov:wasInfluencedBy <http://archive.org/details/nasa_techdoc_20020063487> ;
  prov:wasInfluencedBy <http://en.wikipedia.org/wiki/Integrated_Vehicle_Health_Management> ;
  prov:wasInfluencedBy <http://www.nasa.gov/centers/ames/research/humaninspace/humansinspace-ivhm.html> ;
.
qudt:International-CustomaryUnit
  dct:description "A sub-type of 'Standards unit'. Detailed desciption to be provided in a future version." ;
.
qudt:InverseAmountOfSubstanceUnit
  a owl:Class ;
  dct:description "A sub-type of 'Chemistry Unit'. Detailed desciption to be provided in a future version." ;
  rdfs:isDefinedBy <http://qudt.org/2.0/schema/qudt/science> ;
  rdfs:isDefinedBy qudt:science ;
  rdfs:label "Inverse Amount Of Substance Unit" ;
  rdfs:subClassOf qudt:ChemistryUnit ;
.
qudt:KinematicViscosityUnit
  a owl:Class ;
  qudt:description "Kinematic viscosity is a measure of the resistive flow of a fluid under the influence of gravity. It is frequently measured using a device called a capillary viscometer — basically a graduated can with a narrow tube at the bottom. When two fluids of equal volume are placed in identical capillary viscometers and allowed to flow under the influence of gravity, a viscous fluid takes longer than a less viscous fluid to flow through the tube. Capillary viscometers are discussed in more detail later in this section."^^rdf:HTML ;
  rdfs:isDefinedBy <http://qudt.org/2.0/schema/qudt/science> ;
  rdfs:isDefinedBy qudt:science ;
  rdfs:label "Kinematic Viscosity Units" ;
  rdfs:subClassOf qudt:ViscosityUnit ;
  rdfs:subClassOf [
      a owl:Restriction ;
      owl:hasValue quantitykind:KinematicViscosity ;
      owl:onProperty qudt:hasQuantityKind ;
    ] ;
  prov:wasInfluencedBy <http://en.wikipedia.org/wiki/Viscosity#Kinematic_viscosity> ;
  prov:wasInfluencedBy <http://physics.info/viscosity/> ;
.
qudt:KinematicsQuantityKind
  a owl:Class ;
  dct:description "A sub-type of 'Classical Mechanics Quantity Kind'. Detailed desciption to be provided in a future version." ;
  rdfs:isDefinedBy <http://qudt.org/2.0/schema/qudt/science> ;
  rdfs:isDefinedBy qudt:science ;
  rdfs:label "Kinematics Quantity Kind" ;
  rdfs:subClassOf qudt:ClassicalMechanicsQuantityKind ;
.
qudt:KinematicsUnit
  a owl:Class ;
  dct:description "A sub-type of 'Classical Mechanics Unit'. Detailed desciption to be provided in a future version." ;
  rdfs:isDefinedBy <http://qudt.org/2.0/schema/qudt/science> ;
  rdfs:isDefinedBy qudt:science ;
  rdfs:label "Kinematics unit" ;
  rdfs:subClassOf qudt:ClassicalMechanicsUnit ;
.
qudt:KnowledgeEngineeringQuantityKind
  a owl:Class ;
  dct:description "A sub-type of 'Engineering quantity kind'. Detailed desciption to be provided in a future version." ;
  rdfs:isDefinedBy <http://qudt.org/2.0/schema/qudt/science> ;
  rdfs:isDefinedBy qudt:science ;
  rdfs:label "Knowledge Engineering Quantity Kind" ;
  rdfs:subClassOf qudt:EngineeringQuantityKind ;
.
qudt:LengthTemperatureTimeUnit
  a owl:Class ;
  dct:description "A sub-type of 'Thermodynamics Unit'. Detailed desciption to be provided in a future version." ;
  rdfs:isDefinedBy <http://qudt.org/2.0/schema/qudt/science> ;
  rdfs:isDefinedBy qudt:science ;
  rdfs:label "Length Temperature Time Unit" ;
  rdfs:subClassOf qudt:ThermodynamicsUnit ;
  rdfs:subClassOf [
      a owl:Restriction ;
      owl:hasValue quantitykind:LengthTemperatureTime ;
      owl:onProperty qudt:hasQuantityKind ;
    ] ;
.
qudt:LengthTemperatureUnit
  a owl:Class ;
  dct:description "A sub-type of 'Thermodynamics Unit'. Detailed desciption to be provided in a future version." ;
  rdfs:isDefinedBy <http://qudt.org/2.0/schema/qudt/science> ;
  rdfs:isDefinedBy qudt:science ;
  rdfs:label "Length Temperature Unit" ;
  rdfs:subClassOf qudt:ThermodynamicsUnit ;
  rdfs:subClassOf [
      a owl:Restriction ;
      owl:hasValue quantitykind:LengthTemperature ;
      owl:onProperty qudt:hasQuantityKind ;
    ] ;
.
qudt:LengthUnit
  a owl:Class ;
  dct:description "A sub-type of 'Space And Time Unit'. Detailed desciption to be provided in a future version." ;
  rdfs:isDefinedBy <http://qudt.org/2.0/schema/qudt/science> ;
  rdfs:isDefinedBy qudt:science ;
  rdfs:label "Length Unit" ;
  rdfs:subClassOf qudt:SpaceAndTimeUnit ;
  rdfs:subClassOf [
      a owl:Restriction ;
      owl:hasValue quantitykind:Length ;
      owl:onProperty qudt:hasQuantityKind ;
    ] ;
  skos:exactMatch <http://dbpedia.org/resource/Category:Units_of_length> ;
.
qudt:LifeSciencesQuantityKind
  a owl:Class ;
  dct:description "A sub-type of 'Biology'. Detailed desciption to be provided in a future version." ;
  rdfs:isDefinedBy <http://qudt.org/2.0/schema/qudt/science> ;
  rdfs:isDefinedBy qudt:science ;
  rdfs:label "Life Sciences Quantity Kind" ;
  rdfs:subClassOf qudt:BiologyQuantityKind ;
.
qudt:LightQuantityKind
  a owl:Class ;
  dct:description "A sub-type of 'Science quantity kind'. Detailed desciption to be provided in a future version." ;
  rdfs:isDefinedBy <http://qudt.org/2.0/schema/qudt/science> ;
  rdfs:isDefinedBy qudt:science ;
  rdfs:label "Light quantity kind" ;
  rdfs:subClassOf qudt:ScienceQuantityKind ;
.
qudt:LinearAccelerationUnit
  a owl:Class ;
  dct:description "A sub-type of 'Acceleration Unit'. Detailed desciption to be provided in a future version." ;
  rdfs:isDefinedBy <http://qudt.org/2.0/schema/qudt/science> ;
  rdfs:isDefinedBy qudt:science ;
  rdfs:label "Linear Acceleration Unit" ;
  rdfs:subClassOf qudt:AccelerationUnit ;
  rdfs:subClassOf [
      a owl:Restriction ;
      owl:hasValue quantitykind:LinearAcceleration ;
      owl:onProperty qudt:hasQuantityKind ;
    ] ;
  skos:exactMatch <http://dbpedia.org/resource/Category:Units_of_acceleration> ;
.
qudt:LinearEnergyTransferUnit
  a owl:Class ;
  dct:description "A sub-type of 'Energy unit'. Detailed desciption to be provided in a future version." ;
  rdfs:isDefinedBy <http://qudt.org/2.0/schema/qudt/science> ;
  rdfs:isDefinedBy qudt:science ;
  rdfs:label "Linear energy transfer unit" ;
  rdfs:subClassOf qudt:EnergyUnit ;
  rdfs:subClassOf [
      a owl:Restriction ;
      owl:hasValue quantitykind:LinearEnergyTransfer ;
      owl:onProperty qudt:hasQuantityKind ;
    ] ;
.
qudt:LinearMomentumUnit
  a owl:Class ;
  dct:description "A sub-type of 'Momentum Unit'. Detailed desciption to be provided in a future version." ;
  rdfs:isDefinedBy <http://qudt.org/2.0/schema/qudt/science> ;
  rdfs:isDefinedBy qudt:science ;
  rdfs:label "Linear Momentum Unit" ;
  rdfs:subClassOf qudt:MomentumUnit ;
  rdfs:subClassOf [
      a owl:Restriction ;
      owl:hasValue quantitykind:LinearMomentum ;
      owl:onProperty qudt:hasQuantityKind ;
    ] ;
.
qudt:LinearThermalExpansionUnit
  a owl:Class ;
  qudt:description """When the temperature of a substance changes, the energy that is stored in the intermolecular bonds between atoms changes. When the stored energy increases, so does the length of the molecular bonds. As a result, solids typically expand in response to heating and contract on cooling; this dimensional response to temperature change is expressed by its coefficient of thermal expansion.



Different coefficients of thermal expansion can be defined for a substance depending on whether the expansion is measured by:



    * linear thermal expansion

    * area thermal expansion

    * volumetric thermal expansion



These characteristics are closely related. The volumetric thermal expansion coefficient can be defined for both liquids and solids. The linear thermal expansion can only be defined for solids, and is common in engineering applications.



Some substances expand when cooled, such as freezing water, so they have negative thermal expansion coefficients. [Wikipedia]"""^^rdf:HTML ;
  rdfs:isDefinedBy <http://qudt.org/2.0/schema/qudt/science> ;
  rdfs:isDefinedBy qudt:science ;
  rdfs:label "Linear Thermal Expansion Unit" ;
  rdfs:subClassOf qudt:ThermalExpansionUnit ;
  rdfs:subClassOf [
      a owl:Restriction ;
      owl:hasValue quantitykind:LinearThermalExpansion ;
      owl:onProperty qudt:hasQuantityKind ;
    ] ;
.
qudt:LinearVelocityUnit
  a owl:Class ;
  qudt:description "Linear Velocity units measure change of length per unit time. Examples include meters per second, miles per hour, knots, etc. "^^rdf:HTML ;
  rdfs:isDefinedBy <http://qudt.org/2.0/schema/qudt/science> ;
  rdfs:isDefinedBy qudt:science ;
  rdfs:label "Linear Velocity Unit" ;
  rdfs:subClassOf qudt:VelocityUnit ;
  rdfs:subClassOf [
      a owl:Restriction ;
      owl:hasValue quantitykind:LinearVelocity ;
      owl:onProperty qudt:hasQuantityKind ;
    ] ;
  skos:exactMatch <http://dbpedia.org/resource/Category:Units_of_velocity> ;
.
qudt:LoadsAnalysisQuantityKind
  a owl:Class ;
  dct:description "A sub-type of 'Structures And Mechanics Quantity Kind'. Detailed desciption to be provided in a future version." ;
  rdfs:isDefinedBy <http://qudt.org/2.0/schema/qudt/science> ;
  rdfs:isDefinedBy qudt:science ;
  rdfs:label "Loads Analysis Quantity Kind" ;
  rdfs:subClassOf qudt:StructuresAndMechanicsQuantityKind ;
.
qudt:LoadsQuantityKind
  a owl:Class ;
  dct:description "A sub-type of 'Space System Engineering Quantity Kind'. Detailed desciption to be provided in a future version." ;
  rdfs:isDefinedBy <http://qudt.org/2.0/schema/qudt/science> ;
  rdfs:isDefinedBy qudt:science ;
  rdfs:label "Loads Quantity Kind" ;
  rdfs:subClassOf qudt:SpaceSystemEngineeringQuantityKind ;
.
qudt:LogarithmicUnit
  a owl:Class ;
  qudt:description "Logarithmic units are abstract mathematical units that can be used to express any quantities (physical or mathematical) that are defined on a logarithmic scale, that is, as being proportional to the value of a logarithm function. Examples of logarithmic units include common units of information and entropy, such as the bit, and the byte, as well as units of relative signal strength magnitude such as the decibel."^^rdf:HTML ;
  rdfs:isDefinedBy <http://qudt.org/2.0/schema/qudt/science> ;
  rdfs:isDefinedBy qudt:science ;
  rdfs:label "Logarithmic Unit" ;
  rdfs:subClassOf qudt:MathsUnit ;
.
qudt:LogisticsQuantityKind
  a owl:Class ;
  dct:description "A sub-type of 'Management Quantity Kind'. Detailed desciption to be provided in a future version." ;
  rdfs:isDefinedBy <http://qudt.org/2.0/schema/qudt/science> ;
  rdfs:isDefinedBy qudt:science ;
  rdfs:label "Logistics Quantity Kind" ;
  rdfs:subClassOf qudt:ManagementQuantityKind ;
.
qudt:LuminanceUnit
  a owl:Class ;
  dct:description "A sub-type of 'Photometry Unit'. Detailed desciption to be provided in a future version." ;
  rdfs:isDefinedBy <http://qudt.org/2.0/schema/qudt/science> ;
  rdfs:isDefinedBy qudt:science ;
  rdfs:label "Luminance Unit" ;
  rdfs:subClassOf qudt:PhotometryUnit ;
  rdfs:subClassOf [
      a owl:Restriction ;
      owl:hasValue quantitykind:Luminance ;
      owl:onProperty qudt:hasQuantityKind ;
    ] ;
  skos:exactMatch <http://dbpedia.org/resource/Category:Units_of_illuminance> ;
.
qudt:LuminousEfficacyUnit
  a owl:Class ;
  dct:description "A sub-type of 'Photometry Unit'. Detailed desciption to be provided in a future version." ;
  rdfs:isDefinedBy <http://qudt.org/2.0/schema/qudt/science> ;
  rdfs:isDefinedBy qudt:science ;
  rdfs:label "Luminous Efficacy Unit" ;
  rdfs:subClassOf qudt:PhotometryUnit ;
.
qudt:LuminousEnergyUnit
  a owl:Class ;
  dct:description "A sub-type of 'Photometry Unit'. Detailed desciption to be provided in a future version." ;
  rdfs:isDefinedBy <http://qudt.org/2.0/schema/qudt/science> ;
  rdfs:isDefinedBy qudt:science ;
  rdfs:label "Luminous Energy Unit" ;
  rdfs:subClassOf qudt:PhotometryUnit ;
  skos:exactMatch <http://dbpedia.org/resource/Category:Units_of_luminous_energy> ;
.
qudt:LuminousFluxUnit
  a owl:Class ;
  dct:description "A sub-type of 'Photometry Unit'. Detailed desciption to be provided in a future version." ;
  rdfs:isDefinedBy <http://qudt.org/2.0/schema/qudt/science> ;
  rdfs:isDefinedBy qudt:science ;
  rdfs:label "Luminous Flux Unit" ;
  rdfs:subClassOf qudt:PhotometryUnit ;
  rdfs:subClassOf [
      a owl:Restriction ;
      owl:hasValue quantitykind:LuminousFlux ;
      owl:onProperty qudt:hasQuantityKind ;
    ] ;
  skos:exactMatch <http://dbpedia.org/resource/Category:Units_of_luminous_flux> ;
.
qudt:LuminousIntensityUnit
  a owl:Class ;
  dct:description "A sub-type of 'Photometry Unit'. Detailed desciption to be provided in a future version." ;
  rdfs:isDefinedBy <http://qudt.org/2.0/schema/qudt/science> ;
  rdfs:isDefinedBy qudt:science ;
  rdfs:label "Luminous Intensity Unit" ;
  rdfs:subClassOf qudt:PhotometryUnit ;
  rdfs:subClassOf [
      a owl:Restriction ;
      owl:hasValue quantitykind:LuminousIntensity ;
      owl:onProperty qudt:hasQuantityKind ;
    ] ;
  skos:exactMatch <http://dbpedia.org/resource/Category:Units_of_luminous_intensity> ;
.
qudt:MagneticFieldStrengthUnit
  a owl:Class ;
  qudt:description """A magnetic field is a vector field that permeates space and which can exert a magnetic force on moving electric charges and on magnetic dipoles (such as permanent magnets). [Wikipedia] The strength of a magnetic field at a point in space is the magnitude of the field vector at that point.



This class contains the following instance(s): \"Ampere per meter\", \"Ampere turn per inch\", \"Ampere turn per meter\", \"Oersted\"."""^^rdf:HTML ;
  rdfs:isDefinedBy <http://qudt.org/2.0/schema/qudt/science> ;
  rdfs:isDefinedBy qudt:science ;
  rdfs:label "Magnetic Field Strength Unit" ;
  rdfs:subClassOf qudt:ElectricityAndMagnetismUnit ;
  rdfs:subClassOf [
      a owl:Restriction ;
      owl:hasValue quantitykind:AuxillaryMagneticField ;
      owl:onProperty qudt:hasQuantityKind ;
    ] ;
  skos:exactMatch <http://dbpedia.org/resource/Category:Units_of_magnetic_induction> ;
.
qudt:MagneticFluxDensityUnit
  a owl:Class ;
  dct:description "A sub-type of 'Electricity And Magnetism Unit'. Detailed desciption to be provided in a future version." ;
  rdfs:isDefinedBy <http://qudt.org/2.0/schema/qudt/science> ;
  rdfs:isDefinedBy qudt:science ;
  rdfs:label "Magnetic Flux Density Unit" ;
  rdfs:subClassOf qudt:ElectricityAndMagnetismUnit ;
  rdfs:subClassOf [
      a owl:Restriction ;
      owl:hasValue quantitykind:MagneticFluxDensity ;
      owl:onProperty qudt:hasQuantityKind ;
    ] ;
  skos:exactMatch <http://dbpedia.org/resource/Category:Units_of_magnetic_flux_density> ;
.
qudt:MagneticFluxUnit
  a owl:Class ;
  qudt:description "Magnetic flux is a measure of quantity of magnetism, taking into account the strength and the extent of a magnetic field. The SI unit of magnetic flux is the weber (in derived units: volt-seconds), and the unit of magnetic field is the weber per square meter, or tesla."^^rdf:HTML ;
  rdfs:isDefinedBy <http://qudt.org/2.0/schema/qudt/science> ;
  rdfs:isDefinedBy qudt:science ;
  rdfs:label "Magnetic Flux Unit" ;
  rdfs:subClassOf qudt:ElectricityAndMagnetismUnit ;
  rdfs:subClassOf [
      a owl:Restriction ;
      owl:hasValue quantitykind:MagneticFlux ;
      owl:onProperty qudt:hasQuantityKind ;
    ] ;
  skos:exactMatch <http://dbpedia.org/resource/Category:Units_of_magnetic_flux> ;
.
qudt:MagneticMomentUnit
  a owl:Class ;
  qudt:description "The unit for magnetic moment is not a base unit in the International System of Units (SI) and it can be represented in more than one way. For example, in the current loop definition, the area is measured in square meters and I is measured in amperes, so the magnetic moment is measured in ampere–square meters ($A m^2$). In the equation for torque on a moment, the torque is measured in joules and the magnetic field in tesla, so the moment is measured in Joules per Tesla ($J \\cdot T^{−1}$)."^^rdf:HTML ;
  rdfs:isDefinedBy <http://qudt.org/2.0/schema/qudt/science> ;
  rdfs:isDefinedBy qudt:science ;
  rdfs:label "Magnetic moment unit" ;
  rdfs:subClassOf qudt:ElectricityAndMagnetismUnit ;
  prov:wasInformedBy <http://en.wikipedia.org/wiki/Magnetic_moment> ;
.
qudt:MagnetomotiveForceUnit
  a owl:Class ;
  qudt:description """Magnetomotive force is any physical cause that produces magnetic flux. In other words, it is a field of magnetism (measured in tesla) that has area (measured in square meters), so that (Tesla)(Area)= Flux. It is analogous to electromotive force or voltage in electricity. MMF usually describes electric wire coils in a way so scientists can measure or predict the actual force a wire coil can generate. [Wikipedia]



This class contains the following instance(s): \"Ampere turn\", \"Gilbert\", \"Oersted centimeter\", \"Unit pole\"."""^^rdf:HTML ;
  rdfs:isDefinedBy <http://qudt.org/2.0/schema/qudt/science> ;
  rdfs:isDefinedBy qudt:science ;
  rdfs:label "Magnetomotive Force Unit" ;
  rdfs:subClassOf qudt:ElectricityAndMagnetismUnit ;
  rdfs:subClassOf [
      a owl:Restriction ;
      owl:hasValue quantitykind:MagnetomotiveForce ;
      owl:onProperty qudt:hasQuantityKind ;
    ] ;
.
qudt:ManagementQuantityKind
  a owl:Class ;
  dct:description "A sub-type of 'Quantity Kind'. Detailed desciption to be provided in a future version." ;
  rdfs:isDefinedBy <http://qudt.org/2.0/schema/qudt/science> ;
  rdfs:isDefinedBy qudt:science ;
  rdfs:label "Management Quantity Kind" ;
  rdfs:subClassOf qudt:QuantityKind ;
.
qudt:MassAmountOfSubstanceTemperatureUnit
  a owl:Class ;
  dct:description "A sub-type of 'Chemistry Unit'. Detailed desciption to be provided in a future version." ;
  rdfs:isDefinedBy <http://qudt.org/2.0/schema/qudt/science> ;
  rdfs:isDefinedBy qudt:science ;
  rdfs:label "Mass Amount Of Substance Temperature Unit" ;
  rdfs:subClassOf qudt:ChemistryUnit ;
  rdfs:subClassOf [
      a owl:Restriction ;
      owl:hasValue quantitykind:MassAmountOfSubstanceTemperature ;
      owl:onProperty qudt:hasQuantityKind ;
    ] ;
.
qudt:MassAmountOfSubstanceUnit
  a owl:Class ;
  dct:description "A sub-type of 'Chemistry Unit'. Detailed desciption to be provided in a future version." ;
  rdfs:isDefinedBy <http://qudt.org/2.0/schema/qudt/science> ;
  rdfs:isDefinedBy qudt:science ;
  rdfs:label "Mass Amount Of Substance Unit" ;
  rdfs:subClassOf qudt:ChemistryUnit ;
  rdfs:subClassOf [
      a owl:Restriction ;
      owl:hasValue quantitykind:MassAmountOfSubstance ;
      owl:onProperty qudt:hasQuantityKind ;
    ] ;
.
qudt:MassPerAreaUnit
  a owl:Class ;
  dct:description "A sub-type of 'Mass Unit'. Detailed desciption to be provided in a future version." ;
  rdfs:isDefinedBy <http://qudt.org/2.0/schema/qudt/science> ;
  rdfs:isDefinedBy qudt:science ;
  rdfs:label "Mass Per Area Unit" ;
  rdfs:subClassOf qudt:MassUnit ;
  rdfs:subClassOf [
      a owl:Restriction ;
      owl:hasValue quantitykind:MassPerArea ;
      owl:onProperty qudt:hasQuantityKind ;
    ] ;
.
qudt:MassPerLengthUnit
  a owl:Class ;
  dct:description "A sub-type of 'Mass Unit'. Detailed desciption to be provided in a future version." ;
  rdfs:isDefinedBy <http://qudt.org/2.0/schema/qudt/science> ;
  rdfs:isDefinedBy qudt:science ;
  rdfs:label "Mass Per Length Unit" ;
  rdfs:subClassOf qudt:MassUnit ;
  rdfs:subClassOf [
      a owl:Restriction ;
      owl:hasValue quantitykind:MassPerLength ;
      owl:onProperty qudt:hasQuantityKind ;
    ] ;
.
qudt:MassPerTimeUnit
  a owl:Class ;
  dct:description "A sub-type of 'Mass Unit'. Detailed desciption to be provided in a future version." ;
  rdfs:isDefinedBy <http://qudt.org/2.0/schema/qudt/science> ;
  rdfs:isDefinedBy qudt:science ;
  rdfs:label "Mass Per Time Unit" ;
  rdfs:subClassOf qudt:MassUnit ;
  rdfs:subClassOf [
      a owl:Restriction ;
      owl:hasValue quantitykind:MassPerTime ;
      owl:onProperty qudt:hasQuantityKind ;
    ] ;
.
qudt:MassPerVolumeUnit
  a owl:Class ;
  dct:description "A sub-type of 'Mass Unit'. Detailed desciption to be provided in a future version." ;
  rdfs:isDefinedBy <http://qudt.org/2.0/schema/qudt/science> ;
  rdfs:isDefinedBy qudt:science ;
  rdfs:label "Mass Per Volume Unit" ;
  rdfs:subClassOf qudt:MassUnit ;
  rdfs:subClassOf [
      a owl:Restriction ;
      owl:hasValue quantitykind:Density ;
      owl:onProperty qudt:hasQuantityKind ;
    ] ;
  skos:exactMatch <http://dbpedia.org/resource/Category:Units_of_density> ;
.
qudt:MassPropertyQuantityKind
  a owl:Class ;
  dct:description "A sub-type of 'Classical Mechanics Quantity Kind'. Detailed desciption to be provided in a future version." ;
  rdfs:isDefinedBy <http://qudt.org/2.0/schema/qudt/science> ;
  rdfs:isDefinedBy qudt:science ;
  rdfs:label "Mass property quantity kind" ;
  rdfs:subClassOf qudt:ClassicalMechanicsQuantityKind ;
.
qudt:MassQuantityKind
  a owl:Class ;
  dct:description "A sub-type of 'Classical Mechanics Quantity Kind'. Detailed desciption to be provided in a future version." ;
  rdfs:isDefinedBy <http://qudt.org/2.0/schema/qudt/science> ;
  rdfs:isDefinedBy qudt:science ;
  rdfs:label "Mass Properties Quantity Kind" ;
  rdfs:subClassOf qudt:ClassicalMechanicsQuantityKind ;
.
qudt:MassTemperatureUnit
  a owl:Class ;
  dct:description "A sub-type of 'Thermodynamics Unit'. Detailed desciption to be provided in a future version." ;
  rdfs:isDefinedBy <http://qudt.org/2.0/schema/qudt/science> ;
  rdfs:isDefinedBy qudt:science ;
  rdfs:label "Mass Temperature Unit" ;
  rdfs:subClassOf qudt:ThermodynamicsUnit ;
  rdfs:subClassOf [
      a owl:Restriction ;
      owl:hasValue quantitykind:MassTemperature ;
      owl:onProperty qudt:hasQuantityKind ;
    ] ;
.
qudt:MassUnit
  a owl:Class ;
  dct:description "A sub-type of 'Classical Mechanics Unit'. Detailed desciption to be provided in a future version." ;
  rdfs:isDefinedBy <http://qudt.org/2.0/schema/qudt/science> ;
  rdfs:isDefinedBy qudt:science ;
  rdfs:label "Mass Unit" ;
  rdfs:subClassOf qudt:ClassicalMechanicsUnit ;
  rdfs:subClassOf [
      a owl:Restriction ;
      owl:hasValue quantitykind:Mass ;
      owl:onProperty qudt:hasQuantityKind ;
    ] ;
  skos:exactMatch <http://dbpedia.org/resource/Category:Units_of_mass> ;
.
qudt:MaterialScienceUnit
  a owl:Class ;
  dct:description "A sub-type of 'Science unit'. Detailed desciption to be provided in a future version." ;
  qudt:fieldCode "500" ;
  rdfs:isDefinedBy <http://qudt.org/2.0/schema/qudt/science> ;
  rdfs:isDefinedBy qudt:science ;
  rdfs:label "Materials unit" ;
  rdfs:subClassOf qudt:ScienceUnit ;
  skos:prefLabel "Material Science Unit" ;
.
qudt:MaterialsScienceQuantityKind
  a owl:Class ;
  dct:description "A sub-type of 'Science quantity kind'. Detailed desciption to be provided in a future version." ;
  rdfs:isDefinedBy <http://qudt.org/2.0/schema/qudt/science> ;
  rdfs:isDefinedBy qudt:science ;
  rdfs:label "Materials Science Quantity Kind" ;
  rdfs:subClassOf qudt:ScienceQuantityKind ;
.
qudt:MathFunctionType
  dct:description "A sub-type of 'QUDT Concept'. Detailed desciption to be provided in a future version." ;
.
qudt:MathsFunctionType
  a owl:Class ;
  rdfs:isDefinedBy <http://qudt.org/2.0/schema/qudt/science> ;
  rdfs:isDefinedBy qudt:science ;
  rdfs:label "Maths Function Type" ;
  rdfs:subClassOf qudt:EnumeratedValue ;
  skos:prefLabel "Maths Algorithmn Type" ;
.
qudt:MathsUnit
  a owl:Class ;
  qudt:description "Units that are have only a pure mathematical basis."^^rdf:HTML ;
  qudt:fieldCode "130" ;
  rdfs:isDefinedBy <http://qudt.org/2.0/schema/qudt/science> ;
  rdfs:isDefinedBy qudt:science ;
  rdfs:label "Maths unit" ;
  rdfs:subClassOf qudt:DomainSpecificUnit ;
  skos:prefLabel "Maths unit" ;
.
qudt:MechanicalEngineeringQuantityKind
  a owl:Class ;
  dct:description "A sub-type of 'Engineering quantity kind'. Detailed desciption to be provided in a future version." ;
  rdfs:isDefinedBy <http://qudt.org/2.0/schema/qudt/science> ;
  rdfs:isDefinedBy qudt:science ;
  rdfs:label "Mechanical Engineering Quantity Kind" ;
  rdfs:subClassOf qudt:EngineeringQuantityKind ;
  skos:exactMatch <http://dbpedia.org/resource/Mechanics> ;
.
qudt:MechanicsQuantityKind
  a owl:Class ;
  dct:description "Mechanics is the branch of science concerned with the behavior of physical bodies when subjected to forces or displacements, and the subsequent effects of the bodies on their environment. The foundation is known as classical mechanics. It is a branch of classical physics that deals with the particles that are moving either with less velocity or that are at rest. It can also be defined as a branch of science which deals with the motion and force of the particular object." ;
  rdfs:isDefinedBy <http://qudt.org/2.0/schema/qudt/science> ;
  rdfs:isDefinedBy qudt:science ;
  rdfs:label "Mechanics Quantity Kind" ;
  rdfs:subClassOf qudt:PhysicsQuantityKind ;
  prov:wasInfluencedBy <http://en.wikipedia.org/wiki/Mechanics> ;
.
qudt:MechanicsUnit
  a owl:Class ;
  dct:description "A sub-type of 'Physics Unit'. Detailed desciption to be provided in a future version." ;
  qudt:fieldCode "740" ;
  rdfs:isDefinedBy <http://qudt.org/2.0/schema/qudt/science> ;
  rdfs:isDefinedBy qudt:science ;
  rdfs:label "Mechanics Unit" ;
  rdfs:subClassOf qudt:PhysicsUnit ;
  rdfs:subClassOf [
      a owl:Restriction ;
      owl:allValuesFrom qudt:MechanicalEngineeringQuantityKind ;
      owl:onProperty qudt:hasQuantityKind ;
    ] ;
  owl:equivalentClass [
      a owl:Restriction ;
      owl:allValuesFrom qudt:MechanicalEngineeringQuantityKind ;
      owl:onProperty qudt:hasQuantityKind ;
    ] ;
.
qudt:MechanismsQuantityKind
  a owl:Class ;
  dct:description "A sub-type of 'Structures And Mechanics Quantity Kind'. Detailed desciption to be provided in a future version." ;
  rdfs:isDefinedBy <http://qudt.org/2.0/schema/qudt/science> ;
  rdfs:isDefinedBy qudt:science ;
  rdfs:label "Mechanisms Quantity Kind" ;
  rdfs:subClassOf qudt:StructuresAndMechanicsQuantityKind ;
.
qudt:MedicalInformaticsQuantityKind
  a owl:Class ;
  dct:description "A sub-type of 'Infomatics quantity kind'. Detailed desciption to be provided in a future version." ;
  rdfs:isDefinedBy <http://qudt.org/2.0/schema/qudt/science> ;
  rdfs:isDefinedBy qudt:science ;
  rdfs:label "Medical Informatics Quantity Kind" ;
  rdfs:subClassOf qudt:InformaticsQuantityKind ;
.
qudt:MedicineQuantityKind
  a owl:Class ;
  dct:description "A sub-type of 'Life Sciences Quantity Kind'. Detailed desciption to be provided in a future version." ;
  rdfs:isDefinedBy <http://qudt.org/2.0/schema/qudt/science> ;
  rdfs:isDefinedBy qudt:science ;
  rdfs:label "Medicine Quantity Kind" ;
  rdfs:subClassOf qudt:LifeSciencesQuantityKind ;
.
qudt:MeteorologyQuantityKind
  a owl:Class ;
  dct:description "A sub-type of 'Atmospheric Science Quantity Kind'. Detailed desciption to be provided in a future version." ;
  dct:description """Meteorology is the interdisciplinary scientific study of the atmosphere. Meteorological phenomena are observable weather events which illuminate, and are explained by the science of meteorology. Those events are bound by the variables that exist in Earth's atmosphere; temperature, air pressure, water vapor, and the gradients and interactions of each variable, and how they change in time. Different spatial scales are studied to determine how systems on local, regional, and global levels impact weather and climatology.
Meteorology, climatology, atmospheric physics, and atmospheric chemistry are sub-disciplines of the atmospheric sciences. 

Meteorology and hydrology compose the interdisciplinary field of hydrometeorology. Interactions between Earth's atmosphere and the oceans are part of coupled ocean-atmosphere studies. Meteorology has application in many diverse fields such as the military, energy production, transport, agriculture and construction.""" ;
  rdfs:isDefinedBy <http://qudt.org/2.0/schema/qudt/science> ;
  rdfs:isDefinedBy qudt:science ;
  rdfs:label "Meteorology Quantity Kind" ;
  rdfs:subClassOf qudt:AtmosphericScienceQuantityKind ;
  prov:wasInfluencedBy <http://en.wikipedia.org/wiki/Meteorology> ;
.
qudt:MicrobialFormationUnit
  a owl:Class ;
  dct:description "A sub-type of 'Biomedical Unit'. Detailed desciption to be provided in a future version." ;
  rdfs:isDefinedBy <http://qudt.org/2.0/schema/qudt/science> ;
  rdfs:isDefinedBy qudt:science ;
  rdfs:label "Microbial Formation Unit" ;
  rdfs:subClassOf qudt:BiomedicalUnit ;
  rdfs:subClassOf [
      a owl:Restriction ;
      owl:hasValue quantitykind:MicrobialFormation ;
      owl:onProperty qudt:hasQuantityKind ;
    ] ;
.
qudt:MissionPlanningQuantityKind
  a owl:Class ;
  dct:description "A sub-type of 'Management Quantity Kind' and 'System Engineering Quantity Kind'. Detailed desciption to be provided in a future version." ;
  rdfs:isDefinedBy <http://qudt.org/2.0/schema/qudt/science> ;
  rdfs:isDefinedBy qudt:science ;
  rdfs:label "Mission Planning Quantity Kind" ;
  rdfs:subClassOf qudt:ManagementQuantityKind ;
  rdfs:subClassOf qudt:SystemEngineeringQuantityKind ;
.
qudt:ModelingAndSimulationQuantityKind
  a owl:Class ;
  dct:description "A sub-type of 'System Engineering Quantity Kind'. Detailed desciption to be provided in a future version." ;
  rdfs:isDefinedBy <http://qudt.org/2.0/schema/qudt/science> ;
  rdfs:isDefinedBy qudt:science ;
  rdfs:label "Modeling and Simulation Quantity Kind" ;
  rdfs:subClassOf qudt:SystemEngineeringQuantityKind ;
.
qudt:MolalConcentrationUnit
  a owl:Class ;
  qudt:citation "http://chemistry.about.com/od/chemistryterminology/a/What-Is-The-Difference-Between-Molarity-And-Molality.htm" ;
  qudt:citation "http://en.wikipedia.org/wiki/Molality" ;
  qudt:description "$\\textbf{Molality}$, also called $\\textbf{molal concentration}$, is a measure of the concentration of a solute in a solution in terms of amount of substance in a specified amount of mass of the solvent. This contrasts with the definition of molarity which is based on a specified volume of solution. A commonly used unit for molality used in chemistry is $ mol/kg $. A solution of concentration $1\\,mol/kg $ is also sometimes denoted as $1\\,molal$."^^rdf:HTML ;
  rdfs:isDefinedBy <http://qudt.org/2.0/schema/qudt/science> ;
  rdfs:isDefinedBy qudt:science ;
  rdfs:label "Molal Concentration Unit" ;
  rdfs:subClassOf qudt:ConcentrationUnit ;
  rdfs:subClassOf [
      a owl:Restriction ;
      owl:hasValue quantitykind:AmountOfSubstancePerUnitMass ;
      owl:onProperty qudt:hasQuantityKind ;
    ] ;
.
qudt:MolarConcentrationUnit
  a owl:Class ;
  dct:description "A sub-type of 'Concentration Unit'. Detailed desciption to be provided in a future version." ;
  rdfs:isDefinedBy <http://qudt.org/2.0/schema/qudt/science> ;
  rdfs:isDefinedBy qudt:science ;
  rdfs:label "Molar Concentration Unit" ;
  rdfs:subClassOf qudt:ConcentrationUnit ;
  rdfs:subClassOf [
      a owl:Restriction ;
      owl:hasValue quantitykind:AmountOfSubstancePerUnitVolume ;
      owl:onProperty qudt:hasQuantityKind ;
    ] ;
.
qudt:MolarEnergyUnit
  a owl:Class ;
  dct:description "A sub-type of 'Chemistry Unit'. Detailed desciption to be provided in a future version." ;
  rdfs:isDefinedBy <http://qudt.org/2.0/schema/qudt/science> ;
  rdfs:isDefinedBy qudt:science ;
  rdfs:label "Molar Energy Unit" ;
  rdfs:subClassOf qudt:ChemistryUnit ;
  rdfs:subClassOf [
      a owl:Restriction ;
      owl:hasValue quantitykind:MolarEnergy ;
      owl:onProperty qudt:hasQuantityKind ;
    ] ;
.
qudt:MolarHeatCapacityUnit
  a owl:Class ;
  dct:description "A sub-type of 'Thermodynamics Unit'. Detailed desciption to be provided in a future version." ;
  rdfs:isDefinedBy <http://qudt.org/2.0/schema/qudt/science> ;
  rdfs:isDefinedBy qudt:science ;
  rdfs:label "Molar Heat Capacity Unit" ;
  rdfs:subClassOf qudt:ThermodynamicsUnit ;
  rdfs:subClassOf [
      a owl:Restriction ;
      owl:hasValue quantitykind:MolarHeatCapacity ;
      owl:onProperty qudt:hasQuantityKind ;
    ] ;
.
qudt:MomentumUnit
  a owl:Class ;
  dct:description "A sub-type of 'Classical Mechanics Unit'. Detailed desciption to be provided in a future version." ;
  rdfs:isDefinedBy <http://qudt.org/2.0/schema/qudt/science> ;
  rdfs:isDefinedBy qudt:science ;
  rdfs:label "Momentum Unit" ;
  rdfs:subClassOf qudt:ClassicalMechanicsUnit ;
.
qudt:NaturalUnit
  rdfs:isDefinedBy <http://qudt.org/schema/qudt> ;
.
qudt:NominalScale
  a owl:Class ;
  qudt:description "mode, Chi-squared &  One to One (equality (=)) & standard set structure (unordered)"^^rdf:HTML ;
  rdfs:isDefinedBy <http://qudt.org/2.0/schema/qudt/science> ;
  rdfs:isDefinedBy qudt:science ;
  rdfs:label "Nominal scale" ;
  rdfs:subClassOf qudt:Scale ;
  skos:prefLabel "Nominal scale" ;
.
qudt:NonSI-Unit
  rdfs:isDefinedBy <http://qudt.org/schema/qudt> ;
.
qudt:NotUsedWithSI-Unit
  rdfs:isDefinedBy <http://qudt.org/schema/qudt> ;
.
qudt:NuclearPhysicsQuantityKind
  a owl:Class ;
  dct:description "A sub-type of 'Quantum Mechanics Quantity Kind'. Detailed desciption to be provided in a future version." ;
  rdfs:isDefinedBy <http://qudt.org/2.0/schema/qudt/science> ;
  rdfs:isDefinedBy qudt:science ;
  rdfs:label "Nuclear Physics Quantity Kind" ;
  rdfs:subClassOf qudt:QuantumMechanicsQuantityKind ;
.
qudt:NutritionQuantityKind
  a owl:Class ;
  dct:description "A sub-type of 'Life Sciences Quantity Kind'. Detailed desciption to be provided in a future version." ;
  rdfs:isDefinedBy <http://qudt.org/2.0/schema/qudt/science> ;
  rdfs:isDefinedBy qudt:science ;
  rdfs:label "Nutrition Quantity Kind" ;
  rdfs:subClassOf qudt:LifeSciencesQuantityKind ;
.
qudt:OpticsQuantityKind
  a owl:Class ;
  dct:description "A sub-type of 'Light quantity kind' and 'Physics Quantity Kind'. Detailed desciption to be provided in a future version." ;
  rdfs:isDefinedBy <http://qudt.org/2.0/schema/qudt/science> ;
  rdfs:isDefinedBy qudt:science ;
  rdfs:label "Optics" ;
  rdfs:subClassOf qudt:LightQuantityKind ;
  rdfs:subClassOf qudt:PhysicsQuantityKind ;
  skos:exactMatch <http://dbpedia.org/resource/Light> ;
.
qudt:OpticsUnit
  a owl:Class ;
  dct:description "A sub-type of 'Electricity And Magnetism Unit'. Detailed desciption to be provided in a future version." ;
  rdfs:isDefinedBy <http://qudt.org/2.0/schema/qudt/science> ;
  rdfs:isDefinedBy qudt:science ;
  rdfs:label "Light Unit" ;
  rdfs:subClassOf qudt:ElectricityAndMagnetismUnit ;
  rdfs:subClassOf [
      a owl:Restriction ;
      owl:allValuesFrom qudt:OpticsQuantityKind ;
      owl:onProperty qudt:hasQuantityKind ;
    ] ;
  owl:equivalentClass [
      a owl:Restriction ;
      owl:allValuesFrom qudt:OpticsQuantityKind ;
      owl:onProperty qudt:hasQuantityKind ;
    ] ;
.
qudt:OrbitalMechanicsQuantityKind
  a owl:Class ;
  dct:description "A sub-type of 'Astrodynamics Quantity Kind'. Detailed desciption to be provided in a future version." ;
  dct:description """\"Orbital Mechanics} or \\textit{astrodynamics\" is the application of ballistics and celestial mechanics to the practical problems concerning the motion of rockets and other spacecraft. The motion of these objects is usually calculated from Newton's laws of motion and Newton's law of universal gravitation. It is a core discipline within space mission design and control. Celestial mechanics treats more broadly the orbital dynamics of systems under the influence of gravity, including both spacecraft and natural astronomical bodies such as star systems, planets, moons, and comets. 

Orbital mechanics focuses on spacecraft trajectories, including orbital maneuvers, orbit plane changes, and interplanetary transfers, and is used by mission planners to predict the results of propulsive maneuvers. General relativity is a more exact theory than Newton's laws for calculating orbits, and is sometimes necessary for greater accuracy or in high-gravity situations (such as orbits close to the Sun).""" ;
  rdfs:isDefinedBy <http://qudt.org/2.0/schema/qudt/science> ;
  rdfs:isDefinedBy qudt:science ;
  rdfs:label "Orbital Mechanics Quantity Kind" ;
  rdfs:subClassOf qudt:AstrodynamicsQuantityKind ;
  prov:wasInfluencedBy <http://en.wikipedia.org/wiki/Orbital_mechanics> ;
.
qudt:Organization
  dct:description "A sub-type of 'QUDT Concept'. Detailed desciption to be provided in a future version." ;
.
qudt:ParticlePhysicsQuantityKind
  a owl:Class ;
  dct:description "A sub-type of 'Quantum Mechanics Quantity Kind'. Detailed desciption to be provided in a future version." ;
  rdfs:isDefinedBy <http://qudt.org/2.0/schema/qudt/science> ;
  rdfs:isDefinedBy qudt:science ;
  rdfs:label "Particle physics Quantity Kind" ;
  rdfs:subClassOf qudt:QuantumMechanicsQuantityKind ;
.
qudt:PermeabilityUnit
  a owl:Class ;
  dct:description "A sub-type of 'Electricity And Magnetism Unit'. Detailed desciption to be provided in a future version." ;
  rdfs:isDefinedBy <http://qudt.org/2.0/schema/qudt/science> ;
  rdfs:isDefinedBy qudt:science ;
  rdfs:label "Permeability Unit" ;
  rdfs:subClassOf qudt:ElectricityAndMagnetismUnit ;
  rdfs:subClassOf [
      a owl:Restriction ;
      owl:hasValue quantitykind:Permeability ;
      owl:onProperty qudt:hasQuantityKind ;
    ] ;
  rdfs:subClassOf [
      a owl:Restriction ;
      owl:hasValue quantitykind:Permeability ;
      owl:onProperty qudt:hasQuantityKind ;
    ] ;
.
qudt:PermittivityUnit
  a owl:Class ;
  dct:description "A sub-type of 'Electricity And Magnetism Unit'. Detailed desciption to be provided in a future version." ;
  rdfs:isDefinedBy <http://qudt.org/2.0/schema/qudt/science> ;
  rdfs:isDefinedBy qudt:science ;
  rdfs:label "Permittivity Unit" ;
  rdfs:subClassOf qudt:ElectricityAndMagnetismUnit ;
  rdfs:subClassOf [
      a owl:Restriction ;
      owl:hasValue quantitykind:Permittivity ;
      owl:onProperty qudt:hasQuantityKind ;
    ] ;
.
qudt:PhotometryQuantityKind
  a owl:Class ;
  qudt:description "Photometry is the field that studies the measurement of electromagnetic radiation, including visible light. Note that light is also measured using the techniques of photometry, which deal with brightness as perceived by the human eye, rather than absolute power."^^rdf:HTML ;
  rdfs:isDefinedBy <http://qudt.org/2.0/schema/qudt/science> ;
  rdfs:isDefinedBy qudt:science ;
  rdfs:label "Photometry Quantity Kind" ;
  rdfs:subClassOf qudt:OpticsQuantityKind ;
.
qudt:PhotometryUnit
  a owl:Class ;
  dct:description "A sub-type of 'Light Unit'. Detailed desciption to be provided in a future version." ;
  rdfs:isDefinedBy <http://qudt.org/2.0/schema/qudt/science> ;
  rdfs:isDefinedBy qudt:science ;
  rdfs:label "Photometry Unit" ;
  rdfs:subClassOf qudt:OpticsUnit ;
.
qudt:PhysicsQuantityKind
  a owl:Class ;
  dct:description "The study of the laws that determine the structure of the universe with reference to the matter and energy of which it consists. It is concerned not with chemical changes that occur but with the forces that exist between objects and the interrelationship between matter and energy. Physics covers phenomena associated with heat, light, sound, electricity and magnetism, and mechanics. Since the turn of the century, quantum mechanics and relativistic physics have led to the growth of modern physics embracing atomic physics, nuclear physics, and particle physics. The physics of astronomical bodies and their interactions is known as astrophysics, the physics of the earth is known as geophysics, and the study of the physical aspects of biology is called biophysics. Each phenomenon of physics has \"Quantity Kinds\". These are paritioned according to their respective fields of knowledge." ;
  rdfs:isDefinedBy <http://qudt.org/2.0/schema/qudt/science> ;
  rdfs:isDefinedBy qudt:science ;
  rdfs:label "Physics Quantity Kind" ;
  rdfs:subClassOf qudt:ScienceQuantityKind ;
  prov:wasInfluencedBy <http://en.wikipedia.org/wiki/Physics> ;
  prov:wasInfluencedBy <http://www.oxfordreference.com/view/10.1093/acref/9780199233991.001.0001/acref-9780199233991-e-2324> ;
  prov:wasInfluencedBy <http://www.physicsforums.com> ;
.
qudt:PhysicsUnit
  a owl:Class ;
  dct:description "A sub-type of 'Science unit'. Detailed desciption to be provided in a future version." ;
  qudt:fieldCode "700" ;
  rdfs:isDefinedBy <http://qudt.org/2.0/schema/qudt/science> ;
  rdfs:isDefinedBy qudt:science ;
  rdfs:label "Physics Unit" ;
  rdfs:subClassOf qudt:ScienceUnit ;
.
qudt:PlaneAngleUnit
  a owl:Class ;
  dct:description "A sub-type of 'Angle unit'. Detailed desciption to be provided in a future version." ;
  rdfs:isDefinedBy <http://qudt.org/2.0/schema/qudt/science> ;
  rdfs:isDefinedBy qudt:science ;
  rdfs:label "Plane Angle Unit" ;
  rdfs:subClassOf qudt:AngleUnit ;
.
qudt:PlasmaDynamicsQuantityKind
  a owl:Class ;
  dct:description "A sub-type of 'Plasma Physics Quantity Kind'. Detailed desciption to be provided in a future version." ;
  dct:description "\"Plasma Dynamics} is a branch of \\textit{Plasma Physics\" which characterizes phenomena associated with the flows of nonequilibrium gases and plasmas. The field has relevance for the research and devlopment of systems of electric propulsion, hypersonic aerothermodynamics, flows involving very small length scales (MEMS devices), and materials processing (jets used in deposition thin films for advanced materials). Due to nonequilibrium effects, these flows cannot always be computed accurately with the macroscopic equations of gas dynamics and plasma physics. " ;
  rdfs:isDefinedBy <http://qudt.org/2.0/schema/qudt/science> ;
  rdfs:isDefinedBy qudt:science ;
  rdfs:label "Plasma Dynamics Quantity Kind" ;
  rdfs:subClassOf qudt:PlasmaPhysicsQuantityKind ;
  prov:wasInfluencedBy <http://en.wikipedia.org/wiki/Nonequilibrium_Gas_and_Plasma_Dynamics_Laboratory> ;
  prov:wasInfluencedBy <http://en.wikipedia.org/wiki/Plasma_physics> ;
.
qudt:PlasmaPhysicsQuantityKind
  a owl:Class ;
  dct:description "A sub-type of 'Physics Quantity Kind'. Detailed desciption to be provided in a future version." ;
  dct:description """In physics and chemistry, plasma is a state of matter similar to gas in which a certain portion of the particles is ionized. Heating a gas may ionize its molecules or atoms (reduce or increase the number of electrons in them), thus turning it into a plasma, which contains charged particles: positive ions and negative electrons or ions. 

Ionization can be induced by other means, such as strong electromagnetic field applied with a laser or microwave generator, and is accompanied by the dissociation of molecular bonds, if present. The presence of a non-negligible number of charge carriers makes the plasma electrically conductive so that it responds strongly to electromagnetic fields. 

Plasma, therefore, has properties quite unlike those of solids, liquids, or gases and is considered a distinct state of matter. Like gas, plasma does not have a definite shape or a definite volume unless enclosed in a container; unlike gas, under the influence of a magnetic field, it may form structures such as filaments, beams and double layers. Some common plasmas are found in stars and neon signs. In the universe, plasma is the most common state of matter for ordinary matter, most of which is in the rarefied intergalactic plasma (particularly intracluster medium) and in stars. Much of the understanding of plasmas has come from the pursuit of controlled nuclear fusion and fusion power, for which plasma physics provides the scientific basis.""" ;
  rdfs:isDefinedBy <http://qudt.org/2.0/schema/qudt/science> ;
  rdfs:isDefinedBy qudt:science ;
  rdfs:label "Plasma Physics Quantity Kind" ;
  rdfs:subClassOf qudt:PhysicsQuantityKind ;
  prov:wasInfluencedBy <http://en.wikipedia.org/wiki/Plasma_physics> ;
.
qudt:PowerPerAreaUnit
  a owl:Class ;
  dct:description "A sub-type of 'Power Units'. Detailed desciption to be provided in a future version." ;
  rdfs:isDefinedBy <http://qudt.org/2.0/schema/qudt/science> ;
  rdfs:isDefinedBy qudt:science ;
  rdfs:label "Power Per Area Unit" ;
  rdfs:subClassOf qudt:PowerUnit ;
  rdfs:subClassOf [
      a owl:Restriction ;
      owl:hasValue quantitykind:PowerPerArea ;
      owl:onProperty qudt:hasQuantityKind ;
    ] ;
.
qudt:PowerPerElectricChargeUnit
  a owl:Class ;
  qudt:description "The ratio of power to electric charge is proportional to the rate of change of electric potential."^^rdf:HTML ;
  rdfs:isDefinedBy <http://qudt.org/2.0/schema/qudt/science> ;
  rdfs:isDefinedBy qudt:science ;
  rdfs:label "Energy per Electric Charge Unit" ;
  rdfs:subClassOf qudt:ElectricityAndMagnetismUnit ;
.
qudt:PowerUnit
  a owl:Class ;
  qudt:description "In physics, power is the rate at which energy is transferred, used, or transformed. The unit of power is the joule per second (J/s). Energy transfer can be used to do work, so power is also the rate at which this work is performed. The integral of power over time defines the work done. Because this integral depends on the trajectory of the point of application of the force and torque, this calculation of work is said to be \"path dependent.\" The dimension of power is energy divided by time."^^rdf:HTML ;
  rdfs:isDefinedBy <http://qudt.org/2.0/schema/qudt/science> ;
  rdfs:isDefinedBy qudt:science ;
  rdfs:label "Power Units" ;
  rdfs:subClassOf qudt:MechanicsUnit ;
  rdfs:subClassOf [
      a owl:Restriction ;
      owl:hasValue quantitykind:ElectricPower ;
      owl:onProperty qudt:hasQuantityKind ;
    ] ;
  prov:wasInfluencedBy <http://en.wikipedia.org/wiki/Power_%28physics%29> ;
.
qudt:PrefixUnit
  dct:description "A sub-type of 'Unit'. Detailed desciption to be provided in a future version." ;
  rdfs:isDefinedBy <http://qudt.org/schema/qudt> ;
  rdfs:subClassOf [
      a owl:Restriction ;
      owl:hasValue quantitykind:Dimensionless ;
      owl:onProperty qudt:hasQuantityKind ;
    ] ;
  rdfs:subClassOf [
      a owl:Restriction ;
      owl:hasValue quantitykind:Dimensionless ;
      owl:onProperty qudt:hasQuantityKind ;
    ] ;
.
qudt:PressureOrStressRateUnit
  a owl:Class ;
  dct:description "A sub-type of 'Pressure unit'. Detailed desciption to be provided in a future version." ;
  rdfs:isDefinedBy <http://qudt.org/2.0/schema/qudt/science> ;
  rdfs:isDefinedBy qudt:science ;
  rdfs:label "Pressure or stress rate" ;
  rdfs:subClassOf qudt:PressureUnit ;
.
qudt:PressureOrStressUnit
  a owl:Class ;
  dct:description "A sub-type of 'Pressure unit'. Detailed desciption to be provided in a future version." ;
  rdfs:isDefinedBy <http://qudt.org/2.0/schema/qudt/science> ;
  rdfs:isDefinedBy qudt:science ;
  rdfs:label "Pressure Or Stress Unit" ;
  rdfs:subClassOf qudt:PressureUnit ;
  rdfs:subClassOf [
      a owl:Restriction ;
      owl:hasValue quantitykind:Stress ;
      owl:onProperty qudt:hasQuantityKind ;
    ] ;
  skos:exactMatch <http://dbpedia.org/resource/Category:Units_of_pressure> ;
.
qudt:PressureUnit
  a owl:Class ;
  dct:description "A sub-type of 'Mechanics Unit'. Detailed desciption to be provided in a future version." ;
  rdfs:isDefinedBy <http://qudt.org/2.0/schema/qudt/science> ;
  rdfs:isDefinedBy qudt:science ;
  rdfs:label "Pressure unit" ;
  rdfs:subClassOf qudt:MechanicsUnit ;
.
qudt:PressurizedSystemsQuantityKind
  a owl:Class ;
  dct:description "A sub-type of 'System Engineering Quantity Kind'. Detailed desciption to be provided in a future version." ;
  rdfs:isDefinedBy <http://qudt.org/2.0/schema/qudt/science> ;
  rdfs:isDefinedBy qudt:science ;
  rdfs:label "Pressurized systems" ;
  rdfs:subClassOf qudt:SystemEngineeringQuantityKind ;
.
qudt:ProportionalityConstant
  a owl:Class ;
  dct:description "A sub-type of 'Quantity'. Detailed desciption to be provided in a future version." ;
  dct:description """Two quantities proportional if they vary in such a way that one of the quantities is a constant multiple of the other. The multiple is the constant of proportionality between the two quantities. Constants of proportionality may be dimensioned in some quantity systems and dimensionless in others. For example, in the SI system, the permittivity of a vacuum has the dimensions L^-3 M^-1 T^4 I^2 and is measured in Farads per Meter; in the CGS-EMU system it has dimensions L^-2T^2 and is measured in Abfarads per Centimeter; in the CGS-ESU system it is dimensionless.



Constants of proportionality are important in the definition of systems of natural units, where units are chosen in order to make certain constants of proportionality dimensionless and equal to 1.""" ;
  rdfs:isDefinedBy <http://qudt.org/2.0/schema/qudt/science> ;
  rdfs:isDefinedBy qudt:science ;
  rdfs:label "Constant of Proportionality" ;
  rdfs:subClassOf qudt:Quantity ;
  skos:closeMatch <http://dbpedia.org/resource/Proportionality_%28mathematics%29> ;
.
qudt:PropulsionQuantityKind
  a owl:Class ;
  dct:description "A sub-type of 'Space System Engineering Quantity Kind'. Detailed desciption to be provided in a future version." ;
  rdfs:isDefinedBy <http://qudt.org/2.0/schema/qudt/science> ;
  rdfs:isDefinedBy qudt:science ;
  rdfs:label "Propulsion Quantity Kind" ;
  rdfs:subClassOf qudt:SpaceSystemEngineeringQuantityKind ;
.
qudt:QuantityType
  a owl:Class ;
  rdfs:isDefinedBy <http://qudt.org/2.0/schema/qudt/science> ;
  rdfs:isDefinedBy qudt:science ;
  rdfs:label "Quantity type" ;
  rdfs:subClassOf qudt:Enumeration ;
  rdfs:subClassOf [
      a owl:Restriction ;
      owl:allValuesFrom qudt:Unit ;
      owl:onProperty qudt:default ;
    ] ;
  rdfs:subClassOf [
      a owl:Restriction ;
      owl:allValuesFrom qudt:Unit ;
      owl:onProperty qudt:element ;
    ] ;
  rdfs:subClassOf [
      a owl:Restriction ;
      owl:cardinality "1"^^xsd:nonNegativeInteger ;
      owl:onProperty qudt:elementKind ;
    ] ;
.
qudt:QuantumMechanicsQuantityKind
  a owl:Class ;
  dct:description "A sub-type of 'Mechanics Quantity Kind'. Detailed desciption to be provided in a future version." ;
  dct:description "Quantum mechanics (QM – also known as quantum physics, or quantum theory) is a branch of physics dealing with physical phenomena where the action is on the order of the Planck constant. Quantum mechanics departs from classical mechanics primarily at the quantum realm of atomic and subatomic length scales. QM provides a mathematical description of much of the dual particle-like and wave-like behavior and interactions of energy and matter." ;
  rdfs:isDefinedBy <http://qudt.org/2.0/schema/qudt/science> ;
  rdfs:isDefinedBy qudt:science ;
  rdfs:label "Quantum Mechanics Quantity Kind" ;
  rdfs:subClassOf qudt:MechanicsQuantityKind ;
  prov:wasInfluencedBy <http://en.wikipedia.org/wiki/Quantum_mechanics> ;
  prov:wasInfluencedBy <http://www.oxfordreference.com/view/10.1093/acref/9780199233991.001.0001/acref-9780199233991-e-2483> ;
.
qudt:RF-PowerUnit
  rdfs:isDefinedBy <http://qudt.org/schema/qudt> ;
  rdfs:subClassOf [
      a owl:Restriction ;
      owl:hasValue quantitykind:RF-Power ;
      owl:onProperty qudt:hasQuantityKind ;
    ] ;
.
qudt:RadianceUnit
  a owl:Class ;
  dct:description "A sub-type of 'Thermodynamics Unit'. Detailed desciption to be provided in a future version." ;
  rdfs:isDefinedBy <http://qudt.org/2.0/schema/qudt/science> ;
  rdfs:isDefinedBy qudt:science ;
  rdfs:label "Radiance Unit" ;
  rdfs:subClassOf qudt:ThermodynamicsUnit ;
  rdfs:subClassOf [
      a owl:Restriction ;
      owl:hasValue quantitykind:PowerPerAreaAngle ;
      owl:onProperty qudt:hasQuantityKind ;
    ] ;
.
qudt:RadiantIntensityUnit
  a owl:Class ;
  dct:description "A sub-type of 'Radiometry Unit'. Detailed desciption to be provided in a future version." ;
  rdfs:isDefinedBy <http://qudt.org/2.0/schema/qudt/science> ;
  rdfs:isDefinedBy qudt:science ;
  rdfs:label "Radiant Intensity Unit" ;
  rdfs:subClassOf qudt:RadiometryUnit ;
  rdfs:subClassOf [
      a owl:Restriction ;
      owl:hasValue quantitykind:RadiantIntensity ;
      owl:onProperty qudt:hasQuantityKind ;
    ] ;
.
qudt:RadiationQuantityKind
  a owl:Class ;
  dct:description "A sub-type of 'Physics Quantity Kind'. Detailed desciption to be provided in a future version." ;
  rdfs:isDefinedBy <http://qudt.org/2.0/schema/qudt/science> ;
  rdfs:isDefinedBy qudt:science ;
  rdfs:label "Radiation Quantity Kind" ;
  rdfs:subClassOf qudt:PhysicsQuantityKind ;
.
qudt:RadiologyQuantityKind
  a owl:Class ;
  dct:description "A sub-type of 'Physics Quantity Kind'. Detailed desciption to be provided in a future version." ;
  rdfs:isDefinedBy <http://qudt.org/2.0/schema/qudt/science> ;
  rdfs:isDefinedBy qudt:science ;
  rdfs:label "Radiology" ;
  rdfs:subClassOf qudt:PhysicsQuantityKind ;
  skos:exactMatch <http://dbpedia.org/resource/Radiology> ;
.
qudt:RadiologyUnit
  a owl:Class ;
  dct:description "A sub-type of 'Physics Unit'. Detailed desciption to be provided in a future version." ;
  qudt:fieldCode "770" ;
  rdfs:isDefinedBy <http://qudt.org/2.0/schema/qudt/science> ;
  rdfs:isDefinedBy qudt:science ;
  rdfs:label "Radiology Unit" ;
  rdfs:subClassOf qudt:PhysicsUnit ;
  rdfs:subClassOf [
      a owl:Restriction ;
      owl:allValuesFrom qudt:RadiologyQuantityKind ;
      owl:onProperty qudt:hasQuantityKind ;
    ] ;
  owl:equivalentClass [
      a owl:Restriction ;
      owl:allValuesFrom qudt:RadiologyQuantityKind ;
      owl:onProperty qudt:hasQuantityKind ;
    ] ;
  skos:exactMatch <http://dbpedia.org/resource/Category:Units_of_radiation_dose> ;
.
qudt:RadiometryQuantityKind
  a owl:Class ;
  dct:description "A sub-type of 'Optics'. Detailed desciption to be provided in a future version." ;
  rdfs:isDefinedBy <http://qudt.org/2.0/schema/qudt/science> ;
  rdfs:isDefinedBy qudt:science ;
  rdfs:label "Radiometry Quantity Kind" ;
  rdfs:subClassOf qudt:OpticsQuantityKind ;
.
qudt:RadiometryUnit
  a owl:Class ;
  dct:description "A sub-type of 'Light Unit'. Detailed desciption to be provided in a future version." ;
  rdfs:isDefinedBy <http://qudt.org/2.0/schema/qudt/science> ;
  rdfs:isDefinedBy qudt:science ;
  rdfs:label "Radiometry Unit" ;
  rdfs:subClassOf qudt:OpticsUnit ;
.
qudt:RateOfReturnUnit
  rdfs:isDefinedBy <http://qudt.org/schema/qudt> ;
.
qudt:RequirementsEngineeringQuantityKind
  a owl:Class ;
  dct:description "A sub-type of 'System Engineering Quantity Kind'. Detailed desciption to be provided in a future version." ;
  rdfs:isDefinedBy <http://qudt.org/2.0/schema/qudt/science> ;
  rdfs:isDefinedBy qudt:science ;
  rdfs:label "Requirements Engineering Quantity Kind" ;
  rdfs:subClassOf qudt:SystemEngineeringQuantityKind ;
.
qudt:ResistanceUnit
  a owl:Class ;
  qudt:description "Electrical resistance is a ratio of the degree to which an object opposes an electric current through it, measured in ohms. Its reciprocal quantity is electrical conductance measured in siemens."^^rdf:HTML ;
  rdfs:isDefinedBy <http://qudt.org/2.0/schema/qudt/science> ;
  rdfs:isDefinedBy qudt:science ;
  rdfs:label "Resistance Unit" ;
  rdfs:subClassOf qudt:ElectricityAndMagnetismUnit ;
  rdfs:subClassOf [
      a owl:Restriction ;
      owl:hasValue quantitykind:Resistance ;
      owl:onProperty qudt:hasQuantityKind ;
    ] ;
  skos:exactMatch <http://dbpedia.org/resource/Category:Units_of_electrical_resistance> ;
.
qudt:ResourceUnit
  a owl:Class ;
  qudt:description "A Resource Unit is a unit for measuring the amount of various types of resources."^^rdf:HTML ;
  rdfs:isDefinedBy <http://qudt.org/2.0/schema/qudt/science> ;
  rdfs:isDefinedBy qudt:science ;
  rdfs:label "Resource Unit" ;
  rdfs:subClassOf qudt:MathsUnit ;
.
qudt:RespiratoryRateUnit
  a owl:Class ;
  dct:description "A sub-type of 'Biomedical Unit'. Detailed desciption to be provided in a future version." ;
  rdfs:isDefinedBy <http://qudt.org/2.0/schema/qudt/science> ;
  rdfs:isDefinedBy qudt:science ;
  rdfs:label "Respiratory Rate Unit" ;
  rdfs:subClassOf qudt:BiomedicalUnit ;
  rdfs:subClassOf [
      a owl:Restriction ;
      owl:hasValue quantitykind:RespiratoryRate ;
      owl:onProperty qudt:hasQuantityKind ;
    ] ;
.
qudt:RiskManagementQuantityKind
  a owl:Class ;
  dct:description "A sub-type of 'Management Quantity Kind'. Detailed desciption to be provided in a future version." ;
  rdfs:isDefinedBy <http://qudt.org/2.0/schema/qudt/science> ;
  rdfs:isDefinedBy qudt:science ;
  rdfs:label "Risk Management Quantity Kind" ;
  rdfs:subClassOf qudt:ManagementQuantityKind ;
.
qudt:Rule
  dct:description "A sub-type of 'QUDT Concept'. Detailed desciption to be provided in a future version." ;
.
qudt:SI-BaseUnit
  rdfs:isDefinedBy <http://qudt.org/schema/qudt> ;
.
qudt:SI-DerivedUnit
  rdfs:isDefinedBy <http://qudt.org/schema/qudt> ;
.
qudt:SI-DimensionVector
  dct:description "A sub-type of 'Quantity Dimension Vector'. Detailed desciption to be provided in a future version." ;
.
qudt:SI-Unit
  rdfs:isDefinedBy <http://qudt.org/schema/qudt> ;
.
qudt:ScaledUnit
  dct:description "A sub-type of 'Unit'. Detailed desciption to be provided in a future version." ;
.
qudt:ScienceQuantityKind
  a owl:Class ;
  dct:description "A sub-type of 'Quantity Kind'. Detailed desciption to be provided in a future version." ;
  rdfs:isDefinedBy <http://qudt.org/2.0/schema/qudt/science> ;
  rdfs:isDefinedBy qudt:science ;
  rdfs:label "Science Quantity Kind" ;
  rdfs:subClassOf qudt:QuantityKind ;
  skos:prefLabel "Science quantity kind" ;
.
qudt:ScienceUnit
  a owl:Class ;
  dct:description "A sub-type of 'Domain-specific Unit'. Detailed desciption to be provided in a future version." ;
  rdfs:isDefinedBy <http://qudt.org/2.0/schema/qudt/science> ;
  rdfs:isDefinedBy qudt:science ;
  rdfs:label "Science unit" ;
  rdfs:subClassOf qudt:DomainSpecificUnit ;
.
qudt:SerumOrPlasmaLevelUnit
  a owl:Class ;
  dct:description "A sub-type of 'Biomedical Unit'. Detailed desciption to be provided in a future version." ;
  rdfs:isDefinedBy <http://qudt.org/2.0/schema/qudt/science> ;
  rdfs:isDefinedBy qudt:science ;
  rdfs:label "Serum Or Plasma Level Unit" ;
  rdfs:subClassOf qudt:BiomedicalUnit ;
  rdfs:subClassOf [
      a owl:Restriction ;
      owl:hasValue quantitykind:SerumOrPlasmaLevel ;
      owl:onProperty qudt:hasQuantityKind ;
    ] ;
.
qudt:SignalDetectionThresholdUnit
  rdfs:isDefinedBy <http://qudt.org/schema/qudt> ;
  rdfs:subClassOf [
      a owl:Restriction ;
      owl:hasValue quantitykind:SignalDetectionThreshold ;
      owl:onProperty qudt:hasQuantityKind ;
    ] ;
.
qudt:SocialScienceQuantityKind
  a owl:Class ;
  dct:description "A sub-type of 'Science quantity kind'. Detailed desciption to be provided in a future version." ;
  rdfs:isDefinedBy <http://qudt.org/2.0/schema/qudt/science> ;
  rdfs:isDefinedBy qudt:science ;
  rdfs:label "Social Science Quantity Kind" ;
  rdfs:subClassOf qudt:ScienceQuantityKind ;
.
qudt:SoftwareEngineeringQuantityKind
  a owl:Class ;
  dct:description "A sub-type of 'Engineering quantity kind'. Detailed desciption to be provided in a future version." ;
  rdfs:isDefinedBy <http://qudt.org/2.0/schema/qudt/science> ;
  rdfs:isDefinedBy qudt:science ;
  rdfs:label "Software Engineering Quantity Kind" ;
  rdfs:subClassOf qudt:EngineeringQuantityKind ;
.
qudt:SolidAngleUnit
  a owl:Class ;
  qudt:description "The solid angle subtended by a surface S is defined as the surface area of a unit sphere covered by the surface S's projection onto the sphere. A solid angle is related to the surface of a sphere in the same way an ordinary angle is related to the circumference of a circle. Since the total surface area of the unit sphere is 4*pi, the measure of solid angle will always be between 0 and 4*pi."^^rdf:HTML ;
  rdfs:isDefinedBy <http://qudt.org/2.0/schema/qudt/science> ;
  rdfs:isDefinedBy qudt:science ;
  rdfs:label "Solid Angle Unit" ;
  rdfs:subClassOf qudt:AngleUnit ;
  rdfs:subClassOf [
      a owl:Restriction ;
      owl:hasValue quantitykind:SolidAngle ;
      owl:onProperty qudt:hasQuantityKind ;
    ] ;
.
qudt:SolidStatePhysicsQuantityKind
  a owl:Class ;
  dct:description "A sub-type of 'Physics Quantity Kind'. Detailed desciption to be provided in a future version." ;
  rdfs:isDefinedBy <http://qudt.org/2.0/schema/qudt/science> ;
  rdfs:isDefinedBy qudt:science ;
  rdfs:label "Solid State Physics Quantity Kind" ;
  rdfs:subClassOf qudt:PhysicsQuantityKind ;
.
qudt:SolidStatePhysicsUnit
  a owl:Class ;
  dct:description "A sub-type of 'Physics Unit'. Detailed desciption to be provided in a future version." ;
  qudt:fieldCode "780" ;
  rdfs:isDefinedBy <http://qudt.org/2.0/schema/qudt/science> ;
  rdfs:isDefinedBy qudt:science ;
  rdfs:label "Solid state physics unit" ;
  rdfs:subClassOf qudt:PhysicsUnit ;
.
qudt:SpaceAndTimeQuantityKind
  a owl:Class ;
  dct:description "A sub-type of 'Physics Quantity Kind'. Detailed desciption to be provided in a future version." ;
  rdfs:isDefinedBy <http://qudt.org/2.0/schema/qudt/science> ;
  rdfs:isDefinedBy qudt:science ;
  rdfs:label "Space and Time" ;
  rdfs:subClassOf qudt:PhysicsQuantityKind ;
.
qudt:SpaceAndTimeUnit
  a owl:Class ;
  dct:description "A sub-type of 'Physics Unit'. Detailed desciption to be provided in a future version." ;
  qudt:fieldCode "780" ;
  rdfs:isDefinedBy <http://qudt.org/2.0/schema/qudt/science> ;
  rdfs:isDefinedBy qudt:science ;
  rdfs:label "Space And Time Unit" ;
  rdfs:subClassOf qudt:PhysicsUnit ;
  rdfs:subClassOf [
      a owl:Restriction ;
      owl:allValuesFrom qudt:SpaceAndTimeQuantityKind ;
      owl:onProperty qudt:hasQuantityKind ;
    ] ;
  owl:equivalentClass [
      a owl:Restriction ;
      owl:allValuesFrom qudt:SpaceAndTimeQuantityKind ;
      owl:onProperty qudt:hasQuantityKind ;
    ] ;
.
qudt:SpaceSystemEngineeringQuantityKind
  a owl:Class ;
  dct:description "A sub-type of 'Engineering quantity kind'. Detailed desciption to be provided in a future version." ;
  rdfs:isDefinedBy <http://qudt.org/2.0/schema/qudt/science> ;
  rdfs:isDefinedBy qudt:science ;
  rdfs:label "Space System Engineering Quantity Kind" ;
  rdfs:subClassOf qudt:EngineeringQuantityKind ;
.
qudt:SpecificEnergyUnit
  a owl:Class ;
  qudt:description "Units which quantify specific energy, that is, energy per unit mass."^^rdf:HTML ;
  rdfs:isDefinedBy <http://qudt.org/2.0/schema/qudt/science> ;
  rdfs:isDefinedBy qudt:science ;
  rdfs:label "Specific Energy Unit" ;
  rdfs:subClassOf qudt:EnergyUnit ;
  rdfs:subClassOf [
      a owl:Restriction ;
      owl:hasValue quantitykind:SpecificEnergy ;
      owl:onProperty qudt:hasQuantityKind ;
    ] ;
.
qudt:SpecificHeatCapacityUnit
  a owl:Class ;
  dct:description "A sub-type of 'Thermodynamics Unit'. Detailed desciption to be provided in a future version." ;
  rdfs:isDefinedBy <http://qudt.org/2.0/schema/qudt/science> ;
  rdfs:isDefinedBy qudt:science ;
  rdfs:label "Specific Heat Capacity Unit" ;
  rdfs:subClassOf qudt:ThermodynamicsUnit ;
  rdfs:subClassOf [
      a owl:Restriction ;
      owl:hasValue quantitykind:SpecificHeatCapacity ;
      owl:onProperty qudt:hasQuantityKind ;
    ] ;
.
qudt:SpecificHeatPressureUnit
  a owl:Class ;
  qudt:description "This class contains units of measure for specific heat capacity at a constant pressure."^^rdf:HTML ;
  rdfs:isDefinedBy <http://qudt.org/2.0/schema/qudt/science> ;
  rdfs:isDefinedBy qudt:science ;
  rdfs:label "Specific Heat Pressure Unit" ;
  rdfs:subClassOf qudt:ThermodynamicsUnit ;
.
qudt:SpecificHeatVolumeUnit
  a owl:Class ;
  qudt:description "This class contains units of measure for specific heat capacity at a constant volume."^^rdf:HTML ;
  rdfs:isDefinedBy <http://qudt.org/2.0/schema/qudt/science> ;
  rdfs:isDefinedBy qudt:science ;
  rdfs:label "Specific Heat Volume Unit" ;
  rdfs:subClassOf qudt:ThermodynamicsUnit ;
.
qudt:SpectroscopyQuantityKind
  a owl:Class ;
  dct:description "A sub-type of 'Light quantity kind' and 'Physics Quantity Kind'. Detailed desciption to be provided in a future version." ;
  rdfs:isDefinedBy <http://qudt.org/2.0/schema/qudt/science> ;
  rdfs:isDefinedBy qudt:science ;
  rdfs:label "Spectroscopy Quantity Kind" ;
  rdfs:subClassOf qudt:LightQuantityKind ;
  rdfs:subClassOf qudt:PhysicsQuantityKind ;
.
qudt:StandardsUnit
  dct:description "A sub-type of 'Unit'. Detailed desciption to be provided in a future version." ;
.
qudt:StatisticalMechanicsQuantityKind
  a owl:Class ;
  dct:description "A sub-type of 'Mechanics Quantity Kind'. Detailed desciption to be provided in a future version." ;
  rdfs:isDefinedBy <http://qudt.org/2.0/schema/qudt/science> ;
  rdfs:isDefinedBy qudt:science ;
  rdfs:label "Statistical Mechanics Quantity Kind" ;
  rdfs:subClassOf qudt:MechanicsQuantityKind ;
.
qudt:StructuresAndMechanicsQuantityKind
  a owl:Class ;
  dct:description "A sub-type of 'Space System Engineering Quantity Kind'. Detailed desciption to be provided in a future version." ;
  dct:description "Determination of initial mass probabilities, centroids, moments of inertia, etc." ;
  rdfs:isDefinedBy <http://qudt.org/2.0/schema/qudt/science> ;
  rdfs:isDefinedBy qudt:science ;
  rdfs:label "Structures And Mechanics Quantity Kind" ;
  rdfs:subClassOf qudt:SpaceSystemEngineeringQuantityKind ;
.
qudt:StructuresQuantityKind
  a owl:Class ;
  dct:description "A sub-type of 'Structures And Mechanics Quantity Kind'. Detailed desciption to be provided in a future version." ;
  rdfs:isDefinedBy <http://qudt.org/2.0/schema/qudt/science> ;
  rdfs:isDefinedBy qudt:science ;
  rdfs:label "Structures Quantity Kind" ;
  rdfs:subClassOf qudt:StructuresAndMechanicsQuantityKind ;
.
qudt:Symbol
  dct:description "A sub-type of 'QUDT Concept'. Detailed desciption to be provided in a future version." ;
.
qudt:SystemDesignQuantityKind
  a owl:Class ;
  dct:description "A sub-type of 'System Engineering Quantity Kind'. Detailed desciption to be provided in a future version." ;
  rdfs:isDefinedBy <http://qudt.org/2.0/schema/qudt/science> ;
  rdfs:isDefinedBy qudt:science ;
  rdfs:label "System Design Quantity Kind" ;
  rdfs:subClassOf qudt:SystemEngineeringQuantityKind ;
.
qudt:SystemEngineeringQuantityKind
  a owl:Class ;
  dct:description "A sub-type of 'Engineering quantity kind'. Detailed desciption to be provided in a future version." ;
  rdfs:isDefinedBy <http://qudt.org/2.0/schema/qudt/science> ;
  rdfs:isDefinedBy qudt:science ;
  rdfs:label "System Engineering Quantity Kind" ;
  rdfs:subClassOf qudt:EngineeringQuantityKind ;
.
qudt:SystemIntegrationQuantityKind
  a owl:Class ;
  dct:description "A sub-type of 'System Engineering Quantity Kind'. Detailed desciption to be provided in a future version." ;
  rdfs:isDefinedBy <http://qudt.org/2.0/schema/qudt/science> ;
  rdfs:isDefinedBy qudt:science ;
  rdfs:label "System Integration Quantity Kind" ;
  rdfs:subClassOf qudt:SystemEngineeringQuantityKind ;
.
qudt:SystemOfNaturalUnits
  rdfs:isDefinedBy <http://qudt.org/schema/qudt> ;
.
qudt:SystemTestingQuantityKind
  a owl:Class ;
  dct:description "A sub-type of 'System Engineering Quantity Kind'. Detailed desciption to be provided in a future version." ;
  rdfs:isDefinedBy <http://qudt.org/2.0/schema/qudt/science> ;
  rdfs:isDefinedBy qudt:science ;
  rdfs:label "System Testing Quantity Kind" ;
  rdfs:subClassOf qudt:SystemEngineeringQuantityKind ;
.
qudt:TelebiometricsQuantityKind
  a owl:Class ;
  dct:description "A sub-type of 'Computer Science Quantity Kind'. Detailed desciption to be provided in a future version." ;
  rdfs:isDefinedBy <http://qudt.org/2.0/schema/qudt/science> ;
  rdfs:isDefinedBy qudt:science ;
  rdfs:label "Telebiometrics Quantity Kind" ;
  rdfs:subClassOf qudt:ComputerScienceQuantityKind ;
  skos:prefLabel "Telebiometrics Quantity Kind" ;
.
qudt:TelemetryQuantityKind
  a owl:Class ;
  dct:description "A sub-type of 'Space System Engineering Quantity Kind'. Detailed desciption to be provided in a future version." ;
  rdfs:isDefinedBy <http://qudt.org/2.0/schema/qudt/science> ;
  rdfs:isDefinedBy qudt:science ;
  rdfs:label "Telemetry Quantity Kind" ;
  rdfs:subClassOf qudt:SpaceSystemEngineeringQuantityKind ;
.
qudt:TemperaturePerTimeUnit
  a owl:Class ;
  dct:description "A sub-type of 'Thermodynamics Unit'. Detailed desciption to be provided in a future version." ;
  rdfs:isDefinedBy <http://qudt.org/2.0/schema/qudt/science> ;
  rdfs:isDefinedBy qudt:science ;
  rdfs:label "Temperature per time unit" ;
  rdfs:subClassOf qudt:ThermodynamicsUnit ;
.
qudt:TemperatureUnit
  a owl:Class ;
  dct:description "A sub-type of 'Thermodynamics Unit'. Detailed desciption to be provided in a future version." ;
  rdfs:isDefinedBy <http://qudt.org/2.0/schema/qudt/science> ;
  rdfs:isDefinedBy qudt:science ;
  rdfs:label "Temperature Unit" ;
  rdfs:subClassOf qudt:ThermodynamicsUnit ;
  rdfs:subClassOf [
      a owl:Restriction ;
      owl:hasValue quantitykind:ThermodynamicTemperature ;
      owl:onProperty qudt:hasQuantityKind ;
    ] ;
  skos:exactMatch <http://dbpedia.org/resource/Category:Units_of_temperature> ;
.
qudt:ThermalConductivityUnit
  a owl:Class ;
  dct:description "A sub-type of 'Thermodynamics Unit'. Detailed desciption to be provided in a future version." ;
  rdfs:isDefinedBy <http://qudt.org/2.0/schema/qudt/science> ;
  rdfs:isDefinedBy qudt:science ;
  rdfs:label "Thermal Conductivity Unit" ;
  rdfs:subClassOf qudt:ThermodynamicsUnit ;
  rdfs:subClassOf [
      a owl:Restriction ;
      owl:hasValue quantitykind:ThermalConductivity ;
      owl:onProperty qudt:hasQuantityKind ;
    ] ;
.
qudt:ThermalControlQuantityKind
  a owl:Class ;
  dct:description "A sub-type of 'Space System Engineering Quantity Kind'. Detailed desciption to be provided in a future version." ;
  rdfs:isDefinedBy <http://qudt.org/2.0/schema/qudt/science> ;
  rdfs:isDefinedBy qudt:science ;
  rdfs:label "Thermal Control Quantity Kind" ;
  rdfs:subClassOf qudt:SpaceSystemEngineeringQuantityKind ;
.
qudt:ThermalDiffusivityUnit
  a owl:Class ;
  dct:description "A sub-type of 'Thermodynamics Unit'. Detailed desciption to be provided in a future version." ;
  rdfs:isDefinedBy <http://qudt.org/2.0/schema/qudt/science> ;
  rdfs:isDefinedBy qudt:science ;
  rdfs:label "Thermal Diffusivity Unit" ;
  rdfs:subClassOf qudt:ThermodynamicsUnit ;
  rdfs:subClassOf [
      a owl:Restriction ;
      owl:hasValue quantitykind:ThermalDiffusivity ;
      owl:onProperty qudt:hasQuantityKind ;
    ] ;
.
qudt:ThermalEnergyLengthUnit
  a owl:Class ;
  dct:description "A sub-type of 'Thermodynamics Unit'. Detailed desciption to be provided in a future version." ;
  rdfs:isDefinedBy <http://qudt.org/2.0/schema/qudt/science> ;
  rdfs:isDefinedBy qudt:science ;
  rdfs:label "Thermal Energy Length Unit" ;
  rdfs:subClassOf qudt:ThermodynamicsUnit ;
  rdfs:subClassOf [
      a owl:Restriction ;
      owl:hasValue quantitykind:ThermalEnergyLength ;
      owl:onProperty qudt:hasQuantityKind ;
    ] ;
.
qudt:ThermalEnergyUnit
  a owl:Class ;
  dct:description "A sub-type of 'Thermodynamics Unit'. Detailed desciption to be provided in a future version." ;
  rdfs:isDefinedBy <http://qudt.org/2.0/schema/qudt/science> ;
  rdfs:isDefinedBy qudt:science ;
  rdfs:label "Thermal Energy Unit" ;
  rdfs:subClassOf qudt:ThermodynamicsUnit ;
  rdfs:subClassOf [
      a owl:Restriction ;
      owl:hasValue quantitykind:EnergyAndWork ;
      owl:onProperty qudt:hasQuantityKind ;
    ] ;
  rdfs:subClassOf [
      a owl:Restriction ;
      owl:hasValue quantitykind:ThermalEnergy ;
      owl:onProperty qudt:hasQuantityKind ;
    ] ;
.
qudt:ThermalEngineeringQuantityKind
  a owl:Class ;
  dct:description "A sub-type of 'Engineering quantity kind'. Detailed desciption to be provided in a future version." ;
  rdfs:isDefinedBy <http://qudt.org/2.0/schema/qudt/science> ;
  rdfs:isDefinedBy qudt:science ;
  rdfs:label "Thermal Engineering Quantity Kind" ;
  rdfs:subClassOf qudt:EngineeringQuantityKind ;
.
qudt:ThermalExpansionUnit
  a owl:Class ;
  qudt:description """When the temperature of a substance changes, the energy that is stored in the intermolecular bonds between atoms changes. When the stored energy increases, so does the length of the molecular bonds. As a result, solids typically expand in response to heating and contract on cooling; this dimensional response to temperature change is expressed by its coefficient of thermal expansion.



Different coefficients of thermal expansion can be defined for a substance depending on whether the expansion is measured by:



    * linear thermal expansion

    * area thermal expansion

    * volumetric thermal expansion



These characteristics are closely related. The volumetric thermal expansion coefficient can be defined for both liquids and solids. The linear thermal expansion can only be defined for solids, and is common in engineering applications.



Some substances expand when cooled, such as freezing water, so they have negative thermal expansion coefficients. [Wikipedia]"""^^rdf:HTML ;
  rdfs:isDefinedBy <http://qudt.org/2.0/schema/qudt/science> ;
  rdfs:isDefinedBy qudt:science ;
  rdfs:label "Thermal Expansion Unit" ;
  rdfs:subClassOf qudt:ThermodynamicsUnit ;
.
qudt:ThermalHeatCapacityUnit
  a owl:Class ;
  dct:description "A sub-type of 'Specific Energy Unit' and 'Thermodynamics Unit'. Detailed desciption to be provided in a future version." ;
  rdfs:isDefinedBy <http://qudt.org/2.0/schema/qudt/science> ;
  rdfs:isDefinedBy qudt:science ;
  rdfs:label "Thermal Heat Capacity Unit" ;
  rdfs:subClassOf qudt:SpecificEnergyUnit ;
  rdfs:subClassOf qudt:ThermodynamicsUnit ;
.
qudt:ThermalInsulanceUnit
  a owl:Class ;
  dct:description "A sub-type of 'Thermodynamics Unit'. Detailed desciption to be provided in a future version." ;
  rdfs:isDefinedBy <http://qudt.org/2.0/schema/qudt/science> ;
  rdfs:isDefinedBy qudt:science ;
  rdfs:label "Thermal Insulance Unit" ;
  rdfs:subClassOf qudt:ThermodynamicsUnit ;
  rdfs:subClassOf [
      a owl:Restriction ;
      owl:hasValue quantitykind:ThermalInsulance ;
      owl:onProperty qudt:hasQuantityKind ;
    ] ;
.
qudt:ThermalProtectionQuantityKind
  a owl:Class ;
  dct:description "A sub-type of 'Space System Engineering Quantity Kind'. Detailed desciption to be provided in a future version." ;
  rdfs:isDefinedBy <http://qudt.org/2.0/schema/qudt/science> ;
  rdfs:isDefinedBy qudt:science ;
  rdfs:label "Thermal Protection Quantity Kind" ;
  rdfs:subClassOf qudt:SpaceSystemEngineeringQuantityKind ;
.
qudt:ThermalResistanceUnit
  a owl:Class ;
  dct:description "A sub-type of 'Thermodynamics Unit'. Detailed desciption to be provided in a future version." ;
  rdfs:isDefinedBy <http://qudt.org/2.0/schema/qudt/science> ;
  rdfs:isDefinedBy qudt:science ;
  rdfs:label "Thermal Resistance Unit" ;
  rdfs:subClassOf qudt:ThermodynamicsUnit ;
  rdfs:subClassOf [
      a owl:Restriction ;
      owl:hasValue quantitykind:ThermalResistance ;
      owl:onProperty qudt:hasQuantityKind ;
    ] ;
.
qudt:ThermalResistivityUnit
  a owl:Class ;
  dct:description "A sub-type of 'Thermodynamics Unit'. Detailed desciption to be provided in a future version." ;
  rdfs:isDefinedBy <http://qudt.org/2.0/schema/qudt/science> ;
  rdfs:isDefinedBy qudt:science ;
  rdfs:label "Thermal Resistivity Unit" ;
  rdfs:subClassOf qudt:ThermodynamicsUnit ;
  rdfs:subClassOf [
      a owl:Restriction ;
      owl:hasValue quantitykind:ThermalResistivity ;
      owl:onProperty qudt:hasQuantityKind ;
    ] ;
.
qudt:ThermodynamicsQuantityKind
  a owl:Class ;
  dct:description "A sub-type of 'Mechanics Quantity Kind'. Detailed desciption to be provided in a future version." ;
  rdfs:isDefinedBy <http://qudt.org/2.0/schema/qudt/science> ;
  rdfs:isDefinedBy qudt:science ;
  rdfs:label "Thermodynamics" ;
  rdfs:subClassOf qudt:MechanicsQuantityKind ;
  skos:exactMatch <http://dbpedia.org/resource/Thermodynamics> ;
.
qudt:ThermodynamicsUnit
  a owl:Class ;
  qudt:description "Thermodynamics units are units that provide reference scales for quantifying the conversion of energy into work, as well as heat and its relation to macroscopic variables such as temperature and pressure."^^rdf:HTML ;
  qudt:fieldCode "790" ;
  rdfs:isDefinedBy <http://qudt.org/2.0/schema/qudt/science> ;
  rdfs:isDefinedBy qudt:science ;
  rdfs:label "Thermodynamics Unit" ;
  rdfs:subClassOf qudt:PhysicsUnit ;
  rdfs:subClassOf [
      a owl:Restriction ;
      owl:allValuesFrom qudt:ThermodynamicsQuantityKind ;
      owl:onProperty qudt:hasQuantityKind ;
    ] ;
  owl:equivalentClass [
      a owl:Restriction ;
      owl:allValuesFrom qudt:ThermodynamicsQuantityKind ;
      owl:onProperty qudt:hasQuantityKind ;
    ] ;
  skos:closeMatch <http://dbpedia.org/resource/Category:Thermodynamics> ;
.
qudt:ThrustToMassRatioUnit
  a owl:Class ;
  dct:description "A sub-type of 'Force Unit' and 'Mass Unit'. Detailed desciption to be provided in a future version." ;
  rdfs:isDefinedBy <http://qudt.org/2.0/schema/qudt/science> ;
  rdfs:isDefinedBy qudt:science ;
  rdfs:label "Thrust To Mass Ratio Unit" ;
  rdfs:subClassOf qudt:ForceUnit ;
  rdfs:subClassOf qudt:MassUnit ;
  rdfs:subClassOf [
      a owl:Restriction ;
      owl:hasValue quantitykind:ThrustToMassRatio ;
      owl:onProperty qudt:hasQuantityKind ;
    ] ;
.
qudt:TimeUnit
  a owl:Class ;
  qudt:description "Units that measure time."^^rdf:HTML ;
  rdfs:isDefinedBy <http://qudt.org/2.0/schema/qudt/science> ;
  rdfs:isDefinedBy qudt:science ;
  rdfs:label "Time Unit" ;
  rdfs:subClassOf qudt:SpaceAndTimeUnit ;
  skos:exactMatch <http://dbpedia.org/resource/Category:Units_of_time> ;
.
qudt:TradeStudiesQuantityKind
  a owl:Class ;
  dct:description "A sub-type of 'Management Quantity Kind'. Detailed desciption to be provided in a future version." ;
  rdfs:isDefinedBy <http://qudt.org/2.0/schema/qudt/science> ;
  rdfs:isDefinedBy qudt:science ;
  rdfs:label "Trade studies" ;
  rdfs:subClassOf qudt:ManagementQuantityKind ;
.
qudt:TrajectoryQuantityKind
  a owl:Class ;
  dct:description "A sub-type of 'Space System Engineering Quantity Kind'. Detailed desciption to be provided in a future version." ;
  dct:description "Planet-centric and Heliocentric trajectory analysis" ;
  rdfs:isDefinedBy <http://qudt.org/2.0/schema/qudt/science> ;
  rdfs:isDefinedBy qudt:science ;
  rdfs:label "Trajectory Quantity Kind" ;
  rdfs:subClassOf qudt:SpaceSystemEngineeringQuantityKind ;
.
qudt:TransformType
  a owl:Class ;
  rdfs:isDefinedBy <http://qudt.org/2.0/schema/qudt/science> ;
  rdfs:isDefinedBy qudt:science ;
  rdfs:label "Transform type" ;
  rdfs:subClassOf qudt:EnumeratedValue ;
  skos:prefLabel "Transform type" ;
.
qudt:TurbidityUnit
  a owl:Class ;
  qudt:description "Turbidity is the cloudiness or haziness of a fluid caused by individual particles (suspended solids) that are generally invisible to the naked eye, similar to smoke in air."^^rdf:HTML ;
  rdfs:isDefinedBy <http://qudt.org/2.0/schema/qudt/science> ;
  rdfs:isDefinedBy qudt:science ;
  rdfs:label "Turbidity Unit" ;
  rdfs:subClassOf qudt:BiomedicalUnit ;
  rdfs:subClassOf [
      a owl:Restriction ;
      owl:hasValue quantitykind:Turbidity ;
      owl:onProperty qudt:hasQuantityKind ;
    ] ;
.
qudt:US-CustomaryUnit
  dct:description "A sub-type of 'Standards unit'. Detailed desciption to be provided in a future version." ;
.
qudt:US-SurveyUnit
  dct:description "A sub-type of 'Standards unit'. Detailed desciption to be provided in a future version." ;
.
qudt:Unit
  rdfs:isDefinedBy <http://qudt.org/schema/qudt> ;
  rdfs:subClassOf [
      a owl:Restriction ;
      owl:maxCardinality "1"^^xsd:nonNegativeInteger ;
      owl:onProperty qudt:isMetricUnit ;
    ] ;
.
qudt:UsedWithSI-Unit
  rdfs:isDefinedBy <http://qudt.org/schema/qudt> ;
.
qudt:VelocityUnit
  a owl:Class ;
  dct:description "A sub-type of 'Space And Time Unit'. Detailed desciption to be provided in a future version." ;
  rdfs:isDefinedBy <http://qudt.org/2.0/schema/qudt/science> ;
  rdfs:isDefinedBy qudt:science ;
  rdfs:label "Velocity Unit" ;
  rdfs:subClassOf qudt:SpaceAndTimeUnit ;
  rdfs:subClassOf [
      a owl:Restriction ;
      owl:hasValue quantitykind:Velocity ;
      owl:onProperty qudt:hasQuantityKind ;
    ] ;
.
qudt:VibrationQuantityKind
  a owl:Class ;
  dct:description "A sub-type of 'Mechanics Quantity Kind'. Detailed desciption to be provided in a future version." ;
  dct:description "Vibration is a mechanical phenomenon whereby oscillations occur about an equilibrium point." ;
  rdfs:isDefinedBy <http://qudt.org/2.0/schema/qudt/science> ;
  rdfs:isDefinedBy qudt:science ;
  rdfs:label "Vibration Quantity Kind" ;
  rdfs:subClassOf qudt:MechanicsQuantityKind ;
  prov:wasInfluencedBy <http://en.wikipedia.org/wiki/Vibration> ;
.
qudt:VideoFrameRateUnit
  a owl:Class ;
  dct:description "A sub-type of 'Informatics Unit'. Detailed desciption to be provided in a future version." ;
  rdfs:isDefinedBy <http://qudt.org/2.0/schema/qudt/science> ;
  rdfs:isDefinedBy qudt:science ;
  rdfs:label "Video Frame Rate Unit" ;
  rdfs:subClassOf qudt:InformaticsUnit ;
  rdfs:subClassOf [
      a owl:Restriction ;
      owl:hasValue quantitykind:VideoFrameRate ;
      owl:onProperty qudt:hasQuantityKind ;
    ] ;
.
qudt:ViscosityUnit
  a owl:Class ;
  qudt:description """<p class=\"lm-para\"><b>Viscosity</b> is a measure of the resistance of a fluid which is being deformed by either shear stress or tensile stress. In everyday terms (and for fluids only), viscosity is \"thickness\" or \"internal friction\". Thus, water is \"thin\", having a lower viscosity, while honey is \"thick\", having a higher viscosity. Put simply, the less viscous the fluid is, the greater its ease of movement (fluidity). Fluids resist the relative motion of immersed objects through them as well as to the motion of layers with differing velocities within them.</p>
<p class=\"lm-para\">Formally, viscosity (represented by the symbol \\(\\eta\\) (\"eta\") is the ratio of the shearing stress (\\(f/A\\)) to the velocity gradient (\\(\\Delta v_x / \\Delta  z\\)  or \\(dv_x / dz\\)) in a fluid.</p>
<p class=\"lm-para\">The SI quantity quantity for viscosity is sometimes called <i>dynamic viscosity</i>, <i>absolute viscosity</i>, or <i>simple viscosity</i>, but is usually just called <i>viscosity</i>.</p>"""^^rdf:HTML ;
  rdfs:isDefinedBy <http://qudt.org/2.0/schema/qudt/science> ;
  rdfs:isDefinedBy qudt:science ;
  rdfs:label "Viscosity Units" ;
  rdfs:subClassOf qudt:MechanicsUnit ;
  prov:wasInfluencedBy <http://en.wikipedia.org/wiki/Viscosity> ;
  prov:wasInfluencedBy <http://physics.info/viscosity/> ;
.
qudt:VolumeThermalExpansionUnit
  a owl:Class ;
  qudt:description """<p class=\"lm-para\">When the temperature of a substance changes, the energy that is stored in the intermolecular bonds between atoms changes. When the stored energy increases, so does the length of the molecular bonds. As a result, solids typically expand in response to heating and contract on cooling; this dimensional response to temperature change is expressed by its coefficient of thermal expansion.</p>
<p class=\"lm-para\">Different coefficients of thermal expansion can be defined for a substance depending on whether the expansion is measured by:</p>
<ul>
<li>linear thermal expansion</li>
<li>area thermal expansion</li>
<li>volumetric thermal expansion</li>
</ul>
<p class=\"lm-para\">These characteristics are closely related. The volumetric thermal expansion coefficient can be defined for both liquids and solids. The linear thermal expansion can only be defined for solids, and is common in engineering applications.</p>
<p class=\"lm-para\">Some substances expand when cooled, such as freezing water, so they have negative thermal expansion coefficients. For exactly isotropic materials, the volumetric thermal expansion coefficient is very closely approximated as three times the linear coefficient.</p>"""^^rdf:HTML ;
  rdfs:isDefinedBy <http://qudt.org/2.0/schema/qudt/science> ;
  rdfs:isDefinedBy qudt:science ;
  rdfs:label "Volume Thermal Expansion Unit" ;
  rdfs:subClassOf qudt:ThermalExpansionUnit ;
  rdfs:subClassOf [
      a owl:Restriction ;
      owl:hasValue quantitykind:VolumeThermalExpansion ;
      owl:onProperty qudt:hasQuantityKind ;
    ] ;
  prov:wasInfluencedBy <http://hyperphysics.phy-astr.gsu.edu/hbase/thermo/thexp2.html> ;
  prov:wasInfluencedBy <http://physics.info/expansion/> ;
  prov:wasInfluencedBy <http://www.engineeringtoolbox.com/volumetric-temperature-expansion-d_315.html> ;
  prov:wasInfluencedBy <https://en.wikipedia.org/wiki/Thermal_expansion> ;
.
qudt:VolumeUnit
  a owl:Class ;
  qudt:description "A \"Space And Time\" Unit with the following instance(s): \"Cubic foot per minute\", \"Cubic foot per second\", \"Cubic inch per minute\", \"Cubic meter per second\", \"Cubic yard per minute\", \"Gallon per day\", \"Gallon per minute\"."^^rdf:HTML ;
  rdfs:isDefinedBy <http://qudt.org/2.0/schema/qudt/science> ;
  rdfs:isDefinedBy qudt:science ;
  rdfs:label "Volume per Time Squared Unit" ;
  rdfs:subClassOf qudt:SpaceAndTimeUnit ;
  skos:exactMatch <http://dbpedia.org/resource/Category:Units_of_volume> ;
.
qudt:floatPercentage
  rdfs:isDefinedBy <http://qudt.org/schema/qudt> ;
.
qudt:integerPercentage
  rdfs:isDefinedBy <http://qudt.org/schema/qudt> ;
.
vaem:GMD_QUDT-SCHEMA-SCIENCE
  a vaem:GraphMetaData ;
  dct:author "Ralph Hodgson" ;
  dct:contributor "Daniel Mekonnen" ;
  dct:contributor "David Price" ;
  dct:contributor "James E. Masters" ;
  dct:contributor "Steve Ray" ;
  dct:created "2011-04-20"^^xsd:date ;
  dct:creator "Ralph Hodgson" ;
  dct:description "The science domain of QUDT defines the base classes properties, and restrictions used for modeling physical quantities, units of measure, and their dimensions for upper level domains of science and mathematics. The goal of the QUDT ontology is to provide a unified model of, measurable quantities, units for measuring different kinds of quantities, the numerical values of quantities in different units of measure and the data structures and data types used to store and manipulate these objects in software. Except for unit prefixes, all units are specified in separate vocabularies. Descriptions are provided in both HTML and LaTeX formats. " ;
  dct:modified "2019-10-04T12:30:51.335-07:00"^^xsd:dateTime ;
  dct:rights "The QUDT Ontologies are issued under a Creative Commons Attribution 4.0 International License (CC BY 4.0), available at https://creativecommons.org/licenses/by/4.0/. Attribution should be made to QUDT.org" ;
  dct:subject "Schema for Science and Mathematics Quantities, Units, Dimensions and Types" ;
  dct:title "QUDT Schema for Science and Mathematics- Version 2.0" ;
  vaem:hasGraphRole vaem:SchemaGraph ;
  vaem:hasLicenseType voag:CC-SHAREALIKE_3PT0-US ;
  vaem:hasOwner vaem:QUDT ;
  vaem:hasSteward vaem:QUDT ;
  vaem:intent "This ontology specifies classes for Science and Mathematics units and quantity kinds. Instances are held in spearate graphs." ;
  vaem:isMetadataFor "http://qudt.org/2.0/schema/qudt/science" ;
  vaem:latestPublishedVersion "http://www.qudt.org/doc/2017/DOC_SCHEMA-QUDT-SCIENCE-v2.0.html"^^xsd:anyURI ;
  vaem:logo "http://www.linkedmodel.org/lib/lm/images/logos/qudt_logo-300x110.png"^^xsd:anyURI ;
  vaem:name "qudt" ;
  vaem:namespace "http://qudt.org/schema/qudt/" ;
  vaem:namespacePrefix "qudt" ;
  vaem:owner "QUDT.org" ;
  vaem:revision "2.0" ;
  vaem:title "QUDT Schema for Science and Mathematics - Version 2.0" ;
  vaem:turtleFileURL "http://qudt.org/2.0/schema/SCHEMA_QUDT-SCIENCE-v2.0.ttl"^^xsd:anyURI ;
  vaem:usesNonImportedResource dct:abstract ;
  vaem:usesNonImportedResource dct:author ;
  vaem:usesNonImportedResource dct:contributor ;
  vaem:usesNonImportedResource dct:created ;
  vaem:usesNonImportedResource dct:description ;
  vaem:usesNonImportedResource dct:modified ;
  vaem:usesNonImportedResource dct:rights ;
  vaem:usesNonImportedResource dct:source ;
  vaem:usesNonImportedResource dct:subject ;
  vaem:usesNonImportedResource dct:title ;
  vaem:usesNonImportedResource voag:QUDT-Attribution ;
  vaem:usesNonImportedResource <http://voag.linkedmodel.org/voag/CC-SHAREALIKE_3PT0-US> ;
  vaem:usesNonImportedResource skos:closeMatch ;
  vaem:usesNonImportedResource skos:exactMatch ;
  vaem:usesNonImportedResource prov:wasInfluencedBy ;
  vaem:withAttributionTo voag:QUDT-Attribution ;
  rdfs:isDefinedBy <http://qudt.org/2.0/schema/qudt/science> ;
  rdfs:isDefinedBy qudt:science ;
  rdfs:label "QUDT Schema for Science and Mathematics - Version 2.0" ;
  owl:versionIRI <http://qudt.org/2.0/schema/qudt/science> ;
.
<http://www.w3.org/2004/02/skos/core>
  vaem:namespace "http://www.w3.org/2004/02/skos/core#"^^xsd:anyURI ;
  vaem:namespacePrefix "skos" ;
.
skos:closeMatch
  a rdf:Property ;
  rdfs:label "close match" ;
.
skos:exactMatch
  a rdf:Property ;
  rdfs:label "exact match" ;
.
prov:wasInfluencedBy
  a owl:ObjectProperty ;
.
